<?xml version="1.0"?>
<rdf:RDF xmlns="http://www.openmicroscopy.org/rdf/2016-06/ome_core/"
     xml:base="http://www.openmicroscopy.org/rdf/2016-06/ome_core/"
     xmlns:owl="http://www.w3.org/2002/07/owl#"
     xmlns:rdf="http://www.w3.org/1999/02/22-rdf-syntax-ns#"
     xmlns:xml="http://www.w3.org/XML/1998/namespace"
     xmlns:xsd="http://www.w3.org/2001/XMLSchema#"
     xmlns:mbmp="http://www.openmicroscopy.org/rdf/2016-06/ome_core/MicrobeamManipuration#"
     xmlns:rdfs="http://www.w3.org/2000/01/rdf-schema#"
     xmlns:expType="http://www.openmicroscopy.org/rdf/2016-06/ome_core/ExperimentType#">
    <owl:Ontology rdf:about="http://www.openmicroscopy.org/rdf/ome_core/">
        <owl:versionIRI rdf:resource="http://www.openmicroscopy.org/rdf/2016-06/ome_core/"/>
        <rdfs:comment xml:lang="en">The OME ontology provides a set of concepts for all information objects described as metadata accessible by OME.  These information objects are parts of metadata include descriptions of the imaging experiments and the people who perform them, descriptions of the microscope, the resulting images and how they were acquired, the analyses performed on those images, and the analysis results themselves. An OME metadata may contain any or all of this information. This is the initial version of OWL-based OME data model ontology generated by Norio Kobayashi at RIKEN.</rdfs:comment>
        <rdfs:label xml:lang="en">OME data model core ontology</rdfs:label>
        <owl:versionInfo xml:lang="en">2016-06</owl:versionInfo>
    </owl:Ontology>
    


    <!-- 
    ///////////////////////////////////////////////////////////////////////////////////////
    //
    // Annotation properties
    //
    ///////////////////////////////////////////////////////////////////////////////////////
     -->

    


    <!-- http://www.w3.org/2000/01/rdf-schema#common -->

    <owl:AnnotationProperty rdf:about="http://www.w3.org/2000/01/rdf-schema#common"/>
    


    <!-- http://www.w3.org/2000/01/rdf-schema#label -->

    <rdf:Description rdf:about="http://www.w3.org/2000/01/rdf-schema#label">
        <rdfs:label xml:lang="en">label</rdfs:label>
        <rdfs:range rdf:resource="http://www.w3.org/2001/XMLSchema#string"/>
    </rdf:Description>
    


    <!-- http://www.w3.org/2000/01/rdf-schema#lael -->

    <owl:AnnotationProperty rdf:about="http://www.w3.org/2000/01/rdf-schema#lael"/>
    


    <!-- 
    ///////////////////////////////////////////////////////////////////////////////////////
    //
    // Datatypes
    //
    ///////////////////////////////////////////////////////////////////////////////////////
     -->

    


    <!-- http://www.w3.org/2001/XMLSchema#anyURI -->

    <rdfs:Datatype rdf:about="http://www.w3.org/2001/XMLSchema#anyURI">
        <rdfs:comment xml:lang="en">The anyURI data type is used to specify a URI.</rdfs:comment>
    </rdfs:Datatype>
    


    <!-- http://www.w3.org/2001/XMLSchema#boolean -->

    <rdfs:Datatype rdf:about="http://www.w3.org/2001/XMLSchema#boolean">
        <rdfs:comment xml:lang="en">The boolean data type is used to specify a true or false value.</rdfs:comment>
    </rdfs:Datatype>
    


    <!-- http://www.w3.org/2001/XMLSchema#dateTime -->

    <rdfs:Datatype rdf:about="http://www.w3.org/2001/XMLSchema#dateTime">
        <rdfs:comment xml:lang="en">The dateTime data type is used to specify a date and a time. The dateTime is specified in the following form &quot;YYYY-MM-DDThh:mm:ss&quot; where: YYYY indicates the year, MM indicates the month, DD indicates the day, T indicates the start of the required time section, hh indicates the hour, mm indicates the minute and ss indicates the second.</rdfs:comment>
    </rdfs:Datatype>
    


    <!-- http://www.w3.org/2001/XMLSchema#float -->

    <rdfs:Datatype rdf:about="http://www.w3.org/2001/XMLSchema#float">
        <rdfs:comment xml:lang="en">float is patterned after the IEEE single-precision 32-bit floating point type.</rdfs:comment>
    </rdfs:Datatype>
    


    <!-- http://www.w3.org/2001/XMLSchema#nonNegativeInteger -->

    <rdfs:Datatype rdf:about="http://www.w3.org/2001/XMLSchema#nonNegativeInteger">
        <rdfs:comment xml:lang="en">An integer containing only non-negative values.</rdfs:comment>
    </rdfs:Datatype>
    


    <!-- http://www.w3.org/2001/XMLSchema#positiveInteger -->

    <rdfs:Datatype rdf:about="http://www.w3.org/2001/XMLSchema#positiveInteger">
        <rdfs:comment xml:lang="en">An integer containing only positive values.</rdfs:comment>
    </rdfs:Datatype>
    


    <!-- http://www.w3.org/2001/XMLSchema#string -->

    <rdfs:Datatype rdf:about="http://www.w3.org/2001/XMLSchema#string">
        <rdfs:comment xml:lang="en">The string data type can contain characters, line feeds, carriage returns, and tab characters.</rdfs:comment>
    </rdfs:Datatype>
    


    <!-- 
    ///////////////////////////////////////////////////////////////////////////////////////
    //
    // Object Properties
    //
    ///////////////////////////////////////////////////////////////////////////////////////
     -->

    


    <!-- http://qudt.org/schema/qudt#unit -->

    <owl:ObjectProperty rdf:about="http://qudt.org/schema/qudt#unit">
        <rdfs:comment xml:lang="en">Property &quot;http://qudt.org/schema/qudt#unit&quot; specifies the appropriate unit of measure.</rdfs:comment>
        <rdfs:label xml:lang="en">unit</rdfs:label>
    </owl:ObjectProperty>
    


    <!-- http://www.openmicroscopy.org/rdf/2016-06/ome_core/acquisitionMode -->

    <owl:ObjectProperty rdf:about="http://www.openmicroscopy.org/rdf/2016-06/ome_core/acquisitionMode">
        <rdfs:domain rdf:resource="http://www.openmicroscopy.org/rdf/2016-06/ome_core/Channel"/>
        <rdfs:comment xml:lang="en">Property &quot;acquisitionMode&quot; specifies the acquisition mode that describes the type of microscopy performed for each channel.</rdfs:comment>
        <rdfs:label xml:lang="en">acquisition mode</rdfs:label>
    </owl:ObjectProperty>
    


    <!-- http://www.openmicroscopy.org/rdf/2016-06/ome_core/airPressure -->

    <owl:ObjectProperty rdf:about="http://www.openmicroscopy.org/rdf/2016-06/ome_core/airPressure">
        <rdfs:domain rdf:resource="http://www.openmicroscopy.org/rdf/2016-06/ome_core/ImagingEnvironment"/>
        <rdfs:comment xml:lang="en">Property &quot;airPressure&quot; specifies the air pressure which is the define units.</rdfs:comment>
        <rdfs:label xml:lang="en">air pressure</rdfs:label>
    </owl:ObjectProperty>
    


    <!-- http://www.openmicroscopy.org/rdf/2016-06/ome_core/annotation -->

    <owl:ObjectProperty rdf:about="http://www.openmicroscopy.org/rdf/2016-06/ome_core/annotation">
        <rdfs:domain rdf:resource="http://www.openmicroscopy.org/rdf/2016-06/ome_core/Dataset"/>
        <rdfs:domain rdf:resource="http://www.openmicroscopy.org/rdf/2016-06/ome_core/Experiment"/>
        <rdfs:domain rdf:resource="http://www.openmicroscopy.org/rdf/2016-06/ome_core/ExperimenterGroup"/>
        <rdfs:domain rdf:resource="http://www.openmicroscopy.org/rdf/2016-06/ome_core/Image"/>
        <rdfs:domain rdf:resource="http://www.openmicroscopy.org/rdf/2016-06/ome_core/Project"/>
        <rdfs:domain rdf:resource="http://www.openmicroscopy.org/rdf/2016-06/ome_core/ReagentSet"/>
        <rdfs:domain rdf:resource="http://www.openmicroscopy.org/rdf/2016-06/ome_core/Well"/>
        <rdfs:range rdf:resource="http://www.openmicroscopy.org/rdf/2016-06/ome_core/Annotation"/>
        <rdfs:comment xml:lang="en">Property &quot;annotation&quot; specifies the annotation from which all others are ultimately derived.</rdfs:comment>
        <rdfs:label xml:lang="en">annotation</rdfs:label>
    </owl:ObjectProperty>
    


    <!-- http://www.openmicroscopy.org/rdf/2016-06/ome_core/annotator -->

    <owl:ObjectProperty rdf:about="http://www.openmicroscopy.org/rdf/2016-06/ome_core/annotator">
        <rdfs:domain rdf:resource="http://www.openmicroscopy.org/rdf/2016-06/ome_core/Annotation"/>
        <rdfs:range rdf:resource="http://xmlns.com/foaf/0.1/Person"/>
        <rdfs:comment xml:lang="en">Property &quot;annotator&quot; specifies  the person who attached this annotation.  e.g. If UserA annotates something with TagB, owned by UserB, UserA is still the Annotator.</rdfs:comment>
        <rdfs:label xml:lang="en">annotator</rdfs:label>
    </owl:ObjectProperty>
    


    <!-- http://www.openmicroscopy.org/rdf/2016-06/ome_core/binData -->

    <owl:ObjectProperty rdf:about="http://www.openmicroscopy.org/rdf/2016-06/ome_core/binData">
        <rdfs:domain rdf:resource="http://www.openmicroscopy.org/rdf/2016-06/ome_core/Pixels"/>
        <rdfs:range rdf:resource="http://www.openmicroscopy.org/rdf/2016-06/ome_core/BinData"/>
        <rdfs:common xml:lang="en">Property &quot;bindata&quot; specifies the binary data which are base64-encoded.</rdfs:common>
        <rdfs:label xml:lang="en">bin data</rdfs:label>
    </owl:ObjectProperty>
    


    <!-- http://www.openmicroscopy.org/rdf/2016-06/ome_core/binFile -->

    <owl:ObjectProperty rdf:about="http://www.openmicroscopy.org/rdf/2016-06/ome_core/binFile">
        <rdfs:domain rdf:resource="http://www.openmicroscopy.org/rdf/2016-06/ome_core/FileAnnotation"/>
        <rdfs:range rdf:resource="http://www.openmicroscopy.org/rdf/2016-06/ome_core/BinFile"/>
        <rdfs:comment xml:lang="en">Property &quot;binFile&quot; specifies the binary file. </rdfs:comment>
        <rdfs:label xml:lang="en">binary file</rdfs:label>
    </owl:ObjectProperty>
    


    <!-- http://www.openmicroscopy.org/rdf/2016-06/ome_core/binning -->

    <owl:ObjectProperty rdf:about="http://www.openmicroscopy.org/rdf/2016-06/ome_core/binning">
        <rdfs:domain rdf:resource="http://www.openmicroscopy.org/rdf/2016-06/ome_core/DetectorSettings"/>
        <rdfs:range rdf:resource="http://www.openmicroscopy.org/rdf/2016-06/ome_core/Binning"/>
        <rdfs:comment xml:lang="en">Property &quot;binning&quot; specifies the binning data that represents the number of pixels combined to form larger pixels.</rdfs:comment>
        <rdfs:label xml:lang="en">binning</rdfs:label>
    </owl:ObjectProperty>
    


    <!-- http://www.openmicroscopy.org/rdf/2016-06/ome_core/channel -->

    <owl:ObjectProperty rdf:about="http://www.openmicroscopy.org/rdf/2016-06/ome_core/channel">
        <rdfs:domain rdf:resource="http://www.openmicroscopy.org/rdf/2016-06/ome_core/Pixels"/>
        <rdfs:range rdf:resource="http://www.openmicroscopy.org/rdf/2016-06/ome_core/Channel"/>
        <rdfs:comment xml:lang="en">Property &quot;channel&quot; speficies the channel.</rdfs:comment>
        <rdfs:label xml:lang="en">channel</rdfs:label>
    </owl:ObjectProperty>
    


    <!-- http://www.openmicroscopy.org/rdf/2016-06/ome_core/color -->

    <owl:ObjectProperty rdf:about="http://www.openmicroscopy.org/rdf/2016-06/ome_core/color">
        <rdfs:domain rdf:resource="http://www.openmicroscopy.org/rdf/2016-06/ome_core/Channel"/>
        <rdfs:domain rdf:resource="http://www.openmicroscopy.org/rdf/2016-06/ome_core/Shape"/>
        <rdfs:domain rdf:resource="http://www.openmicroscopy.org/rdf/2016-06/ome_core/Well"/>
        <rdfs:range rdf:resource="http://www.openmicroscopy.org/rdf/2016-06/ome_core/Color"/>
        <rdfs:comment xml:lang="en">Property &quot;color&quot; speficies the color, such as the color used to reder the channel and the marker color used to highlight the well.</rdfs:comment>
        <rdfs:label xml:lang="en">color</rdfs:label>
    </owl:ObjectProperty>
    


    <!-- http://www.openmicroscopy.org/rdf/2016-06/ome_core/columnNamingConvention -->

    <owl:ObjectProperty rdf:about="http://www.openmicroscopy.org/rdf/2016-06/ome_core/columnNamingConvention">
        <rdfs:domain rdf:resource="http://www.openmicroscopy.org/rdf/2016-06/ome_core/Plate"/>
        <rdfs:range rdf:resource="http://www.openmicroscopy.org/rdf/2016-06/ome_core/NamingConvention"/>
        <rdfs:comment xml:lang="en">Property &quot;columnNamingConvention&quot; specifies the naming convention for columns that is a predefined list of values for the well labels.</rdfs:comment>
        <rdfs:label xml:lang="en">column naming convention</rdfs:label>
    </owl:ObjectProperty>
    


    <!-- http://www.openmicroscopy.org/rdf/2016-06/ome_core/compression -->

    <owl:ObjectProperty rdf:about="http://www.openmicroscopy.org/rdf/2016-06/ome_core/compression">
        <rdfs:domain rdf:resource="http://www.openmicroscopy.org/rdf/2016-06/ome_core/BinData"/>
        <rdfs:range rdf:resource="http://www.openmicroscopy.org/rdf/2016-06/ome_core/Compression"/>
        <rdfs:comment xml:lang="en">Property &quot;compression&quot; specifies the compression scheme used to encode the data.</rdfs:comment>
        <rdfs:label xml:lang="en">compression</rdfs:label>
    </owl:ObjectProperty>
    


    <!-- http://www.openmicroscopy.org/rdf/2016-06/ome_core/contrastMethod -->

    <owl:ObjectProperty rdf:about="http://www.openmicroscopy.org/rdf/2016-06/ome_core/contrastMethod">
        <rdfs:domain rdf:resource="http://www.openmicroscopy.org/rdf/2016-06/ome_core/Channel"/>
        <rdfs:range rdf:resource="http://www.openmicroscopy.org/rdf/2016-06/ome_core/ContrastMethod"/>
        <rdfs:comment xml:lang="en">Property &quot;contrastMethod&quot; specifies the technique used to achieve contrast for each channel.</rdfs:comment>
        <rdfs:label xml:lang="en">contrast method</rdfs:label>
    </owl:ObjectProperty>
    


    <!-- http://www.openmicroscopy.org/rdf/2016-06/ome_core/correction -->

    <owl:ObjectProperty rdf:about="http://www.openmicroscopy.org/rdf/2016-06/ome_core/correction">
        <rdfs:domain rdf:resource="http://www.openmicroscopy.org/rdf/2016-06/ome_core/Objective"/>
        <rdfs:range rdf:resource="http://www.openmicroscopy.org/rdf/2016-06/ome_core/Correction"/>
        <rdfs:comment xml:lang="en">Property &quot;correction&quot; specifies the correction applied to the lens.</rdfs:comment>
        <rdfs:label xml:lang="en">correction</rdfs:label>
    </owl:ObjectProperty>
    


    <!-- http://www.openmicroscopy.org/rdf/2016-06/ome_core/cutIn -->

    <owl:ObjectProperty rdf:about="http://www.openmicroscopy.org/rdf/2016-06/ome_core/cutIn">
        <rdfs:domain rdf:resource="http://www.openmicroscopy.org/rdf/2016-06/ome_core/TransmittanceRange"/>
        <rdfs:comment xml:lang="en">Property &quot;cutIn&quot; speficies the wavelength below which there is less than 50% transmittance for a filter.</rdfs:comment>
        <rdfs:label xml:lang="en">cut in</rdfs:label>
    </owl:ObjectProperty>
    


    <!-- http://www.openmicroscopy.org/rdf/2016-06/ome_core/cutInTolerance -->

    <owl:ObjectProperty rdf:about="http://www.openmicroscopy.org/rdf/2016-06/ome_core/cutInTolerance">
        <rdfs:domain rdf:resource="http://www.openmicroscopy.org/rdf/2016-06/ome_core/TransmittanceRange"/>
        <rdfs:comment xml:lang="en">Property &quot;cutInTolerance&quot; speficies the cutIn tolerance.</rdfs:comment>
        <rdfs:label xml:lang="en">cut in tolerance</rdfs:label>
    </owl:ObjectProperty>
    


    <!-- http://www.openmicroscopy.org/rdf/2016-06/ome_core/cutOut -->

    <owl:ObjectProperty rdf:about="http://www.openmicroscopy.org/rdf/2016-06/ome_core/cutOut">
        <rdfs:domain rdf:resource="http://www.openmicroscopy.org/rdf/2016-06/ome_core/TransmittanceRange"/>
        <rdfs:comment xml:lang="en">Property &quot;cutOut&quot; speficies the wavelength above which there is less than 50% transmittance for a filter.</rdfs:comment>
        <rdfs:label xml:lang="en">cut out</rdfs:label>
    </owl:ObjectProperty>
    


    <!-- http://www.openmicroscopy.org/rdf/2016-06/ome_core/cutOutTolerance -->

    <owl:ObjectProperty rdf:about="http://www.openmicroscopy.org/rdf/2016-06/ome_core/cutOutTolerance">
        <rdfs:domain rdf:resource="http://www.openmicroscopy.org/rdf/2016-06/ome_core/TransmittanceRange"/>
        <rdfs:comment xml:lang="en">Property &quot;cutOutTolerance&quot; speficies the cutOut tolerance.</rdfs:comment>
        <rdfs:label xml:lang="en">cut out tolerance</rdfs:label>
    </owl:ObjectProperty>
    


    <!-- http://www.openmicroscopy.org/rdf/2016-06/ome_core/dataset -->

    <owl:ObjectProperty rdf:about="http://www.openmicroscopy.org/rdf/2016-06/ome_core/dataset">
        <rdfs:domain rdf:resource="http://www.openmicroscopy.org/rdf/2016-06/ome_core/Project"/>
        <rdfs:range rdf:resource="http://www.openmicroscopy.org/rdf/2016-06/ome_core/Dataset"/>
        <rdfs:comment xml:lang="en">Property &quot;dataset&quot; specifies a collection of images that are always processed together.</rdfs:comment>
        <rdfs:label xml:lang="en">dataset</rdfs:label>
    </owl:ObjectProperty>
    


    <!-- http://www.openmicroscopy.org/rdf/2016-06/ome_core/deltaT -->

    <owl:ObjectProperty rdf:about="http://www.openmicroscopy.org/rdf/2016-06/ome_core/deltaT">
        <rdfs:domain rdf:resource="http://www.openmicroscopy.org/rdf/2016-06/ome_core/Plane"/>
        <rdfs:comment xml:lang="en">Property &quot;deltaT&quot; specifies time since the beginning of the experiment.</rdfs:comment>
        <rdfs:label xml:lang="en">delta t</rdfs:label>
    </owl:ObjectProperty>
    


    <!-- http://www.openmicroscopy.org/rdf/2016-06/ome_core/dichroic -->

    <owl:ObjectProperty rdf:about="http://www.openmicroscopy.org/rdf/2016-06/ome_core/dichroic">
        <rdfs:domain rdf:resource="http://www.openmicroscopy.org/rdf/2016-06/ome_core/FilterSet"/>
        <rdfs:domain rdf:resource="http://www.openmicroscopy.org/rdf/2016-06/ome_core/LightPath"/>
        <rdfs:range rdf:resource="http://www.openmicroscopy.org/rdf/2016-06/ome_core/Dichroic"/>
        <rdfs:comment xml:lang="en">Property &quot;dichroic&quot; specifies the dichromatic beamsplitter or dichroic mirror used for this filter combination.</rdfs:comment>
        <rdfs:label xml:lang="en">dichroic</rdfs:label>
    </owl:ObjectProperty>
    


    <!-- http://www.openmicroscopy.org/rdf/2016-06/ome_core/dimensionOrder -->

    <owl:ObjectProperty rdf:about="http://www.openmicroscopy.org/rdf/2016-06/ome_core/dimensionOrder">
        <rdfs:domain rdf:resource="http://www.openmicroscopy.org/rdf/2016-06/ome_core/Pixels"/>
        <rdfs:range rdf:resource="http://www.openmicroscopy.org/rdf/2016-06/ome_core/DimensionOrder"/>
        <rdfs:comment xml:lang="en">Property &quot;dimensionOrder&quot; specifies the order in which the individual planes of data are interleaved.</rdfs:comment>
        <rdfs:label xml:lang="en">dimension order</rdfs:label>
    </owl:ObjectProperty>
    


    <!-- http://www.openmicroscopy.org/rdf/2016-06/ome_core/emissionFilter -->

    <owl:ObjectProperty rdf:about="http://www.openmicroscopy.org/rdf/2016-06/ome_core/emissionFilter">
        <rdfs:domain rdf:resource="http://www.openmicroscopy.org/rdf/2016-06/ome_core/FilterSet"/>
        <rdfs:domain rdf:resource="http://www.openmicroscopy.org/rdf/2016-06/ome_core/LightPath"/>
        <rdfs:range rdf:resource="http://www.openmicroscopy.org/rdf/2016-06/ome_core/EmissionFilter"/>
        <rdfs:comment xml:lang="en">Property &quot;emissionFilter&quot; specifies the filters placed in the emission light path.</rdfs:comment>
        <rdfs:label xml:lang="en">emission filter</rdfs:label>
    </owl:ObjectProperty>
    


    <!-- http://www.openmicroscopy.org/rdf/2016-06/ome_core/emissionWavelength -->

    <owl:ObjectProperty rdf:about="http://www.openmicroscopy.org/rdf/2016-06/ome_core/emissionWavelength">
        <rdfs:domain rdf:resource="http://www.openmicroscopy.org/rdf/2016-06/ome_core/Channel"/>
        <rdfs:comment xml:lang="en">Property &quot;emissionWavelength&quot; specifies the wavelength of emission for a particular channel.</rdfs:comment>
        <rdfs:label xml:lang="en">emission wavelength</rdfs:label>
    </owl:ObjectProperty>
    


    <!-- http://www.openmicroscopy.org/rdf/2016-06/ome_core/excitationWavelength -->

    <owl:ObjectProperty rdf:about="http://www.openmicroscopy.org/rdf/2016-06/ome_core/excitationWavelength">
        <rdfs:comment xml:lang="en">Property &quot;excitationWavelength&quot; spefifies the wavelength of excitation for a particular channel.</rdfs:comment>
        <rdfs:label xml:lang="en">excitation wavelength</rdfs:label>
    </owl:ObjectProperty>
    


    <!-- http://www.openmicroscopy.org/rdf/2016-06/ome_core/experiment -->

    <owl:ObjectProperty rdf:about="http://www.openmicroscopy.org/rdf/2016-06/ome_core/experiment">
        <rdfs:domain rdf:resource="http://www.openmicroscopy.org/rdf/2016-06/ome_core/Dataset"/>
        <rdfs:domain rdf:resource="http://www.openmicroscopy.org/rdf/2016-06/ome_core/ExperimenterGroup"/>
        <rdfs:domain rdf:resource="http://www.openmicroscopy.org/rdf/2016-06/ome_core/Image"/>
        <rdfs:range rdf:resource="http://www.openmicroscopy.org/rdf/2016-06/ome_core/Experiment"/>
        <rdfs:comment xml:lang="en">Property &quot;experiment&quot; specifies the experiment.</rdfs:comment>
        <rdfs:label xml:lang="en">experiment</rdfs:label>
    </owl:ObjectProperty>
    


    <!-- http://www.openmicroscopy.org/rdf/2016-06/ome_core/experimentType -->

    <owl:ObjectProperty rdf:about="http://www.openmicroscopy.org/rdf/2016-06/ome_core/experimentType">
        <rdfs:domain rdf:resource="http://www.openmicroscopy.org/rdf/2016-06/ome_core/Experiment"/>
        <rdfs:range rdf:resource="http://www.openmicroscopy.org/rdf/2016-06/ome_core/ExperimentType"/>
        <rdfs:comment xml:lang="en">Property &quot;experimentType&quot; specifies the type of experiment.</rdfs:comment>
        <rdfs:label xml:lang="en">experiment type</rdfs:label>
    </owl:ObjectProperty>
    


    <!-- http://www.openmicroscopy.org/rdf/2016-06/ome_core/experimenterGroup -->

    <owl:ObjectProperty rdf:about="http://www.openmicroscopy.org/rdf/2016-06/ome_core/experimenterGroup">
        <rdfs:domain rdf:resource="http://www.openmicroscopy.org/rdf/2016-06/ome_core/Dataset"/>
        <rdfs:domain rdf:resource="http://www.openmicroscopy.org/rdf/2016-06/ome_core/Image"/>
        <rdfs:domain rdf:resource="http://www.openmicroscopy.org/rdf/2016-06/ome_core/Project"/>
        <rdfs:range rdf:resource="http://www.openmicroscopy.org/rdf/2016-06/ome_core/ExperimenterGroup"/>
        <rdfs:range rdf:resource="http://xmlns.com/foaf/0.1/Person"/>
        <rdfs:comment xml:lang="en">Property &quot;experimenter&quot; specifies the person performed an imaging experiment.</rdfs:comment>
        <rdfs:comment xml:lang="en">Property &quot;experimenterGroup&quot; specifies the group of experimenters who performed an imaging experiment.</rdfs:comment>
        <rdfs:label xml:lang="en">experimenter</rdfs:label>
        <rdfs:label xml:lang="en">experimenter group</rdfs:label>
    </owl:ObjectProperty>
    


    <!-- http://www.openmicroscopy.org/rdf/2016-06/ome_core/exposureTime -->

    <owl:ObjectProperty rdf:about="http://www.openmicroscopy.org/rdf/2016-06/ome_core/exposureTime">
        <rdfs:domain rdf:resource="http://www.openmicroscopy.org/rdf/2016-06/ome_core/Plane"/>
        <rdfs:comment xml:lang="en">Property &quot;exposureTime&quot; specifies the length of the exposure.</rdfs:comment>
        <rdfs:label xml:lang="en">exposure time</rdfs:label>
    </owl:ObjectProperty>
    


    <!-- http://www.openmicroscopy.org/rdf/2016-06/ome_core/extractionFilter -->

    <owl:ObjectProperty rdf:about="http://www.openmicroscopy.org/rdf/2016-06/ome_core/extractionFilter">
        <rdfs:domain rdf:resource="http://www.openmicroscopy.org/rdf/2016-06/ome_core/FilterSet"/>
        <rdfs:domain rdf:resource="http://www.openmicroscopy.org/rdf/2016-06/ome_core/LightPath"/>
        <rdfs:range rdf:resource="http://www.openmicroscopy.org/rdf/2016-06/ome_core/ExtractionFilter"/>
        <rdfs:comment xml:lang="en">Property &quot;extractionFilter&quot; specifies the filters placed in the extraction light path.</rdfs:comment>
        <rdfs:label xml:lang="en">extraction filter</rdfs:label>
    </owl:ObjectProperty>
    


    <!-- http://www.openmicroscopy.org/rdf/2016-06/ome_core/fillColor -->

    <owl:ObjectProperty rdf:about="http://www.openmicroscopy.org/rdf/2016-06/ome_core/fillColor">
        <rdfs:domain rdf:resource="http://www.openmicroscopy.org/rdf/2016-06/ome_core/Shape"/>
        <rdfs:range rdf:resource="http://www.openmicroscopy.org/rdf/2016-06/ome_core/Color"/>
        <rdfs:comment xml:lang="en">Property &quot;fillColor&quot; specifies the color of the fill.</rdfs:comment>
        <rdfs:label xml:lang="en">fill color</rdfs:label>
    </owl:ObjectProperty>
    


    <!-- http://www.openmicroscopy.org/rdf/2016-06/ome_core/fillRule -->

    <owl:ObjectProperty rdf:about="http://www.openmicroscopy.org/rdf/2016-06/ome_core/fillRule">
        <rdfs:domain rdf:resource="http://www.openmicroscopy.org/rdf/2016-06/ome_core/Shape"/>
        <rdfs:range rdf:resource="http://www.openmicroscopy.org/rdf/2016-06/ome_core/FillRule"/>
        <rdfs:comment xml:lang="en">Property &quot;fillRule&quot; specifies the rule used to decide which parts of the shape to fill.</rdfs:comment>
        <rdfs:label xml:lang="en">fill rule</rdfs:label>
    </owl:ObjectProperty>
    


    <!-- http://www.openmicroscopy.org/rdf/2016-06/ome_core/filterType -->

    <owl:ObjectProperty rdf:about="http://www.openmicroscopy.org/rdf/2016-06/ome_core/filterType">
        <rdfs:domain rdf:resource="http://www.openmicroscopy.org/rdf/2016-06/ome_core/Filter"/>
        <rdfs:range rdf:resource="http://www.openmicroscopy.org/rdf/2016-06/ome_core/FilterType"/>
        <rdfs:comment xml:lang="en">Property &quot;filterType&quot; specifies the type of the filter.</rdfs:comment>
        <rdfs:label xml:lang="en">filer type</rdfs:label>
    </owl:ObjectProperty>
    


    <!-- http://www.openmicroscopy.org/rdf/2016-06/ome_core/folder -->

    <owl:ObjectProperty rdf:about="http://www.openmicroscopy.org/rdf/2016-06/ome_core/folder">
        <rdfs:domain rdf:resource="http://www.openmicroscopy.org/rdf/2016-06/ome_core/Folder"/>
        <rdfs:domain rdf:resource="http://www.openmicroscopy.org/rdf/2016-06/ome_core/Project"/>
        <rdfs:range rdf:resource="http://www.openmicroscopy.org/rdf/2016-06/ome_core/Folder"/>
        <rdfs:comment xml:lang="en">Property &quot;folder&quot; specifies a folder which is a possibly heterogeneous collection of data.</rdfs:comment>
        <rdfs:label xml:lang="en">folder</rdfs:label>
    </owl:ObjectProperty>
    


    <!-- http://www.openmicroscopy.org/rdf/2016-06/ome_core/fontFamily -->

    <owl:ObjectProperty rdf:about="http://www.openmicroscopy.org/rdf/2016-06/ome_core/fontFamily">
        <rdfs:domain rdf:resource="http://www.openmicroscopy.org/rdf/2016-06/ome_core/Font"/>
        <rdfs:domain rdf:resource="http://www.openmicroscopy.org/rdf/2016-06/ome_core/Shape"/>
        <rdfs:range rdf:resource="http://www.openmicroscopy.org/rdf/2016-06/ome_core/Font"/>
        <rdfs:range rdf:resource="http://www.openmicroscopy.org/rdf/2016-06/ome_core/FontFamily"/>
        <rdfs:comment xml:lang="en">Property &quot;fonf&quot; specifies the font used to draw the text.</rdfs:comment>
        <rdfs:comment xml:lang="en">Property &quot;fonfFamily&quot; specifies the font family used to draw the text.</rdfs:comment>
        <rdfs:label xml:lang="en">font</rdfs:label>
        <rdfs:label xml:lang="en">font family</rdfs:label>
    </owl:ObjectProperty>
    


    <!-- http://www.openmicroscopy.org/rdf/2016-06/ome_core/fontSize -->

    <owl:ObjectProperty rdf:about="http://www.openmicroscopy.org/rdf/2016-06/ome_core/fontSize">
        <rdfs:domain rdf:resource="http://www.openmicroscopy.org/rdf/2016-06/ome_core/Font"/>
        <rdfs:comment xml:lang="en">Property &quot;fontSize&quot; specifies the size of the font.</rdfs:comment>
        <rdfs:label xml:lang="en">font size</rdfs:label>
    </owl:ObjectProperty>
    


    <!-- http://www.openmicroscopy.org/rdf/2016-06/ome_core/fontStyle -->

    <owl:ObjectProperty rdf:about="http://www.openmicroscopy.org/rdf/2016-06/ome_core/fontStyle">
        <rdfs:domain rdf:resource="http://www.openmicroscopy.org/rdf/2016-06/ome_core/Font"/>
        <rdfs:range rdf:resource="http://www.openmicroscopy.org/rdf/2016-06/ome_core/FontStyle"/>
        <rdfs:comment xml:lang="en">Property &quot;fontStyle&quot; specifies the style and weight applied to the text.</rdfs:comment>
        <rdfs:label xml:lang="en">font style</rdfs:label>
    </owl:ObjectProperty>
    


    <!-- http://www.openmicroscopy.org/rdf/2016-06/ome_core/illuminationType -->

    <owl:ObjectProperty rdf:about="http://www.openmicroscopy.org/rdf/2016-06/ome_core/illuminationType">
        <rdfs:domain rdf:resource="http://www.openmicroscopy.org/rdf/2016-06/ome_core/Channel"/>
        <rdfs:range rdf:resource="http://www.openmicroscopy.org/rdf/2016-06/ome_core/IlluminationType"/>
        <rdfs:comment xml:lang="en">Property &quot;illuminationType&quot; specifies the method illumination used to capture the channel.</rdfs:comment>
        <rdfs:label xml:lang="en">illumination type</rdfs:label>
    </owl:ObjectProperty>
    


    <!-- http://www.openmicroscopy.org/rdf/2016-06/ome_core/image -->

    <owl:ObjectProperty rdf:about="http://www.openmicroscopy.org/rdf/2016-06/ome_core/image">
        <rdfs:domain rdf:resource="http://www.openmicroscopy.org/rdf/2016-06/ome_core/Dataset"/>
        <rdfs:domain rdf:resource="http://www.openmicroscopy.org/rdf/2016-06/ome_core/Folder"/>
        <rdfs:domain rdf:resource="http://www.openmicroscopy.org/rdf/2016-06/ome_core/WellSample"/>
        <rdfs:range rdf:resource="http://www.openmicroscopy.org/rdf/2016-06/ome_core/Image"/>
        <rdfs:comment xml:lang="en">Property &quot;image&quot; specifies the actual image.</rdfs:comment>
        <rdfs:label xml:lang="en">image</rdfs:label>
    </owl:ObjectProperty>
    


    <!-- http://www.openmicroscopy.org/rdf/2016-06/ome_core/imagingEnvironment -->

    <owl:ObjectProperty rdf:about="http://www.openmicroscopy.org/rdf/2016-06/ome_core/imagingEnvironment">
        <rdfs:domain rdf:resource="http://www.openmicroscopy.org/rdf/2016-06/ome_core/ImagingCondition"/>
        <rdfs:range rdf:resource="http://www.openmicroscopy.org/rdf/2016-06/ome_core/ImagingEnvironment"/>
        <rdfs:comment xml:lang="en">Property &quot;imagingEnvironment&quot; specifies the environment that the biological sample was in during the experiment.</rdfs:comment>
        <rdfs:label xml:lang="en">Imaging Environment</rdfs:label>
    </owl:ObjectProperty>
    


    <!-- http://www.openmicroscopy.org/rdf/2016-06/ome_core/immersion -->

    <owl:ObjectProperty rdf:about="http://www.openmicroscopy.org/rdf/2016-06/ome_core/immersion">
        <rdfs:domain rdf:resource="http://www.openmicroscopy.org/rdf/2016-06/ome_core/Objective"/>
        <rdfs:range rdf:resource="http://www.openmicroscopy.org/rdf/2016-06/ome_core/Immersion"/>
        <rdfs:comment xml:lang="en">Property &quot;immersion&quot; specifies the immersion medium the lens is designed for.</rdfs:comment>
        <rdfs:label xml:lang="en">immersion</rdfs:label>
    </owl:ObjectProperty>
    


    <!-- http://www.openmicroscopy.org/rdf/2016-06/ome_core/laserMedium -->

    <owl:ObjectProperty rdf:about="http://www.openmicroscopy.org/rdf/2016-06/ome_core/laserMedium">
        <rdfs:domain rdf:resource="http://www.openmicroscopy.org/rdf/2016-06/ome_core/Laser"/>
        <rdfs:range rdf:resource="http://www.openmicroscopy.org/rdf/2016-06/ome_core/LaserMedium"/>
        <rdfs:comment xml:lang="en">Property &quot;laserMedium&quot; specifies the Medium attribute specifies the actual lasing medium for a given laser type.</rdfs:comment>
        <rdfs:label xml:lang="en">laser medium</rdfs:label>
    </owl:ObjectProperty>
    


    <!-- http://www.openmicroscopy.org/rdf/2016-06/ome_core/leader -->

    <owl:ObjectProperty rdf:about="http://www.openmicroscopy.org/rdf/2016-06/ome_core/leader">
        <rdfs:domain rdf:resource="http://www.openmicroscopy.org/rdf/2016-06/ome_core/ExperimenterGroup"/>
        <rdfs:range rdf:resource="http://xmlns.com/foaf/0.1/Person"/>
        <rdfs:comment xml:lang="en">Property &quot;leader&quot; specifies an experimenter group leader.</rdfs:comment>
        <rdfs:label xml:lang="en">leader</rdfs:label>
    </owl:ObjectProperty>
    


    <!-- http://www.openmicroscopy.org/rdf/2016-06/ome_core/manufacturer -->

    <owl:ObjectProperty rdf:about="http://www.openmicroscopy.org/rdf/2016-06/ome_core/manufacturer">
        <rdfs:domain rdf:resource="http://www.openmicroscopy.org/rdf/2016-06/ome_core/ManufacturerSpec"/>
        <rdfs:range rdf:resource="http://www.openmicroscopy.org/rdf/2016-06/ome_core/Manufacturer"/>
        <rdfs:comment xml:lang="en">Property &quot;manufacturer&quot; specifies the manufacturer of the component.</rdfs:comment>
        <rdfs:label xml:lang="en">manufacturer</rdfs:label>
    </owl:ObjectProperty>
    


    <!-- http://www.openmicroscopy.org/rdf/2016-06/ome_core/manufacturerSpec -->

    <owl:ObjectProperty rdf:about="http://www.openmicroscopy.org/rdf/2016-06/ome_core/manufacturerSpec">
        <rdfs:range rdf:resource="http://www.openmicroscopy.org/rdf/2016-06/ome_core/ManufacturerSpec"/>
        <rdfs:comment xml:lang="en">Property &quot;manufacturerSpec&quot; specifies the base from which many microscope components are extended.</rdfs:comment>
        <rdfs:label xml:lang="en">manufacturer spec</rdfs:label>
    </owl:ObjectProperty>
    


    <!-- http://www.openmicroscopy.org/rdf/2016-06/ome_core/mapAnnotationValue -->

    <owl:ObjectProperty rdf:about="http://www.openmicroscopy.org/rdf/2016-06/ome_core/mapAnnotationValue">
        <rdfs:domain rdf:resource="http://www.openmicroscopy.org/rdf/2016-06/ome_core/MapAnnotation"/>
        <rdfs:range rdf:resource="http://www.openmicroscopy.org/rdf/2016-06/ome_core/Map"/>
        <rdfs:comment xml:lang="en">Property &quot;mapAnnotationValue&quot; specifies the value of the map annotation that contains of a list of key/value pairs.</rdfs:comment>
        <rdfs:label xml:lang="en">map annotation value</rdfs:label>
    </owl:ObjectProperty>
    


    <!-- http://www.openmicroscopy.org/rdf/2016-06/ome_core/markerEnd -->

    <owl:ObjectProperty rdf:about="http://www.openmicroscopy.org/rdf/2016-06/ome_core/markerEnd">
        <rdfs:domain rdf:resource="http://www.openmicroscopy.org/rdf/2016-06/ome_core/Line"/>
        <rdfs:domain rdf:resource="http://www.openmicroscopy.org/rdf/2016-06/ome_core/Polyline"/>
        <rdfs:domain rdf:resource="http://www.openmicroscopy.org/rdf/2016-06/ome_core/Shape"/>
        <rdfs:range rdf:resource="http://www.openmicroscopy.org/rdf/2016-06/ome_core/Marker"/>
        <rdfs:comment xml:lang="en">Property &quot;markerEnd&quot; specifies the end of the marker.</rdfs:comment>
        <rdfs:label xml:lang="en">maker end</rdfs:label>
    </owl:ObjectProperty>
    


    <!-- http://www.openmicroscopy.org/rdf/2016-06/ome_core/markerStart -->

    <owl:ObjectProperty rdf:about="http://www.openmicroscopy.org/rdf/2016-06/ome_core/markerStart">
        <rdfs:domain rdf:resource="http://www.openmicroscopy.org/rdf/2016-06/ome_core/Line"/>
        <rdfs:domain rdf:resource="http://www.openmicroscopy.org/rdf/2016-06/ome_core/Polyline"/>
        <rdfs:domain rdf:resource="http://www.openmicroscopy.org/rdf/2016-06/ome_core/Shape"/>
        <rdfs:range rdf:resource="http://www.openmicroscopy.org/rdf/2016-06/ome_core/Marker"/>
        <rdfs:comment xml:lang="en">Property &quot;markerStart&quot; specifies the start of the marker.</rdfs:comment>
        <rdfs:label xml:lang="en">marker start</rdfs:label>
    </owl:ObjectProperty>
    


    <!-- http://www.openmicroscopy.org/rdf/2016-06/ome_core/microbeamManipulation -->

    <owl:ObjectProperty rdf:about="http://www.openmicroscopy.org/rdf/2016-06/ome_core/microbeamManipulation">
        <rdfs:domain rdf:resource="http://www.openmicroscopy.org/rdf/2016-06/ome_core/Experiment"/>
        <rdfs:domain rdf:resource="http://www.openmicroscopy.org/rdf/2016-06/ome_core/Image"/>
        <rdfs:domain rdf:resource="http://www.openmicroscopy.org/rdf/2016-06/ome_core/ImagingCondition"/>
        <rdfs:range rdf:resource="http://www.openmicroscopy.org/rdf/2016-06/ome_core/MicrobeamManipuration"/>
        <rdfs:comment xml:lang="en">Property &quot;microbeamManipuration&quot; specifies the microbeam operation that describes a microbeam operation type and the region of the image it was applied to.</rdfs:comment>
        <rdfs:label xml:lang="en">microbeam manipuration</rdfs:label>
    </owl:ObjectProperty>
    


    <!-- http://www.openmicroscopy.org/rdf/2016-06/ome_core/microscope -->

    <owl:ObjectProperty rdf:about="http://www.openmicroscopy.org/rdf/2016-06/ome_core/microscope">
        <rdfs:domain rdf:resource="http://www.openmicroscopy.org/rdf/2016-06/ome_core/Image"/>
        <rdfs:domain rdf:resource="http://www.openmicroscopy.org/rdf/2016-06/ome_core/ImagingCondition"/>
        <rdfs:range rdf:resource="http://www.openmicroscopy.org/rdf/2016-06/ome_core/Microscope"/>
        <rdfs:comment xml:lang="en">Property &quot;microscope&quot; specifies the microscope.</rdfs:comment>
        <rdfs:label xml:lang="en">microscope</rdfs:label>
    </owl:ObjectProperty>
    


    <!-- http://www.openmicroscopy.org/rdf/2016-06/ome_core/mimeType -->

    <owl:ObjectProperty rdf:about="http://www.openmicroscopy.org/rdf/2016-06/ome_core/mimeType">
        <rdfs:domain rdf:resource="http://www.openmicroscopy.org/rdf/2016-06/ome_core/BinFile"/>
        <rdfs:range rdf:resource="http://purl.org/dc/terms/FileFormat"/>
        <rdfs:comment xml:lang="en">Property &quot;mimeType&quot; specifies the MIME type of the binary file.</rdfs:comment>
        <rdfs:label xml:lang="en">MIME type</rdfs:label>
    </owl:ObjectProperty>
    


    <!-- http://www.openmicroscopy.org/rdf/2016-06/ome_core/model -->

    <owl:ObjectProperty rdf:about="http://www.openmicroscopy.org/rdf/2016-06/ome_core/model">
        <rdfs:domain rdf:resource="http://www.openmicroscopy.org/rdf/2016-06/ome_core/ManufacturerSpec"/>
        <rdfs:range rdf:resource="http://www.openmicroscopy.org/rdf/2016-06/ome_core/Model"/>
        <rdfs:comment xml:lang="en">Property &quot;model&quot; specifies the model of the component.</rdfs:comment>
        <rdfs:label xml:lang="en">model</rdfs:label>
    </owl:ObjectProperty>
    


    <!-- http://www.openmicroscopy.org/rdf/2016-06/ome_core/objectiveMedium -->

    <owl:ObjectProperty rdf:about="http://www.openmicroscopy.org/rdf/2016-06/ome_core/objectiveMedium">
        <rdfs:domain rdf:resource="http://www.openmicroscopy.org/rdf/2016-06/ome_core/ObjectiveSettings"/>
        <rdfs:range rdf:resource="http://www.openmicroscopy.org/rdf/2016-06/ome_core/ObjectiveMedium"/>
        <rdfs:comment xml:lang="en">Property &quot;objectvieMedium&quot; specifies a medium used for the lens.</rdfs:comment>
        <rdfs:label xml:lang="en">objective medium</rdfs:label>
    </owl:ObjectProperty>
    


    <!-- http://www.openmicroscopy.org/rdf/2016-06/ome_core/objectiveSettings -->

    <owl:ObjectProperty rdf:about="http://www.openmicroscopy.org/rdf/2016-06/ome_core/objectiveSettings">
        <rdfs:domain rdf:resource="http://www.openmicroscopy.org/rdf/2016-06/ome_core/ImagingCondition"/>
        <rdfs:range rdf:resource="http://www.openmicroscopy.org/rdf/2016-06/ome_core/ObjectiveSettings"/>
        <rdfs:comment xml:lang="en">Property &quot;objectiveSettings&quot; specifies the physical size of a pixel.</rdfs:comment>
        <rdfs:label xml:lang="en">objective settings</rdfs:label>
    </owl:ObjectProperty>
    


    <!-- http://www.openmicroscopy.org/rdf/2016-06/ome_core/physicalSizeX -->

    <owl:ObjectProperty rdf:about="http://www.openmicroscopy.org/rdf/2016-06/ome_core/physicalSizeX">
        <rdfs:domain rdf:resource="http://www.openmicroscopy.org/rdf/2016-06/ome_core/Pixels"/>
        <rdfs:comment xml:lang="en">Property &quot;physicalSizeX&quot; specifies the physical size of a pixel on the x axis.</rdfs:comment>
        <rdfs:label xml:lang="en">physical size x</rdfs:label>
    </owl:ObjectProperty>
    


    <!-- http://www.openmicroscopy.org/rdf/2016-06/ome_core/physicalSizeY -->

    <owl:ObjectProperty rdf:about="http://www.openmicroscopy.org/rdf/2016-06/ome_core/physicalSizeY">
        <rdfs:domain rdf:resource="http://www.openmicroscopy.org/rdf/2016-06/ome_core/Pixels"/>
        <rdfs:comment xml:lang="en">Property &quot;physicalSizeY&quot; specifies the physical size of a pixel on the y axis.</rdfs:comment>
        <rdfs:label xml:lang="en">physical size y</rdfs:label>
    </owl:ObjectProperty>
    


    <!-- http://www.openmicroscopy.org/rdf/2016-06/ome_core/physicalSizeZ -->

    <owl:ObjectProperty rdf:about="http://www.openmicroscopy.org/rdf/2016-06/ome_core/physicalSizeZ">
        <rdfs:domain rdf:resource="http://www.openmicroscopy.org/rdf/2016-06/ome_core/Pixels"/>
        <rdfs:comment xml:lang="en">Property &quot;physicalSizeZ&quot; specifies the physical size of a pixel on the z axis.</rdfs:comment>
        <rdfs:label xml:lang="en">physical size z</rdfs:label>
    </owl:ObjectProperty>
    


    <!-- http://www.openmicroscopy.org/rdf/2016-06/ome_core/pinholeSize -->

    <owl:ObjectProperty rdf:about="http://www.openmicroscopy.org/rdf/2016-06/ome_core/pinholeSize">
        <rdfs:domain rdf:resource="http://www.openmicroscopy.org/rdf/2016-06/ome_core/Channel"/>
        <rdfs:comment xml:lang="en">Property &quot;pinholeSize&quot; specifies the adjustable pin hole diameters for confocal microscopes.</rdfs:comment>
        <rdfs:label xml:lang="en">pinhole size</rdfs:label>
    </owl:ObjectProperty>
    


    <!-- http://www.openmicroscopy.org/rdf/2016-06/ome_core/pixcelType -->

    <owl:ObjectProperty rdf:about="http://www.openmicroscopy.org/rdf/2016-06/ome_core/pixcelType">
        <rdfs:domain rdf:resource="http://www.openmicroscopy.org/rdf/2016-06/ome_core/Pixels"/>
        <rdfs:range rdf:resource="http://www.openmicroscopy.org/rdf/2016-06/ome_core/PixelType"/>
        <rdfs:comment xml:lang="en">Property &quot;pixcelType&quot; specifies the number size/kind used to represent a pixel.</rdfs:comment>
        <rdfs:label xml:lang="en">pixcel type</rdfs:label>
    </owl:ObjectProperty>
    


    <!-- http://www.openmicroscopy.org/rdf/2016-06/ome_core/pixels -->

    <owl:ObjectProperty rdf:about="http://www.openmicroscopy.org/rdf/2016-06/ome_core/pixels">
        <rdfs:domain rdf:resource="http://www.openmicroscopy.org/rdf/2016-06/ome_core/Image"/>
        <rdfs:range rdf:resource="http://www.openmicroscopy.org/rdf/2016-06/ome_core/Pixels"/>
        <rdfs:comment xml:lang="en">Property &quot;pixels&quot; specifies the pixels of the image.</rdfs:comment>
        <rdfs:label xml:lang="en">pixels</rdfs:label>
    </owl:ObjectProperty>
    


    <!-- http://www.openmicroscopy.org/rdf/2016-06/ome_core/plane -->

    <owl:ObjectProperty rdf:about="http://www.openmicroscopy.org/rdf/2016-06/ome_core/plane">
        <rdfs:domain rdf:resource="http://www.openmicroscopy.org/rdf/2016-06/ome_core/Channel"/>
        <rdfs:range rdf:resource="http://www.openmicroscopy.org/rdf/2016-06/ome_core/Plane"/>
        <rdfs:comment xml:lang="en">Property &quot;plane&quot; specifies the microscope stage and image timing data for a given channel/z-section/timepoint.</rdfs:comment>
        <rdfs:label xml:lang="en">plane</rdfs:label>
    </owl:ObjectProperty>
    


    <!-- http://www.openmicroscopy.org/rdf/2016-06/ome_core/plate -->

    <owl:ObjectProperty rdf:about="http://www.openmicroscopy.org/rdf/2016-06/ome_core/plate">
        <rdfs:domain rdf:resource="http://www.openmicroscopy.org/rdf/2016-06/ome_core/Screen"/>
        <rdfs:range rdf:resource="http://www.openmicroscopy.org/rdf/2016-06/ome_core/Plate"/>
        <rdfs:comment xml:lang="en">Property &quot;plate&quot; specifies a microtiter plate within the screen.</rdfs:comment>
        <rdfs:label xml:lang="en">plate</rdfs:label>
    </owl:ObjectProperty>
    


    <!-- http://www.openmicroscopy.org/rdf/2016-06/ome_core/plateAcquisition -->

    <owl:ObjectProperty rdf:about="http://www.openmicroscopy.org/rdf/2016-06/ome_core/plateAcquisition">
        <rdfs:domain rdf:resource="http://www.openmicroscopy.org/rdf/2016-06/ome_core/Plate"/>
        <rdfs:range rdf:resource="http://www.openmicroscopy.org/rdf/2016-06/ome_core/PlateAcquisition"/>
        <rdfs:comment xml:lang="en">Property &quot;plateAcquisition&quot; specifies the plate qcquisition that describes a single acquisition run for a plate.</rdfs:comment>
        <rdfs:label xml:lang="en">plate acquisition</rdfs:label>
    </owl:ObjectProperty>
    


    <!-- http://www.openmicroscopy.org/rdf/2016-06/ome_core/point -->

    <owl:ObjectProperty rdf:about="http://www.openmicroscopy.org/rdf/2016-06/ome_core/point">
        <rdfs:domain rdf:resource="http://www.openmicroscopy.org/rdf/2016-06/ome_core/Polygon"/>
        <rdfs:domain rdf:resource="http://www.openmicroscopy.org/rdf/2016-06/ome_core/Polyline"/>
        <rdfs:range rdf:resource="http://www.openmicroscopy.org/rdf/2016-06/ome_core/Point"/>
        <rdfs:comment xml:lang="en">Property &quot;point&quot; specifies the point.</rdfs:comment>
        <rdfs:label xml:lang="en">point</rdfs:label>
    </owl:ObjectProperty>
    


    <!-- http://www.openmicroscopy.org/rdf/2016-06/ome_core/positionX -->

    <owl:ObjectProperty rdf:about="http://www.openmicroscopy.org/rdf/2016-06/ome_core/positionX">
        <rdfs:domain rdf:resource="http://www.openmicroscopy.org/rdf/2016-06/ome_core/Plane"/>
        <rdfs:domain rdf:resource="http://www.openmicroscopy.org/rdf/2016-06/ome_core/StageLabel"/>
        <rdfs:domain rdf:resource="http://www.openmicroscopy.org/rdf/2016-06/ome_core/WellSample"/>
        <rdfs:comment xml:lang="en">Property &quot;positionX&quot; specifies the x position of the stage.</rdfs:comment>
        <rdfs:label xml:lang="en">position x</rdfs:label>
    </owl:ObjectProperty>
    


    <!-- http://www.openmicroscopy.org/rdf/2016-06/ome_core/positionY -->

    <owl:ObjectProperty rdf:about="http://www.openmicroscopy.org/rdf/2016-06/ome_core/positionY">
        <rdfs:domain rdf:resource="http://www.openmicroscopy.org/rdf/2016-06/ome_core/Plane"/>
        <rdfs:domain rdf:resource="http://www.openmicroscopy.org/rdf/2016-06/ome_core/StageLabel"/>
        <rdfs:domain rdf:resource="http://www.openmicroscopy.org/rdf/2016-06/ome_core/WellSample"/>
        <rdfs:comment xml:lang="en">Property &quot;positionY&quot; specifies the y position of the stage.</rdfs:comment>
        <rdfs:label xml:lang="en">position y</rdfs:label>
    </owl:ObjectProperty>
    


    <!-- http://www.openmicroscopy.org/rdf/2016-06/ome_core/positionZ -->

    <owl:ObjectProperty rdf:about="http://www.openmicroscopy.org/rdf/2016-06/ome_core/positionZ">
        <rdfs:domain rdf:resource="http://www.openmicroscopy.org/rdf/2016-06/ome_core/Plane"/>
        <rdfs:domain rdf:resource="http://www.openmicroscopy.org/rdf/2016-06/ome_core/StageLabel"/>
        <rdfs:comment xml:lang="en">Property &quot;positionX&quot; specifies the z position of the stage.</rdfs:comment>
        <rdfs:label xml:lang="en">position z</rdfs:label>
    </owl:ObjectProperty>
    


    <!-- http://www.openmicroscopy.org/rdf/2016-06/ome_core/power -->

    <owl:ObjectProperty rdf:about="http://www.openmicroscopy.org/rdf/2016-06/ome_core/power">
        <rdfs:domain rdf:resource="http://www.openmicroscopy.org/rdf/2016-06/ome_core/LightSource"/>
        <rdfs:comment xml:lang="en">Property &quot;power&quot; specifies the light-source power.</rdfs:comment>
        <rdfs:label xml:lang="en">power</rdfs:label>
    </owl:ObjectProperty>
    


    <!-- http://www.openmicroscopy.org/rdf/2016-06/ome_core/protocol -->

    <owl:ObjectProperty rdf:about="http://www.openmicroscopy.org/rdf/2016-06/ome_core/protocol">
        <rdfs:domain rdf:resource="http://www.openmicroscopy.org/rdf/2016-06/ome_core/Screen"/>
        <rdfs:comment xml:lang="en">Property &quot;protocol&quot; specifies the protocol such as the screen protocol.</rdfs:comment>
        <rdfs:label xml:lang="en">protocol</rdfs:label>
    </owl:ObjectProperty>
    


    <!-- http://www.openmicroscopy.org/rdf/2016-06/ome_core/pulse -->

    <owl:ObjectProperty rdf:about="http://www.openmicroscopy.org/rdf/2016-06/ome_core/pulse">
        <rdfs:domain rdf:resource="http://www.openmicroscopy.org/rdf/2016-06/ome_core/Laser"/>
        <rdfs:comment xml:lang="en">Property &quot;pulse&quot; specifies the pulse mode of the laser.</rdfs:comment>
        <rdfs:label xml:lang="en">pulse</rdfs:label>
    </owl:ObjectProperty>
    


    <!-- http://www.openmicroscopy.org/rdf/2016-06/ome_core/readOutRate -->

    <owl:ObjectProperty rdf:about="http://www.openmicroscopy.org/rdf/2016-06/ome_core/readOutRate">
        <rdfs:domain rdf:resource="http://www.openmicroscopy.org/rdf/2016-06/ome_core/DetectorSettings"/>
    </owl:ObjectProperty>
    


    <!-- http://www.openmicroscopy.org/rdf/2016-06/ome_core/reagent -->

    <owl:ObjectProperty rdf:about="http://www.openmicroscopy.org/rdf/2016-06/ome_core/reagent">
        <rdfs:domain rdf:resource="http://www.openmicroscopy.org/rdf/2016-06/ome_core/ReagentSet"/>
        <rdfs:domain rdf:resource="http://www.openmicroscopy.org/rdf/2016-06/ome_core/Well"/>
        <rdfs:range rdf:resource="http://www.openmicroscopy.org/rdf/2016-06/ome_core/Reagent"/>
        <rdfs:comment xml:lang="en">Property &quot;reagent&quot; specifies the reagent that describes a chemical or some other physical experimental parameters.</rdfs:comment>
        <rdfs:label xml:lang="en">reagent</rdfs:label>
    </owl:ObjectProperty>
    


    <!-- http://www.openmicroscopy.org/rdf/2016-06/ome_core/reagentSet -->

    <owl:ObjectProperty rdf:about="http://www.openmicroscopy.org/rdf/2016-06/ome_core/reagentSet">
        <rdfs:domain rdf:resource="http://www.openmicroscopy.org/rdf/2016-06/ome_core/Screen"/>
        <rdfs:range rdf:resource="http://www.openmicroscopy.org/rdf/2016-06/ome_core/ReagentSet"/>
        <rdfs:comment xml:lang="en">Property &quot;reagentSet&quot; specifies a set of reagents.</rdfs:comment>
        <rdfs:label xml:lang="en">reagent set</rdfs:label>
    </owl:ObjectProperty>
    


    <!-- http://www.openmicroscopy.org/rdf/2016-06/ome_core/regionOfInterest -->

    <owl:ObjectProperty rdf:about="http://www.openmicroscopy.org/rdf/2016-06/ome_core/regionOfInterest">
        <rdfs:domain rdf:resource="http://www.openmicroscopy.org/rdf/2016-06/ome_core/Folder"/>
        <rdfs:domain rdf:resource="http://www.openmicroscopy.org/rdf/2016-06/ome_core/Image"/>
        <rdfs:domain rdf:resource="http://www.openmicroscopy.org/rdf/2016-06/ome_core/Laser"/>
        <rdfs:range rdf:resource="http://www.openmicroscopy.org/rdf/2016-06/ome_core/RegionOfInterest"/>
        <rdfs:comment xml:lang="en">Property &quot;regionOfInterest&quot; specifies a four dimensional region of interest (ROI).</rdfs:comment>
        <rdfs:label xml:lang="en">region of interest</rdfs:label>
    </owl:ObjectProperty>
    


    <!-- http://www.openmicroscopy.org/rdf/2016-06/ome_core/repetitionRate -->

    <owl:ObjectProperty rdf:about="http://www.openmicroscopy.org/rdf/2016-06/ome_core/repetitionRate">
        <rdfs:comment xml:lang="en">Property &quot;repetitionRate&quot; specifies the rate in Hz at which the laser pulses if the Pulse type is &apos;Repetitive&apos;.</rdfs:comment>
        <rdfs:label xml:lang="en">repeteion rate</rdfs:label>
    </owl:ObjectProperty>
    


    <!-- http://www.openmicroscopy.org/rdf/2016-06/ome_core/rights -->

    <owl:ObjectProperty rdf:about="http://www.openmicroscopy.org/rdf/2016-06/ome_core/rights">
        <rdfs:domain rdf:resource="http://www.openmicroscopy.org/rdf/2016-06/ome_core/Project"/>
        <rdfs:range rdf:resource="http://www.openmicroscopy.org/rdf/2016-06/ome_core/Rights"/>
        <rdfs:comment xml:lang="en">Property &quot;rights&quot; specifies the lights holder and lights held.</rdfs:comment>
        <rdfs:label xml:lang="en">rights</rdfs:label>
    </owl:ObjectProperty>
    


    <!-- http://www.openmicroscopy.org/rdf/2016-06/ome_core/rowNamingConvention -->

    <owl:ObjectProperty rdf:about="http://www.openmicroscopy.org/rdf/2016-06/ome_core/rowNamingConvention">
        <rdfs:domain rdf:resource="http://www.openmicroscopy.org/rdf/2016-06/ome_core/Plate"/>
        <rdfs:range rdf:resource="http://www.openmicroscopy.org/rdf/2016-06/ome_core/NamingConvention"/>
        <rdfs:comment xml:lang="en">Property &quot;columnNamingConvention&quot; specifies the naming convention for rows that is a predefined list of values for the well labels.</rdfs:comment>
        <rdfs:label xml:lang="en">row naming conversion</rdfs:label>
    </owl:ObjectProperty>
    


    <!-- http://www.openmicroscopy.org/rdf/2016-06/ome_core/shape -->

    <owl:ObjectProperty rdf:about="http://www.openmicroscopy.org/rdf/2016-06/ome_core/shape">
        <rdfs:comment xml:lang="en">Property &quot;shape&quot; specifies the shape that contains a single specific ROI shape and links that to any channels, and a timepoint and a z-section.</rdfs:comment>
        <rdfs:label xml:lang="en">shape</rdfs:label>
    </owl:ObjectProperty>
    


    <!-- http://www.openmicroscopy.org/rdf/2016-06/ome_core/size -->

    <owl:ObjectProperty rdf:about="http://www.openmicroscopy.org/rdf/2016-06/ome_core/size">
        <rdfs:domain rdf:resource="http://www.openmicroscopy.org/rdf/2016-06/ome_core/BinFile"/>
        <rdfs:comment xml:lang="en">Property &quot;shape&quot; specifies the size of the uncompressed file.</rdfs:comment>
        <rdfs:label xml:lang="en">size</rdfs:label>
    </owl:ObjectProperty>
    


    <!-- http://www.openmicroscopy.org/rdf/2016-06/ome_core/stageLabel -->

    <owl:ObjectProperty rdf:about="http://www.openmicroscopy.org/rdf/2016-06/ome_core/stageLabel">
        <rdfs:domain rdf:resource="http://www.openmicroscopy.org/rdf/2016-06/ome_core/ImagingCondition"/>
        <rdfs:range rdf:resource="http://www.openmicroscopy.org/rdf/2016-06/ome_core/StageLabel"/>
        <rdfs:comment xml:lang="en">Property &quot;stageLabel&quot; specifies the stage labe which is a name and position for a stage position in the microscope&apos;s reference frame.</rdfs:comment>
        <rdfs:label xml:lang="en">stage label</rdfs:label>
    </owl:ObjectProperty>
    


    <!-- http://www.openmicroscopy.org/rdf/2016-06/ome_core/strokeColor -->

    <owl:ObjectProperty rdf:about="http://www.openmicroscopy.org/rdf/2016-06/ome_core/strokeColor">
        <rdfs:domain rdf:resource="http://www.openmicroscopy.org/rdf/2016-06/ome_core/Shape"/>
        <rdfs:range rdf:resource="http://www.openmicroscopy.org/rdf/2016-06/ome_core/Color"/>
        <rdfs:comment xml:lang="en">Property &quot;strokeColor&quot; specifies the color of stroke.</rdfs:comment>
        <rdfs:label xml:lang="en">stroke color</rdfs:label>
    </owl:ObjectProperty>
    


    <!-- http://www.openmicroscopy.org/rdf/2016-06/ome_core/strokeDashArray -->

    <owl:ObjectProperty rdf:about="http://www.openmicroscopy.org/rdf/2016-06/ome_core/strokeDashArray">
        <rdfs:domain rdf:resource="http://www.openmicroscopy.org/rdf/2016-06/ome_core/Shape"/>
        <rdfs:range rdf:resource="http://www.w3.org/1999/02/22-rdf-syntax-ns#Seq"/>
        <rdfs:comment xml:lang="en">Property &quot;strokeDashArray&quot; specifies the array of stroke dash.</rdfs:comment>
        <rdfs:label xml:lang="en">stroke dash array</rdfs:label>
    </owl:ObjectProperty>
    


    <!-- http://www.openmicroscopy.org/rdf/2016-06/ome_core/strokeWidth -->

    <owl:ObjectProperty rdf:about="http://www.openmicroscopy.org/rdf/2016-06/ome_core/strokeWidth">
        <rdfs:domain rdf:resource="http://www.openmicroscopy.org/rdf/2016-06/ome_core/Shape"/>
        <rdfs:comment xml:lang="en">Property &quot;strokeWidth&quot; specifies the width of the stroke.</rdfs:comment>
        <rdfs:label xml:lang="en">stroke width</rdfs:label>
    </owl:ObjectProperty>
    


    <!-- http://www.openmicroscopy.org/rdf/2016-06/ome_core/tagAnnotation -->

    <owl:ObjectProperty rdf:about="http://www.openmicroscopy.org/rdf/2016-06/ome_core/tagAnnotation">
        <rdfs:range rdf:resource="http://www.openmicroscopy.org/rdf/2016-06/ome_core/TagAnnotation"/>
    </owl:ObjectProperty>
    


    <!-- http://www.openmicroscopy.org/rdf/2016-06/ome_core/temperature -->

    <owl:ObjectProperty rdf:about="http://www.openmicroscopy.org/rdf/2016-06/ome_core/temperature">
        <rdfs:domain rdf:resource="http://www.openmicroscopy.org/rdf/2016-06/ome_core/ImagingEnvironment"/>
        <rdfs:comment xml:lang="en">Property &quot;temperature&quot; specifies the temperature.</rdfs:comment>
        <rdfs:label xml:lang="en">temperature</rdfs:label>
    </owl:ObjectProperty>
    


    <!-- http://www.openmicroscopy.org/rdf/2016-06/ome_core/termAnnotationValue -->

    <owl:ObjectProperty rdf:about="http://www.openmicroscopy.org/rdf/2016-06/ome_core/termAnnotationValue">
        <rdfs:range rdf:resource="http://www.openmicroscopy.org/rdf/2016-06/ome_core/TermAnnotation"/>
    </owl:ObjectProperty>
    


    <!-- http://www.openmicroscopy.org/rdf/2016-06/ome_core/tiffData -->

    <owl:ObjectProperty rdf:about="http://www.openmicroscopy.org/rdf/2016-06/ome_core/tiffData">
        <rdfs:domain rdf:resource="http://www.openmicroscopy.org/rdf/2016-06/ome_core/Pixels"/>
        <rdfs:range rdf:resource="http://www.openmicroscopy.org/rdf/2016-06/ome_core/TiffData"/>
        <rdfs:comment xml:lang="en">Property &quot;tiffData&quot; specifies the pixel data in a tiff file.</rdfs:comment>
        <rdfs:label xml:lang="en">tiffData</rdfs:label>
    </owl:ObjectProperty>
    


    <!-- http://www.openmicroscopy.org/rdf/2016-06/ome_core/timeIncrement -->

    <owl:ObjectProperty rdf:about="http://www.openmicroscopy.org/rdf/2016-06/ome_core/timeIncrement">
        <rdfs:domain rdf:resource="http://www.openmicroscopy.org/rdf/2016-06/ome_core/Pixels"/>
        <rdfs:comment xml:lang="en">Property &quot;timeIncrement&quot; specifies the timeinclement that is used for time series that have a global timing specification instead of per-timepoint timing information.</rdfs:comment>
        <rdfs:label xml:lang="en">time increment</rdfs:label>
    </owl:ObjectProperty>
    


    <!-- http://www.openmicroscopy.org/rdf/2016-06/ome_core/transform -->

    <owl:ObjectProperty rdf:about="http://www.openmicroscopy.org/rdf/2016-06/ome_core/transform">
        <rdfs:domain rdf:resource="http://www.openmicroscopy.org/rdf/2016-06/ome_core/Shape"/>
        <rdfs:range rdf:resource="http://www.openmicroscopy.org/rdf/2016-06/ome_core/Transform"/>
        <rdfs:comment xml:lang="en">Property &quot;transform&quot; specifies a matrix used to transform the shape.</rdfs:comment>
        <rdfs:label xml:lang="en">transform</rdfs:label>
    </owl:ObjectProperty>
    


    <!-- http://www.openmicroscopy.org/rdf/2016-06/ome_core/transmittanceRange -->

    <owl:ObjectProperty rdf:about="http://www.openmicroscopy.org/rdf/2016-06/ome_core/transmittanceRange">
        <rdfs:domain rdf:resource="http://www.openmicroscopy.org/rdf/2016-06/ome_core/Filter"/>
        <rdfs:range rdf:resource="http://www.openmicroscopy.org/rdf/2016-06/ome_core/TransmittanceRange"/>
        <rdfs:comment xml:lang="en">Property &quot;transmittanceRange&quot; specifies the transmittance range that describes wavelengths that are transmitted by the filter.</rdfs:comment>
        <rdfs:label xml:lang="en">transmittance range</rdfs:label>
    </owl:ObjectProperty>
    


    <!-- http://www.openmicroscopy.org/rdf/2016-06/ome_core/union -->

    <owl:ObjectProperty rdf:about="http://www.openmicroscopy.org/rdf/2016-06/ome_core/union">
        <rdfs:domain rdf:resource="http://www.openmicroscopy.org/rdf/2016-06/ome_core/RegionOfInterest"/>
        <rdfs:range rdf:resource="http://www.w3.org/1999/02/22-rdf-syntax-ns#Bag"/>
        <rdfs:comment xml:lang="en">Property &quot;union&quot; specifies the union of sets.</rdfs:comment>
        <rdfs:label xml:lang="en">union</rdfs:label>
    </owl:ObjectProperty>
    


    <!-- http://www.openmicroscopy.org/rdf/2016-06/ome_core/voltage -->

    <owl:ObjectProperty rdf:about="http://www.openmicroscopy.org/rdf/2016-06/ome_core/voltage">
        <rdfs:domain rdf:resource="http://www.openmicroscopy.org/rdf/2016-06/ome_core/Detector"/>
        <rdfs:domain rdf:resource="http://www.openmicroscopy.org/rdf/2016-06/ome_core/DetectorSettings"/>
        <rdfs:comment xml:lang="en">Property &quot;voltage&quot; specifies the voltage of the detector.</rdfs:comment>
        <rdfs:label xml:lang="en">voltage</rdfs:label>
    </owl:ObjectProperty>
    


    <!-- http://www.openmicroscopy.org/rdf/2016-06/ome_core/waveLength -->

    <owl:ObjectProperty rdf:about="http://www.openmicroscopy.org/rdf/2016-06/ome_core/waveLength">
        <rdfs:domain rdf:resource="http://www.openmicroscopy.org/rdf/2016-06/ome_core/Laser"/>
        <rdfs:domain rdf:resource="http://www.openmicroscopy.org/rdf/2016-06/ome_core/LightSourceSettings"/>
        <rdfs:comment xml:lang="en">Property &quot;waveLength&quot; specifies the wave length of the laser.</rdfs:comment>
        <rdfs:label xml:lang="en">wave length</rdfs:label>
    </owl:ObjectProperty>
    


    <!-- http://www.openmicroscopy.org/rdf/2016-06/ome_core/well -->

    <owl:ObjectProperty rdf:about="http://www.openmicroscopy.org/rdf/2016-06/ome_core/well">
        <rdfs:domain rdf:resource="http://www.openmicroscopy.org/rdf/2016-06/ome_core/Plate"/>
        <rdfs:range rdf:resource="http://www.openmicroscopy.org/rdf/2016-06/ome_core/Well"/>
        <rdfs:comment xml:lang="en">Property &quot;well&quot; specifies the well which is a component of the well/plate/screen construct to describe screening applications.</rdfs:comment>
        <rdfs:label xml:lang="en">well</rdfs:label>
    </owl:ObjectProperty>
    


    <!-- http://www.openmicroscopy.org/rdf/2016-06/ome_core/wellOriginX -->

    <owl:ObjectProperty rdf:about="http://www.openmicroscopy.org/rdf/2016-06/ome_core/wellOriginX">
        <rdfs:domain rdf:resource="http://www.openmicroscopy.org/rdf/2016-06/ome_core/Plate"/>
        <rdfs:common xml:lang="en">Property &quot;wellOriginX&quot; specifies the x position to use for the origin of the fields (individual images) taken in a well.</rdfs:common>
        <rdfs:label xml:lang="en">well origin x</rdfs:label>
    </owl:ObjectProperty>
    


    <!-- http://www.openmicroscopy.org/rdf/2016-06/ome_core/wellOriginY -->

    <owl:ObjectProperty rdf:about="http://www.openmicroscopy.org/rdf/2016-06/ome_core/wellOriginY">
        <rdfs:domain rdf:resource="http://www.openmicroscopy.org/rdf/2016-06/ome_core/Plate"/>
        <rdfs:common xml:lang="en">Property &quot;wellOriginX&quot; specifies the y position to use for the origin of the fields (individual images) taken in a well.</rdfs:common>
        <rdfs:label xml:lang="en">well origin y</rdfs:label>
    </owl:ObjectProperty>
    


    <!-- http://www.openmicroscopy.org/rdf/2016-06/ome_core/wellSample -->

    <owl:ObjectProperty rdf:about="http://www.openmicroscopy.org/rdf/2016-06/ome_core/wellSample">
        <rdfs:domain rdf:resource="http://www.openmicroscopy.org/rdf/2016-06/ome_core/PlateAcquisition"/>
        <rdfs:domain rdf:resource="http://www.openmicroscopy.org/rdf/2016-06/ome_core/Well"/>
        <rdfs:range rdf:resource="http://www.openmicroscopy.org/rdf/2016-06/ome_core/WellSample"/>
        <rdfs:common xml:lang="en">Property &quot;wellSample&quot; specifies the well sample which is an individual image that has been captured within the well.</rdfs:common>
        <rdfs:label xml:lang="en">well sample</rdfs:label>
    </owl:ObjectProperty>
    


    <!-- http://www.openmicroscopy.org/rdf/2016-06/ome_core/workingDistance -->

    <owl:ObjectProperty rdf:about="http://www.openmicroscopy.org/rdf/2016-06/ome_core/workingDistance">
        <rdfs:domain rdf:resource="http://www.openmicroscopy.org/rdf/2016-06/ome_core/Objective"/>
        <rdfs:common xml:lang="en">Property &quot;workingDistance&quot; specifies the working distance of the lens.</rdfs:common>
        <rdfs:label xml:lang="en">working distance</rdfs:label>
    </owl:ObjectProperty>
    


    <!-- http://www.w3.org/1999/02/22-rdf-syntax-ns#li -->

    <owl:ObjectProperty rdf:about="http://www.w3.org/1999/02/22-rdf-syntax-ns#li">
        <rdfs:domain rdf:resource="http://www.w3.org/1999/02/22-rdf-syntax-ns#Bag"/>
        <rdfs:range rdf:resource="http://www.openmicroscopy.org/rdf/2016-06/ome_core/Shape"/>
        <rdfs:comment xml:lang="en">Property &quot;li&quot; specifies an element of the Bag.</rdfs:comment>
        <rdfs:label xml:lang="en">li</rdfs:label>
    </owl:ObjectProperty>
    


    <!-- http://xmlns.com/foaf/0.1/depicts -->

    <owl:ObjectProperty rdf:about="http://xmlns.com/foaf/0.1/depicts">
        <rdfs:domain rdf:resource="http://www.openmicroscopy.org/rdf/2016-06/ome_core/Image"/>
        <rdfs:comment xml:lang="en">Property &quot;http://xmlns.com/foaf/0.1/depicts&quot; specifies a relationship between the image and something that the image depicts.</rdfs:comment>
        <rdfs:label xml:lang="en">depicts</rdfs:label>
    </owl:ObjectProperty>
    


    <!-- http://xmlns.com/foaf/0.1/thumbnail -->

    <owl:ObjectProperty rdf:about="http://xmlns.com/foaf/0.1/thumbnail">
        <rdfs:domain rdf:resource="http://www.openmicroscopy.org/rdf/2016-06/ome_core/Image"/>
        <rdfs:range rdf:resource="http://www.openmicroscopy.org/rdf/2016-06/ome_core/ImageFile"/>
        <rdfs:comment xml:lang="en">Property &quot;http://xmlns.com/foaf/0.1/thumnail&quot; specifies  a relationship between a full-size image and a smaller, representative image that has been derrived from it.</rdfs:comment>
        <rdfs:lael xml:lang="en">thumbnail</rdfs:lael>
    </owl:ObjectProperty>
    


    <!-- 
    ///////////////////////////////////////////////////////////////////////////////////////
    //
    // Data properties
    //
    ///////////////////////////////////////////////////////////////////////////////////////
     -->

    


    <!-- http://purl.org/dc/elements/1.1/description -->

    <owl:DatatypeProperty rdf:about="http://purl.org/dc/elements/1.1/description">
        <rdfs:range rdf:resource="http://www.w3.org/2001/XMLSchema#string"/>
        <rdfs:comment xml:lang="en">Description may include but is not limited to: an abstract, a table of contents, a graphical representation, or a free-text account of the resource.</rdfs:comment>
        <rdfs:label xml:lang="en">description</rdfs:label>
    </owl:DatatypeProperty>
    


    <!-- http://purl.org/dc/elements/1.1/identifier -->

    <owl:DatatypeProperty rdf:about="http://purl.org/dc/elements/1.1/identifier">
        <rdfs:range rdf:resource="http://www.w3.org/2001/XMLSchema#string"/>
        <rdfs:comment xml:lang="en">An unambiguous reference to the resource within a given context.</rdfs:comment>
        <rdfs:label xml:lang="en">identifier</rdfs:label>
    </owl:DatatypeProperty>
    


    <!-- http://www.openmicroscopy.org/rdf/2016-06/ome_core/A00 -->

    <owl:DatatypeProperty rdf:about="http://www.openmicroscopy.org/rdf/2016-06/ome_core/A00">
        <rdfs:domain rdf:resource="http://www.openmicroscopy.org/rdf/2016-06/ome_core/Transform"/>
        <rdfs:range rdf:resource="http://www.w3.org/2001/XMLSchema#float"/>
        <rdfs:comment xml:lang="en">Property &quot;A00&quot; specifies the element (0,0) of matrix used to transform the shape.</rdfs:comment>
        <rdfs:label xml:lang="en">A00</rdfs:label>
    </owl:DatatypeProperty>
    


    <!-- http://www.openmicroscopy.org/rdf/2016-06/ome_core/A01 -->

    <owl:DatatypeProperty rdf:about="http://www.openmicroscopy.org/rdf/2016-06/ome_core/A01">
        <rdfs:domain rdf:resource="http://www.openmicroscopy.org/rdf/2016-06/ome_core/Transform"/>
        <rdfs:range rdf:resource="http://www.w3.org/2001/XMLSchema#float"/>
        <rdfs:comment xml:lang="en">Property &quot;A01&quot; specifies the element (0,1) of matrix used to transform the shape.</rdfs:comment>
        <rdfs:label xml:lang="en">A01</rdfs:label>
    </owl:DatatypeProperty>
    


    <!-- http://www.openmicroscopy.org/rdf/2016-06/ome_core/A02 -->

    <owl:DatatypeProperty rdf:about="http://www.openmicroscopy.org/rdf/2016-06/ome_core/A02">
        <rdfs:domain rdf:resource="http://www.openmicroscopy.org/rdf/2016-06/ome_core/Transform"/>
        <rdfs:range rdf:resource="http://www.w3.org/2001/XMLSchema#float"/>
        <rdfs:comment xml:lang="en">Property &quot;A02&quot; specifies the element (0,2) of matrix used to transform the shape.</rdfs:comment>
        <rdfs:label xml:lang="en">A02</rdfs:label>
    </owl:DatatypeProperty>
    


    <!-- http://www.openmicroscopy.org/rdf/2016-06/ome_core/A10 -->

    <owl:DatatypeProperty rdf:about="http://www.openmicroscopy.org/rdf/2016-06/ome_core/A10">
        <rdfs:domain rdf:resource="http://www.openmicroscopy.org/rdf/2016-06/ome_core/Transform"/>
        <rdfs:range rdf:resource="http://www.w3.org/2001/XMLSchema#float"/>
        <rdfs:comment xml:lang="en">Property &quot;A10&quot; specifies the element (1,0) of matrix used to transform the shape.</rdfs:comment>
        <rdfs:label xml:lang="en">A10</rdfs:label>
    </owl:DatatypeProperty>
    


    <!-- http://www.openmicroscopy.org/rdf/2016-06/ome_core/A11 -->

    <owl:DatatypeProperty rdf:about="http://www.openmicroscopy.org/rdf/2016-06/ome_core/A11">
        <rdfs:domain rdf:resource="http://www.openmicroscopy.org/rdf/2016-06/ome_core/Transform"/>
        <rdfs:range rdf:resource="http://www.w3.org/2001/XMLSchema#float"/>
        <rdfs:comment xml:lang="en">Property &quot;A11&quot; specifies the element (1,1) of matrix used to transform the shape.</rdfs:comment>
        <rdfs:label xml:lang="en">A11</rdfs:label>
    </owl:DatatypeProperty>
    


    <!-- http://www.openmicroscopy.org/rdf/2016-06/ome_core/A12 -->

    <owl:DatatypeProperty rdf:about="http://www.openmicroscopy.org/rdf/2016-06/ome_core/A12">
        <rdfs:domain rdf:resource="http://www.openmicroscopy.org/rdf/2016-06/ome_core/Transform"/>
        <rdfs:range rdf:resource="http://www.w3.org/2001/XMLSchema#float"/>
        <rdfs:comment xml:lang="en">Property &quot;A12&quot; specifies the element (1,2) of matrix used to transform the shape.</rdfs:comment>
        <rdfs:label xml:lang="en">A12</rdfs:label>
    </owl:DatatypeProperty>
    


    <!-- http://www.openmicroscopy.org/rdf/2016-06/ome_core/CO2Percent -->

    <owl:DatatypeProperty rdf:about="http://www.openmicroscopy.org/rdf/2016-06/ome_core/CO2Percent">
        <rdfs:domain rdf:resource="http://www.openmicroscopy.org/rdf/2016-06/ome_core/ImagingEnvironment"/>
        <rdfs:comment xml:lang="en">Property &quot;CO2Percent&quot; specifies the carbon dioxide concentration around the sample.</rdfs:comment>
        <rdfs:label xml:lang="en">CO2 percent</rdfs:label>
    </owl:DatatypeProperty>
    


    <!-- http://www.openmicroscopy.org/rdf/2016-06/ome_core/NDFilter -->

    <owl:DatatypeProperty rdf:about="http://www.openmicroscopy.org/rdf/2016-06/ome_core/NDFilter">
        <rdfs:domain rdf:resource="http://www.openmicroscopy.org/rdf/2016-06/ome_core/Channel"/>
        <rdfs:range rdf:resource="http://www.w3.org/2001/XMLSchema#float"/>
        <rdfs:comment xml:lang="en">Property &quot;NDFilter&quot; specifies the combined effect of any neutral density filters used.</rdfs:comment>
        <rdfs:label xml:lang="en">ND Filter</rdfs:label>
    </owl:DatatypeProperty>
    


    <!-- http://www.openmicroscopy.org/rdf/2016-06/ome_core/XMLAnnotationValue -->

    <owl:DatatypeProperty rdf:about="http://www.openmicroscopy.org/rdf/2016-06/ome_core/XMLAnnotationValue">
        <rdfs:domain rdf:resource="http://www.openmicroscopy.org/rdf/2016-06/ome_core/XMLAnnotation"/>
        <rdfs:range rdf:resource="http://www.w3.org/1999/02/22-rdf-syntax-ns#XMLLiteral"/>
        <rdfs:comment xml:lang="en">Property &quot;XMLAnnotationValue&quot; specifies a general XML annotation.</rdfs:comment>
        <rdfs:label xml:lang="en">XML annotation value</rdfs:label>
    </owl:DatatypeProperty>
    


    <!-- http://www.openmicroscopy.org/rdf/2016-06/ome_core/acquisitionDate -->

    <owl:DatatypeProperty rdf:about="http://www.openmicroscopy.org/rdf/2016-06/ome_core/acquisitionDate">
        <rdfs:domain rdf:resource="http://www.openmicroscopy.org/rdf/2016-06/ome_core/Image"/>
        <rdfs:range rdf:resource="http://www.w3.org/2001/XMLSchema#dateTime"/>
        <rdfs:comment xml:lang="en">Property &quot;acquisitionDate&quot; specifies the acquisition date of the Image.</rdfs:comment>
        <rdfs:label xml:lang="en">acquisition date</rdfs:label>
    </owl:DatatypeProperty>
    


    <!-- http://www.openmicroscopy.org/rdf/2016-06/ome_core/amplificationGain -->

    <owl:DatatypeProperty rdf:about="http://www.openmicroscopy.org/rdf/2016-06/ome_core/amplificationGain">
        <rdfs:domain rdf:resource="http://www.openmicroscopy.org/rdf/2016-06/ome_core/Detector"/>
        <rdfs:range rdf:resource="http://www.w3.org/2001/XMLSchema#float"/>
        <rdfs:comment xml:lang="en">Property &quot;amplificationGain&quot; specifies the gain applied to the detector signal.</rdfs:comment>
        <rdfs:label xml:lang="en">amplification gain</rdfs:label>
    </owl:DatatypeProperty>
    


    <!-- http://www.openmicroscopy.org/rdf/2016-06/ome_core/attenuation -->

    <owl:DatatypeProperty rdf:about="http://www.openmicroscopy.org/rdf/2016-06/ome_core/attenuation">
        <rdfs:domain rdf:resource="http://www.openmicroscopy.org/rdf/2016-06/ome_core/LightSourceSettings"/>
        <rdfs:range rdf:resource="http://www.w3.org/2001/XMLSchema#float"/>
        <rdfs:comment xml:lang="en">Property &quot;attenuation&quot; specifies the attenuation of the light source.</rdfs:comment>
        <rdfs:label xml:lang="en">attenuation</rdfs:label>
    </owl:DatatypeProperty>
    


    <!-- http://www.openmicroscopy.org/rdf/2016-06/ome_core/bigEndian -->

    <owl:DatatypeProperty rdf:about="http://www.openmicroscopy.org/rdf/2016-06/ome_core/bigEndian">
        <rdfs:domain rdf:resource="http://www.openmicroscopy.org/rdf/2016-06/ome_core/BinData"/>
        <rdfs:domain rdf:resource="http://www.openmicroscopy.org/rdf/2016-06/ome_core/Pixels"/>
        <rdfs:range rdf:resource="http://www.w3.org/2001/XMLSchema#boolean"/>
        <rdfs:comment xml:lang="en">Property &quot;bigEndian&quot; specifies a boolean value. The value is true if the pixels data was written in BigEndian order.</rdfs:comment>
        <rdfs:label xml:lang="en">big endian</rdfs:label>
    </owl:DatatypeProperty>
    


    <!-- http://www.openmicroscopy.org/rdf/2016-06/ome_core/booleanAnnotationValue -->

    <owl:DatatypeProperty rdf:about="http://www.openmicroscopy.org/rdf/2016-06/ome_core/booleanAnnotationValue">
        <rdfs:domain rdf:resource="http://www.openmicroscopy.org/rdf/2016-06/ome_core/BooleanAnnotation"/>
        <rdfs:range rdf:resource="http://www.w3.org/2001/XMLSchema#boolean"/>
        <rdfs:comment xml:lang="en">Property &quot;booleanAnnotationValue&quot; specifies the boolean value of the BooleanAnnotation.</rdfs:comment>
        <rdfs:label xml:lang="en">boolean annotation value</rdfs:label>
    </owl:DatatypeProperty>
    


    <!-- http://www.openmicroscopy.org/rdf/2016-06/ome_core/calibratedMagnification -->

    <owl:DatatypeProperty rdf:about="http://www.openmicroscopy.org/rdf/2016-06/ome_core/calibratedMagnification">
        <rdfs:domain rdf:resource="http://www.openmicroscopy.org/rdf/2016-06/ome_core/Objective"/>
        <rdfs:range rdf:resource="http://www.w3.org/2001/XMLSchema#float"/>
        <rdfs:comment xml:lang="en">Property &quot;calibratedMagnification&quot; specifies the magnification of the lens as measured by a calibration process- i.e. &apos;59.987&apos; for a 60X lens.</rdfs:comment>
        <rdfs:label xml:lang="en">calibrated maginification</rdfs:label>
    </owl:DatatypeProperty>
    


    <!-- http://www.openmicroscopy.org/rdf/2016-06/ome_core/column -->

    <owl:DatatypeProperty rdf:about="http://www.openmicroscopy.org/rdf/2016-06/ome_core/column">
        <rdfs:domain rdf:resource="http://www.openmicroscopy.org/rdf/2016-06/ome_core/Well"/>
        <rdfs:range rdf:resource="http://www.w3.org/2001/XMLSchema#nonNegativeInteger"/>
        <rdfs:comment xml:lang="en">Property &quot;column&quot; specifies the column index of the well, the origin is the top left corner of the plate with the first column of cells being column zero. i.e top left is (0,0). The combination of row, column has to be unique for each well in a plate.</rdfs:comment>
        <rdfs:label xml:lang="en">column</rdfs:label>
    </owl:DatatypeProperty>
    


    <!-- http://www.openmicroscopy.org/rdf/2016-06/ome_core/columns -->

    <owl:DatatypeProperty rdf:about="http://www.openmicroscopy.org/rdf/2016-06/ome_core/columns">
        <rdfs:domain rdf:resource="http://www.openmicroscopy.org/rdf/2016-06/ome_core/Plate"/>
        <rdfs:range rdf:resource="http://www.w3.org/2001/XMLSchema#positiveInteger"/>
        <rdfs:comment xml:lang="en">Property &quot;columns&quot; specifies the number of columns in the plate.</rdfs:comment>
        <rdfs:label xml:lang="en">columns</rdfs:label>
    </owl:DatatypeProperty>
    


    <!-- http://www.openmicroscopy.org/rdf/2016-06/ome_core/commentAnnotationValue -->

    <owl:DatatypeProperty rdf:about="http://www.openmicroscopy.org/rdf/2016-06/ome_core/commentAnnotationValue">
        <rdfs:domain rdf:resource="http://www.openmicroscopy.org/rdf/2016-06/ome_core/CommentAnnotation"/>
        <rdfs:range rdf:resource="http://www.w3.org/2001/XMLSchema#string"/>
        <rdfs:comment xml:lang="en">Property &quot;commentAnnotationValue&quot; specifies a simple comment annotation.</rdfs:comment>
        <rdfs:label xml:lang="en">comment annotation value</rdfs:label>
    </owl:DatatypeProperty>
    


    <!-- http://www.openmicroscopy.org/rdf/2016-06/ome_core/correctionCollar -->

    <owl:DatatypeProperty rdf:about="http://www.openmicroscopy.org/rdf/2016-06/ome_core/correctionCollar">
        <rdfs:domain rdf:resource="http://www.openmicroscopy.org/rdf/2016-06/ome_core/ObjectiveSettings"/>
        <rdfs:range rdf:resource="http://www.w3.org/2001/XMLSchema#float"/>
        <rdfs:comment xml:lang="en">Property &quot;correctionCollar&quot; specifies normally an adjustable ring on the objective. Each has an arbitrary scale on it so the values is unit-less.</rdfs:comment>
        <rdfs:label xml:lang="en">correction collar</rdfs:label>
    </owl:DatatypeProperty>
    


    <!-- http://www.openmicroscopy.org/rdf/2016-06/ome_core/data -->

    <owl:DatatypeProperty rdf:about="http://www.openmicroscopy.org/rdf/2016-06/ome_core/data">
        <rdfs:domain rdf:resource="http://www.openmicroscopy.org/rdf/2016-06/ome_core/BinData"/>
        <rdfs:range rdf:resource="http://www.w3.org/2001/XMLSchema#base64Binary"/>
        <rdfs:comment xml:lang="en">Property &quot;data&quot; specifies a base64 stream.</rdfs:comment>
        <rdfs:label xml:lang="en">data</rdfs:label>
    </owl:DatatypeProperty>
    


    <!-- http://www.openmicroscopy.org/rdf/2016-06/ome_core/doubleAnnotationValue -->

    <owl:DatatypeProperty rdf:about="http://www.openmicroscopy.org/rdf/2016-06/ome_core/doubleAnnotationValue">
        <rdfs:domain rdf:resource="http://www.openmicroscopy.org/rdf/2016-06/ome_core/DoubleAnnotation"/>
        <rdfs:range rdf:resource="http://www.w3.org/2001/XMLSchema#double"/>
        <rdfs:comment xml:lang="en">Property &quot;doubleAnnotationValue&quot; specifies a simple numerical annotation of type xsd:double.</rdfs:comment>
        <rdfs:label xml:lang="en">double annotation value</rdfs:label>
    </owl:DatatypeProperty>
    


    <!-- http://www.openmicroscopy.org/rdf/2016-06/ome_core/endTime -->

    <owl:DatatypeProperty rdf:about="http://www.openmicroscopy.org/rdf/2016-06/ome_core/endTime">
        <rdfs:domain rdf:resource="http://www.openmicroscopy.org/rdf/2016-06/ome_core/PlateAcquisition"/>
        <rdfs:range rdf:resource="http://www.w3.org/2001/XMLSchema#dateTime"/>
        <rdfs:comment xml:lang="en">Property &quot;endTime&quot; specifies the time when the last image of this acquisition was collected.</rdfs:comment>
        <rdfs:label xml:lang="en">end time</rdfs:label>
    </owl:DatatypeProperty>
    


    <!-- http://www.openmicroscopy.org/rdf/2016-06/ome_core/externalDescription -->

    <owl:DatatypeProperty rdf:about="http://www.openmicroscopy.org/rdf/2016-06/ome_core/externalDescription">
        <rdfs:domain rdf:resource="http://www.openmicroscopy.org/rdf/2016-06/ome_core/Well"/>
        <rdfs:comment xml:lang="en">Property &quot;externalDescription&quot; specifies a description of the externally defined identifier for the object.</rdfs:comment>
        <rdfs:label xml:lang="en">external description</rdfs:label>
    </owl:DatatypeProperty>
    


    <!-- http://www.openmicroscopy.org/rdf/2016-06/ome_core/externalIdentifier -->

    <owl:DatatypeProperty rdf:about="http://www.openmicroscopy.org/rdf/2016-06/ome_core/externalIdentifier">
        <rdfs:domain rdf:resource="http://www.openmicroscopy.org/rdf/2016-06/ome_core/Plate"/>
        <rdfs:domain rdf:resource="http://www.openmicroscopy.org/rdf/2016-06/ome_core/Well"/>
        <rdfs:comment xml:lang="en">Property &quot;externalIdentifier&quot; specifies a reference to an external database.</rdfs:comment>
        <rdfs:label xml:lang="en">external identifier</rdfs:label>
    </owl:DatatypeProperty>
    


    <!-- http://www.openmicroscopy.org/rdf/2016-06/ome_core/fieldIndex -->

    <owl:DatatypeProperty rdf:about="http://www.openmicroscopy.org/rdf/2016-06/ome_core/fieldIndex">
        <rdfs:domain rdf:resource="http://www.openmicroscopy.org/rdf/2016-06/ome_core/Plate"/>
        <rdfs:range rdf:resource="http://www.w3.org/2001/XMLSchema#nonNegativeInteger"/>
        <rdfs:comment xml:lang="en">Property &quot;fieldIndex&quot; specifies the index of the WellSample to display as the default Field.</rdfs:comment>
        <rdfs:label xml:lang="en">field index</rdfs:label>
    </owl:DatatypeProperty>
    


    <!-- http://www.openmicroscopy.org/rdf/2016-06/ome_core/filterWheel -->

    <owl:DatatypeProperty rdf:about="http://www.openmicroscopy.org/rdf/2016-06/ome_core/filterWheel">
        <rdfs:domain rdf:resource="http://www.openmicroscopy.org/rdf/2016-06/ome_core/Filter"/>
        <rdfs:range rdf:resource="http://www.w3.org/2001/XMLSchema#string"/>
        <rdfs:comment xml:lang="en">Property &quot;filterWheel&quot; specifies any arrangement of filters in a filter holder of any shape. It could, for example, be a filter slider.</rdfs:comment>
        <rdfs:label xml:lang="en">filter wheel</rdfs:label>
    </owl:DatatypeProperty>
    


    <!-- http://www.openmicroscopy.org/rdf/2016-06/ome_core/firstC -->

    <owl:DatatypeProperty rdf:about="http://www.openmicroscopy.org/rdf/2016-06/ome_core/firstC">
        <rdfs:domain rdf:resource="http://www.openmicroscopy.org/rdf/2016-06/ome_core/TiffData"/>
        <rdfs:range rdf:resource="http://www.w3.org/2001/XMLSchema#nonNegativeInteger"/>
        <rdfs:comment xml:lang="en">Property &quot;firstC&quot; specifies the C position of the image plane at the specified IFD. Indexed from 0. Default is 0 (the first C position).</rdfs:comment>
        <rdfs:label xml:lang="en">first c</rdfs:label>
    </owl:DatatypeProperty>
    


    <!-- http://www.openmicroscopy.org/rdf/2016-06/ome_core/firstT -->

    <owl:DatatypeProperty rdf:about="http://www.openmicroscopy.org/rdf/2016-06/ome_core/firstT">
        <rdfs:domain rdf:resource="http://www.openmicroscopy.org/rdf/2016-06/ome_core/TiffData"/>
        <rdfs:range rdf:resource="http://www.w3.org/2001/XMLSchema#nonNegativeInteger"/>
        <rdfs:comment xml:lang="en">Property &quot;firstT&quot; specifies the T position of the image plane at the specified IFD. Indexed from 0. Default is 0 (the first T position).</rdfs:comment>
        <rdfs:label xml:lang="en">first t</rdfs:label>
    </owl:DatatypeProperty>
    


    <!-- http://www.openmicroscopy.org/rdf/2016-06/ome_core/firstZ -->

    <owl:DatatypeProperty rdf:about="http://www.openmicroscopy.org/rdf/2016-06/ome_core/firstZ">
        <rdfs:domain rdf:resource="http://www.openmicroscopy.org/rdf/2016-06/ome_core/TiffData"/>
        <rdfs:range rdf:resource="http://www.w3.org/2001/XMLSchema#nonNegativeInteger"/>
        <rdfs:comment xml:lang="en">Property &quot;firstZ&quot; specifies the Z position of the image plane at the specified IFD. Indexed from 0. Default is 0 (the first Z position).</rdfs:comment>
        <rdfs:label xml:lang="en">first z</rdfs:label>
    </owl:DatatypeProperty>
    


    <!-- http://www.openmicroscopy.org/rdf/2016-06/ome_core/fluor -->

    <owl:DatatypeProperty rdf:about="http://www.openmicroscopy.org/rdf/2016-06/ome_core/fluor">
        <rdfs:domain rdf:resource="http://www.openmicroscopy.org/rdf/2016-06/ome_core/Channel"/>
        <rdfs:range rdf:resource="http://www.w3.org/2001/XMLSchema#string"/>
        <rdfs:comment xml:lang="en">Property &quot;fluor&quot; specifies a fluorescence image. This is the name of the fluorophore used to produce this channel.</rdfs:comment>
        <rdfs:label xml:lang="en">fluor</rdfs:label>
    </owl:DatatypeProperty>
    


    <!-- http://www.openmicroscopy.org/rdf/2016-06/ome_core/frequencyMultiplication -->

    <owl:DatatypeProperty rdf:about="http://www.openmicroscopy.org/rdf/2016-06/ome_core/frequencyMultiplication">
        <rdfs:domain rdf:resource="http://www.openmicroscopy.org/rdf/2016-06/ome_core/Laser"/>
        <rdfs:range rdf:resource="http://www.w3.org/2001/XMLSchema#positiveInteger"/>
        <rdfs:comment xml:lang="en">Property &quot;frequencyMultiplication&quot; specifies the frequency multiplication of the laser.</rdfs:comment>
        <rdfs:label xml:lang="en">frequency multiplication</rdfs:label>
    </owl:DatatypeProperty>
    


    <!-- http://www.openmicroscopy.org/rdf/2016-06/ome_core/gain -->

    <owl:DatatypeProperty rdf:about="http://www.openmicroscopy.org/rdf/2016-06/ome_core/gain">
        <rdfs:domain rdf:resource="http://www.openmicroscopy.org/rdf/2016-06/ome_core/Detector"/>
        <rdfs:domain rdf:resource="http://www.openmicroscopy.org/rdf/2016-06/ome_core/DetectorSettings"/>
        <rdfs:range rdf:resource="http://www.w3.org/2001/XMLSchema#float"/>
        <rdfs:comment xml:lang="en">Property &quot;gain&quot; specifies the gain of the detector, as a float.</rdfs:comment>
        <rdfs:label xml:lang="en">gain</rdfs:label>
    </owl:DatatypeProperty>
    


    <!-- http://www.openmicroscopy.org/rdf/2016-06/ome_core/hashSHA1 -->

    <owl:DatatypeProperty rdf:about="http://www.openmicroscopy.org/rdf/2016-06/ome_core/hashSHA1">
        <rdfs:domain rdf:resource="http://www.openmicroscopy.org/rdf/2016-06/ome_core/Plane"/>
        <rdfs:range rdf:resource="http://www.w3.org/2001/XMLSchema#hexBinary"/>
        <rdfs:comment xml:lang="en">Property &quot;hashSHA1&quot; specifies the SHA1 hash value.</rdfs:comment>
        <rdfs:label xml:lang="en">hash SHA1</rdfs:label>
    </owl:DatatypeProperty>
    


    <!-- http://www.openmicroscopy.org/rdf/2016-06/ome_core/height -->

    <owl:DatatypeProperty rdf:about="http://www.openmicroscopy.org/rdf/2016-06/ome_core/height">
        <rdfs:domain rdf:resource="http://www.openmicroscopy.org/rdf/2016-06/ome_core/Mask"/>
        <rdfs:domain rdf:resource="http://www.openmicroscopy.org/rdf/2016-06/ome_core/Rectangle"/>
        <rdfs:range rdf:resource="http://www.w3.org/2001/XMLSchema#float"/>
        <rdfs:comment xml:lang="en">Property &quot;height&quot; specifies the height of the object.</rdfs:comment>
        <rdfs:label xml:lang="en">height</rdfs:label>
    </owl:DatatypeProperty>
    


    <!-- http://www.openmicroscopy.org/rdf/2016-06/ome_core/humidity -->

    <owl:DatatypeProperty rdf:about="http://www.openmicroscopy.org/rdf/2016-06/ome_core/humidity">
        <rdfs:domain rdf:resource="http://www.openmicroscopy.org/rdf/2016-06/ome_core/ImagingEnvironment"/>
        <rdfs:comment xml:lang="en">Property &quot;humidity&quot; specifies the humidity around the sample.</rdfs:comment>
        <rdfs:label xml:lang="en">humidity</rdfs:label>
    </owl:DatatypeProperty>
    


    <!-- http://www.openmicroscopy.org/rdf/2016-06/ome_core/ifd -->

    <owl:DatatypeProperty rdf:about="http://www.openmicroscopy.org/rdf/2016-06/ome_core/ifd">
        <rdfs:domain rdf:resource="http://www.openmicroscopy.org/rdf/2016-06/ome_core/TiffData"/>
        <rdfs:range rdf:resource="http://www.w3.org/2001/XMLSchema#nonNegativeInteger"/>
        <rdfs:comment xml:lang="en">Property &quot;ifd&quot; specifies the IFD(s) for which this element is applicable. Indexed from 0. Default is 0 (the first IFD).</rdfs:comment>
        <rdfs:label xml:lang="en">ifd</rdfs:label>
    </owl:DatatypeProperty>
    


    <!-- http://www.openmicroscopy.org/rdf/2016-06/ome_core/index -->

    <owl:DatatypeProperty rdf:about="http://www.openmicroscopy.org/rdf/2016-06/ome_core/index">
        <rdfs:domain rdf:resource="http://www.openmicroscopy.org/rdf/2016-06/ome_core/WellSample"/>
        <rdfs:range rdf:resource="http://www.w3.org/2001/XMLSchema#nonNegativeInteger"/>
        <rdfs:comment xml:lang="en">Property &quot;index&quot; specifies the order of the well samples. Each index should be unique for a given plate but they do not have to be sequential, there may be gaps if part of the dataset is missing. In the user interface the displayed value of the index will be calculated modulo the number of PlateAcquisitions for the plate.</rdfs:comment>
        <rdfs:label xml:lang="en">index</rdfs:label>
    </owl:DatatypeProperty>
    


    <!-- http://www.openmicroscopy.org/rdf/2016-06/ome_core/integration -->

    <owl:DatatypeProperty rdf:about="http://www.openmicroscopy.org/rdf/2016-06/ome_core/integration">
        <rdfs:domain rdf:resource="http://www.openmicroscopy.org/rdf/2016-06/ome_core/DetectorSettings"/>
        <rdfs:range rdf:resource="http://www.w3.org/2001/XMLSchema#positiveInteger"/>
        <rdfs:comment xml:lang="en">Property &quot;integration&quot; specifies the number of sequential frames that get averaged, to improve the signal-to-noise ratio.</rdfs:comment>
        <rdfs:label xml:lang="en">integration</rdfs:label>
    </owl:DatatypeProperty>
    


    <!-- http://www.openmicroscopy.org/rdf/2016-06/ome_core/interleaved -->

    <owl:DatatypeProperty rdf:about="http://www.openmicroscopy.org/rdf/2016-06/ome_core/interleaved">
        <rdfs:domain rdf:resource="http://www.openmicroscopy.org/rdf/2016-06/ome_core/Pixels"/>
        <rdfs:range rdf:resource="http://www.w3.org/2001/XMLSchema#boolean"/>
        <rdfs:comment xml:lang="en">Property &quot;interleaved&quot; specifies how the channels are arranged within the data block: true if channels are stored RGBRGBRGB...; false if channels are stored RRR...GGG...BBB...</rdfs:comment>
        <rdfs:label xml:lang="en">interleaved</rdfs:label>
    </owl:DatatypeProperty>
    


    <!-- http://www.openmicroscopy.org/rdf/2016-06/ome_core/iris -->

    <owl:DatatypeProperty rdf:about="http://www.openmicroscopy.org/rdf/2016-06/ome_core/iris">
        <rdfs:domain rdf:resource="http://www.openmicroscopy.org/rdf/2016-06/ome_core/Objective"/>
        <rdfs:range rdf:resource="http://www.w3.org/2001/XMLSchema#boolean"/>
        <rdfs:comment xml:lang="en">Property &quot;iris&quot; specifies the boolean value whether or not the objective was fitted with an iris.</rdfs:comment>
        <rdfs:label xml:lang="en">iris</rdfs:label>
    </owl:DatatypeProperty>
    


    <!-- http://www.openmicroscopy.org/rdf/2016-06/ome_core/key -->

    <owl:DatatypeProperty rdf:about="http://www.openmicroscopy.org/rdf/2016-06/ome_core/key">
        <rdfs:domain rdf:resource="http://www.openmicroscopy.org/rdf/2016-06/ome_core/Map"/>
        <rdfs:range rdf:resource="http://www.w3.org/2001/XMLSchema#string"/>
        <rdfs:comment xml:lang="en">Property &quot;key&quot; specifies the key of the map.</rdfs:comment>
        <rdfs:label xml:lang="en">key</rdfs:label>
    </owl:DatatypeProperty>
    


    <!-- http://www.openmicroscopy.org/rdf/2016-06/ome_core/length -->

    <owl:DatatypeProperty rdf:about="http://www.openmicroscopy.org/rdf/2016-06/ome_core/length">
        <rdfs:domain rdf:resource="http://www.openmicroscopy.org/rdf/2016-06/ome_core/BinData"/>
        <rdfs:range rdf:resource="http://www.w3.org/2001/XMLSchema#long"/>
        <rdfs:comment xml:lang="en">Property &quot;length&quot; specifies the length of the object.</rdfs:comment>
        <rdfs:label xml:lang="en">length</rdfs:label>
    </owl:DatatypeProperty>
    


    <!-- http://www.openmicroscopy.org/rdf/2016-06/ome_core/lensNA -->

    <owl:DatatypeProperty rdf:about="http://www.openmicroscopy.org/rdf/2016-06/ome_core/lensNA">
        <rdfs:domain rdf:resource="http://www.openmicroscopy.org/rdf/2016-06/ome_core/Objective"/>
        <rdfs:range rdf:resource="http://www.w3.org/2001/XMLSchema#float"/>
        <rdfs:comment xml:lang="en">Property &quot;lensNA&quot; specifies the numerical aperture of the lens expressed as a floating point (real) number. Expected range 0.02 - 1.5. </rdfs:comment>
        <rdfs:label xml:lang="en">lens NA</rdfs:label>
    </owl:DatatypeProperty>
    


    <!-- http://www.openmicroscopy.org/rdf/2016-06/ome_core/locked -->

    <owl:DatatypeProperty rdf:about="http://www.openmicroscopy.org/rdf/2016-06/ome_core/locked">
        <rdfs:domain rdf:resource="http://www.openmicroscopy.org/rdf/2016-06/ome_core/Shape"/>
        <rdfs:range rdf:resource="http://www.w3.org/2001/XMLSchema#boolean"/>
        <rdfs:comment xml:lang="en">Property &quot;locked&quot; specifies the controls whether the shape is locked and read only, true is locked, false is editable.</rdfs:comment>
        <rdfs:label xml:lang="en">locked</rdfs:label>
    </owl:DatatypeProperty>
    


    <!-- http://www.openmicroscopy.org/rdf/2016-06/ome_core/longAnnotationValue -->

    <owl:DatatypeProperty rdf:about="http://www.openmicroscopy.org/rdf/2016-06/ome_core/longAnnotationValue">
        <rdfs:domain rdf:resource="http://www.openmicroscopy.org/rdf/2016-06/ome_core/LongAnnotation"/>
        <rdfs:range rdf:resource="http://www.w3.org/2001/XMLSchema#long"/>
        <rdfs:comment xml:lang="en">Property &quot;longAnnotationValue&quot; specifies a simple numerical annotation of type xsd:long.</rdfs:comment>
        <rdfs:label xml:lang="en">long annotation value</rdfs:label>
    </owl:DatatypeProperty>
    


    <!-- http://www.openmicroscopy.org/rdf/2016-06/ome_core/lotNumber -->

    <owl:DatatypeProperty rdf:about="http://www.openmicroscopy.org/rdf/2016-06/ome_core/lotNumber">
        <rdfs:domain rdf:resource="http://www.openmicroscopy.org/rdf/2016-06/ome_core/ManufacturerSpec"/>
        <rdfs:range rdf:resource="http://www.w3.org/2001/XMLSchema#string"/>
        <rdfs:comment xml:lang="en">Property &quot;lotNumber&quot; specifies the lot number of the component.</rdfs:comment>
        <rdfs:label xml:lang="en">lot number</rdfs:label>
    </owl:DatatypeProperty>
    


    <!-- http://www.openmicroscopy.org/rdf/2016-06/ome_core/maximumFieldCount -->

    <owl:DatatypeProperty rdf:about="http://www.openmicroscopy.org/rdf/2016-06/ome_core/maximumFieldCount">
        <rdfs:domain rdf:resource="http://www.openmicroscopy.org/rdf/2016-06/ome_core/PlateAcquisition"/>
        <rdfs:comment xml:lang="en">Property &quot;maximumFieldCount&quot; specifies the maximum number of fields (well samples) in any well in this PlateAcquisition. This is only used to speed up user interaction by stopping the reading of every well sample.</rdfs:comment>
        <rdfs:label xml:lang="en">maximum field count</rdfs:label>
    </owl:DatatypeProperty>
    


    <!-- http://www.openmicroscopy.org/rdf/2016-06/ome_core/nameSpace -->

    <owl:DatatypeProperty rdf:about="http://www.openmicroscopy.org/rdf/2016-06/ome_core/nameSpace">
        <rdfs:domain rdf:resource="http://www.openmicroscopy.org/rdf/2016-06/ome_core/StructuredAnnotation"/>
        <rdfs:range rdf:resource="http://www.w3.org/2001/XMLSchema#anyURI"/>
        <rdfs:comment xml:lang="en">Property &quot;nameSpace&quot; specifies the namespace for annotation you define. If it is absent then we assume the annotation is to use our (OME&apos;s) default interpretation for this type.</rdfs:comment>
        <rdfs:label xml:lang="en">name space</rdfs:label>
    </owl:DatatypeProperty>
    


    <!-- http://www.openmicroscopy.org/rdf/2016-06/ome_core/nominalMagnification -->

    <owl:DatatypeProperty rdf:about="http://www.openmicroscopy.org/rdf/2016-06/ome_core/nominalMagnification">
        <rdfs:domain rdf:resource="http://www.openmicroscopy.org/rdf/2016-06/ome_core/Objective"/>
        <rdfs:range rdf:resource="http://www.w3.org/2001/XMLSchema#float"/>
        <rdfs:comment xml:lang="en">Property &quot;nominalMagnification&quot; specifies the magnification of the lens as specified by the manufacturer - i.e. &apos;60&apos; is a 60X lens.</rdfs:comment>
        <rdfs:label xml:lang="en">nominal maginification</rdfs:label>
    </owl:DatatypeProperty>
    


    <!-- http://www.openmicroscopy.org/rdf/2016-06/ome_core/offset -->

    <owl:DatatypeProperty rdf:about="http://www.openmicroscopy.org/rdf/2016-06/ome_core/offset">
        <rdfs:domain rdf:resource="http://www.openmicroscopy.org/rdf/2016-06/ome_core/Detector"/>
        <rdfs:domain rdf:resource="http://www.openmicroscopy.org/rdf/2016-06/ome_core/DetectorSettings"/>
        <rdfs:range rdf:resource="http://www.w3.org/2001/XMLSchema#float"/>
        <rdfs:common xml:lang="en">Property &quot;offset&quot; specifies the offset of the detector.</rdfs:common>
        <rdfs:label xml:lang="en">offset</rdfs:label>
    </owl:DatatypeProperty>
    


    <!-- http://www.openmicroscopy.org/rdf/2016-06/ome_core/planeCount -->

    <owl:DatatypeProperty rdf:about="http://www.openmicroscopy.org/rdf/2016-06/ome_core/planeCount">
        <rdfs:domain rdf:resource="http://www.openmicroscopy.org/rdf/2016-06/ome_core/TiffData"/>
        <rdfs:range rdf:resource="http://www.w3.org/2001/XMLSchema#nonNegativeInteger"/>
        <rdfs:comment xml:lang="en">Property &quot;planeCount&quot; specifies the number of IFDs affected. Dimension order of IFDs is given by the enclosing Pixels element&apos;s DimensionOrder attribute. Default is the number of IFDs in the TIFF file, unless an IFD is specified, in which case the default is 1.</rdfs:comment>
        <rdfs:label xml:lang="en">plane count</rdfs:label>
    </owl:DatatypeProperty>
    


    <!-- http://www.openmicroscopy.org/rdf/2016-06/ome_core/pockelCell -->

    <owl:DatatypeProperty rdf:about="http://www.openmicroscopy.org/rdf/2016-06/ome_core/pockelCell">
        <rdfs:domain rdf:resource="http://www.openmicroscopy.org/rdf/2016-06/ome_core/Laser"/>
        <rdfs:range rdf:resource="http://www.w3.org/2001/XMLSchema#boolean"/>
        <rdfs:comment xml:lang="en">Property &quot;pockelCell&quot; specifies the boolean value if true the laser has a PockelCell to rotate the polarization of the beam.</rdfs:comment>
        <rdfs:label xml:lang="en">pockel cell</rdfs:label>
    </owl:DatatypeProperty>
    


    <!-- http://www.openmicroscopy.org/rdf/2016-06/ome_core/pockelCellSettings -->

    <owl:DatatypeProperty rdf:about="http://www.openmicroscopy.org/rdf/2016-06/ome_core/pockelCellSettings">
        <rdfs:domain rdf:resource="http://www.openmicroscopy.org/rdf/2016-06/ome_core/Channel"/>
        <rdfs:range rdf:resource="http://www.w3.org/2001/XMLSchema#integer"/>
        <rdfs:common xml:lang="en">Property &quot;pockelCellSettings&quot; specifies the pockel cell settings for the channel. This is the amount the polarization of the beam is rotated by.</rdfs:common>
        <rdfs:label xml:lang="en">pockel cell settings</rdfs:label>
    </owl:DatatypeProperty>
    


    <!-- http://www.openmicroscopy.org/rdf/2016-06/ome_core/readOutRate -->

    <owl:DatatypeProperty rdf:about="http://www.openmicroscopy.org/rdf/2016-06/ome_core/readOutRate"/>
    


    <!-- http://www.openmicroscopy.org/rdf/2016-06/ome_core/rediusX -->

    <owl:DatatypeProperty rdf:about="http://www.openmicroscopy.org/rdf/2016-06/ome_core/rediusX">
        <rdfs:domain rdf:resource="http://www.openmicroscopy.org/rdf/2016-06/ome_core/Ellipse"/>
        <rdfs:range rdf:resource="http://www.w3.org/2001/XMLSchema#float"/>
        <rdfs:comment xml:lang="en">Property &quot;rediusX&quot; specifies the horizontal radius of the ellipse.</rdfs:comment>
        <rdfs:label xml:lang="en">redius x</rdfs:label>
    </owl:DatatypeProperty>
    


    <!-- http://www.openmicroscopy.org/rdf/2016-06/ome_core/rediusY -->

    <owl:DatatypeProperty rdf:about="http://www.openmicroscopy.org/rdf/2016-06/ome_core/rediusY">
        <rdfs:domain rdf:resource="http://www.openmicroscopy.org/rdf/2016-06/ome_core/Ellipse"/>
        <rdfs:range rdf:resource="http://www.w3.org/2001/XMLSchema#float"/>
        <rdfs:comment xml:lang="en">Property &quot;rediusY&quot; specifies the vertical radius of the ellipse.</rdfs:comment>
        <rdfs:label xml:lang="en">redius y</rdfs:label>
    </owl:DatatypeProperty>
    


    <!-- http://www.openmicroscopy.org/rdf/2016-06/ome_core/refractiveIndex -->

    <owl:DatatypeProperty rdf:about="http://www.openmicroscopy.org/rdf/2016-06/ome_core/refractiveIndex">
        <rdfs:domain rdf:resource="http://www.openmicroscopy.org/rdf/2016-06/ome_core/ObjectiveSettings"/>
        <rdfs:range rdf:resource="http://www.w3.org/2001/XMLSchema#float"/>
        <rdfs:comment xml:lang="en">Property &quot;refractiveIndex&quot; specifies the refractive index of the immersion medium.</rdfs:comment>
        <rdfs:label xml:lang="en">refractive index</rdfs:label>
    </owl:DatatypeProperty>
    


    <!-- http://www.openmicroscopy.org/rdf/2016-06/ome_core/row -->

    <owl:DatatypeProperty rdf:about="http://www.openmicroscopy.org/rdf/2016-06/ome_core/row">
        <rdfs:domain rdf:resource="http://www.openmicroscopy.org/rdf/2016-06/ome_core/Well"/>
        <rdfs:range rdf:resource="http://www.w3.org/2001/XMLSchema#nonNegativeInteger"/>
        <rdfs:comment xml:lang="en">Property &quot;row&quot; specifies  the row index of the well, the origin is the top left corner of the plate with the first row of wells being row zero. i.e top left is (0,0). The combination of Row, Column has to be unique for each well in a plate.</rdfs:comment>
        <rdfs:label xml:lang="en">row</rdfs:label>
    </owl:DatatypeProperty>
    


    <!-- http://www.openmicroscopy.org/rdf/2016-06/ome_core/rows -->

    <owl:DatatypeProperty rdf:about="http://www.openmicroscopy.org/rdf/2016-06/ome_core/rows">
        <rdfs:domain rdf:resource="http://www.openmicroscopy.org/rdf/2016-06/ome_core/Plate"/>
        <rdfs:range rdf:resource="http://www.w3.org/2001/XMLSchema#positiveInteger"/>
        <rdfs:comment xml:lang="en">Property &quot;rows&quot; specifies the number of rows in the plate.</rdfs:comment>
        <rdfs:label xml:lang="en">rows</rdfs:label>
    </owl:DatatypeProperty>
    


    <!-- http://www.openmicroscopy.org/rdf/2016-06/ome_core/samplesPerPixel -->

    <owl:DatatypeProperty rdf:about="http://www.openmicroscopy.org/rdf/2016-06/ome_core/samplesPerPixel">
        <rdfs:domain rdf:resource="http://www.openmicroscopy.org/rdf/2016-06/ome_core/Channel"/>
        <rdfs:range rdf:resource="http://www.w3.org/2001/XMLSchema#positiveInteger"/>
        <rdfs:comment xml:lang="en">Property &quot;samplePerPixel&quot; specifies the number of samples the detector takes to form each pixel value.</rdfs:comment>
        <rdfs:label xml:lang="en">samples per pixel</rdfs:label>
    </owl:DatatypeProperty>
    


    <!-- http://www.openmicroscopy.org/rdf/2016-06/ome_core/screenType -->

    <owl:DatatypeProperty rdf:about="http://www.openmicroscopy.org/rdf/2016-06/ome_core/screenType">
        <rdfs:domain rdf:resource="http://www.openmicroscopy.org/rdf/2016-06/ome_core/Screen"/>
        <rdfs:comment xml:lang="en">Property &quot;screenType&quot; specifies the screen type.</rdfs:comment>
        <rdfs:label xml:lang="en">screen type</rdfs:label>
    </owl:DatatypeProperty>
    


    <!-- http://www.openmicroscopy.org/rdf/2016-06/ome_core/serialNumber -->

    <owl:DatatypeProperty rdf:about="http://www.openmicroscopy.org/rdf/2016-06/ome_core/serialNumber">
        <rdfs:domain rdf:resource="http://www.openmicroscopy.org/rdf/2016-06/ome_core/ManufacturerSpec"/>
        <rdfs:range rdf:resource="http://www.w3.org/2001/XMLSchema#string"/>
        <rdfs:comment xml:lang="en">Property &quot;serialNumber&quot; specifies the serial number of the component.</rdfs:comment>
        <rdfs:label xml:lang="en">serial number</rdfs:label>
    </owl:DatatypeProperty>
    


    <!-- http://www.openmicroscopy.org/rdf/2016-06/ome_core/significantBits -->

    <owl:DatatypeProperty rdf:about="http://www.openmicroscopy.org/rdf/2016-06/ome_core/significantBits">
        <rdfs:domain rdf:resource="http://www.openmicroscopy.org/rdf/2016-06/ome_core/Pixels"/>
        <rdfs:range rdf:resource="http://www.w3.org/2001/XMLSchema#positiveInteger"/>
        <rdfs:comment xml:lang="en">Property &quot;significantBits&quot; specifies the number of bits within the type storing each pixel that are significant, e.g. you can store 12 bit data within a 16 bit type. This does not reduce the storage requirements but can be a useful indicator when processing or viewing the image data.</rdfs:comment>
        <rdfs:label xml:lang="en">significant bits</rdfs:label>
    </owl:DatatypeProperty>
    


    <!-- http://www.openmicroscopy.org/rdf/2016-06/ome_core/sizeC -->

    <owl:DatatypeProperty rdf:about="http://www.openmicroscopy.org/rdf/2016-06/ome_core/sizeC">
        <rdfs:domain rdf:resource="http://www.openmicroscopy.org/rdf/2016-06/ome_core/Pixels"/>
        <rdfs:range rdf:resource="http://www.w3.org/2001/XMLSchema#positiveInteger"/>
        <rdfs:comment xml:lang="en">Property &quot;sizeC&quot; specifies the dimensional size of pixel data array.</rdfs:comment>
        <rdfs:label xml:lang="en">size c</rdfs:label>
    </owl:DatatypeProperty>
    


    <!-- http://www.openmicroscopy.org/rdf/2016-06/ome_core/sizeT -->

    <owl:DatatypeProperty rdf:about="http://www.openmicroscopy.org/rdf/2016-06/ome_core/sizeT">
        <rdfs:domain rdf:resource="http://www.openmicroscopy.org/rdf/2016-06/ome_core/Pixels"/>
        <rdfs:range rdf:resource="http://www.w3.org/2001/XMLSchema#positiveInteger"/>
        <rdfs:comment xml:lang="en">Property &quot;sizeT&quot; specifies the dimensional size of pixel data array.</rdfs:comment>
        <rdfs:label xml:lang="en">size t</rdfs:label>
    </owl:DatatypeProperty>
    


    <!-- http://www.openmicroscopy.org/rdf/2016-06/ome_core/sizeX -->

    <owl:DatatypeProperty rdf:about="http://www.openmicroscopy.org/rdf/2016-06/ome_core/sizeX">
        <rdfs:domain rdf:resource="http://www.openmicroscopy.org/rdf/2016-06/ome_core/Pixels"/>
        <rdfs:range rdf:resource="http://www.w3.org/2001/XMLSchema#positiveInteger"/>
        <rdfs:comment xml:lang="en">Property &quot;sizeX&quot; specifies the dimensional size of pixel data array.</rdfs:comment>
        <rdfs:label xml:lang="en">size x</rdfs:label>
    </owl:DatatypeProperty>
    


    <!-- http://www.openmicroscopy.org/rdf/2016-06/ome_core/sizeY -->

    <owl:DatatypeProperty rdf:about="http://www.openmicroscopy.org/rdf/2016-06/ome_core/sizeY">
        <rdfs:domain rdf:resource="http://www.openmicroscopy.org/rdf/2016-06/ome_core/Pixels"/>
        <rdfs:range rdf:resource="http://www.w3.org/2001/XMLSchema#positiveInteger"/>
        <rdfs:comment xml:lang="en">Property &quot;sizeY&quot; specifies the dimensional size of pixel data array.</rdfs:comment>
        <rdfs:label xml:lang="en">size y</rdfs:label>
    </owl:DatatypeProperty>
    


    <!-- http://www.openmicroscopy.org/rdf/2016-06/ome_core/sizeZ -->

    <owl:DatatypeProperty rdf:about="http://www.openmicroscopy.org/rdf/2016-06/ome_core/sizeZ">
        <rdfs:domain rdf:resource="http://www.openmicroscopy.org/rdf/2016-06/ome_core/Pixels"/>
        <rdfs:range rdf:resource="http://www.w3.org/2001/XMLSchema#positiveInteger"/>
        <rdfs:comment xml:lang="en">Property &quot;sizeZ&quot; specifies the dimensional size of pixel data array.</rdfs:comment>
        <rdfs:label xml:lang="en">size z</rdfs:label>
    </owl:DatatypeProperty>
    


    <!-- http://www.openmicroscopy.org/rdf/2016-06/ome_core/startTime -->

    <owl:DatatypeProperty rdf:about="http://www.openmicroscopy.org/rdf/2016-06/ome_core/startTime">
        <rdfs:domain rdf:resource="http://www.openmicroscopy.org/rdf/2016-06/ome_core/PlateAcquisition"/>
        <rdfs:range rdf:resource="http://www.w3.org/2001/XMLSchema#dateTime"/>
        <rdfs:comment xml:lang="en">Property &quot;startTime&quot; specifies the time when the first image of this acquisition was collected.</rdfs:comment>
        <rdfs:label xml:lang="en">start time</rdfs:label>
    </owl:DatatypeProperty>
    


    <!-- http://www.openmicroscopy.org/rdf/2016-06/ome_core/status -->

    <owl:DatatypeProperty rdf:about="http://www.openmicroscopy.org/rdf/2016-06/ome_core/status">
        <rdfs:domain rdf:resource="http://www.openmicroscopy.org/rdf/2016-06/ome_core/Plate"/>
        <rdfs:range rdf:resource="http://www.w3.org/2001/XMLSchema#string"/>
        <rdfs:comment xml:lang="en">Property &quot;status&quot; specifies the textual annotation of the current state of the plate with respect to the experiment work-flow.</rdfs:comment>
        <rdfs:label xml:lang="en">status</rdfs:label>
    </owl:DatatypeProperty>
    


    <!-- http://www.openmicroscopy.org/rdf/2016-06/ome_core/tagAnnotation -->

    <owl:DatatypeProperty rdf:about="http://www.openmicroscopy.org/rdf/2016-06/ome_core/tagAnnotation"/>
    


    <!-- http://www.openmicroscopy.org/rdf/2016-06/ome_core/termAnnotationValue -->

    <owl:DatatypeProperty rdf:about="http://www.openmicroscopy.org/rdf/2016-06/ome_core/termAnnotationValue"/>
    


    <!-- http://www.openmicroscopy.org/rdf/2016-06/ome_core/text -->

    <owl:DatatypeProperty rdf:about="http://www.openmicroscopy.org/rdf/2016-06/ome_core/text">
        <rdfs:domain rdf:resource="http://www.openmicroscopy.org/rdf/2016-06/ome_core/Shape"/>
        <rdfs:range rdf:resource="http://www.w3.org/2001/XMLSchema#string"/>
        <rdfs:comment xml:lang="en">Property &quot;text&quot; specifies the text.</rdfs:comment>
        <rdfs:label xml:lang="en">text</rdfs:label>
    </owl:DatatypeProperty>
    


    <!-- http://www.openmicroscopy.org/rdf/2016-06/ome_core/theC -->

    <owl:DatatypeProperty rdf:about="http://www.openmicroscopy.org/rdf/2016-06/ome_core/theC">
        <rdfs:domain rdf:resource="http://www.openmicroscopy.org/rdf/2016-06/ome_core/Plane"/>
        <rdfs:domain rdf:resource="http://www.openmicroscopy.org/rdf/2016-06/ome_core/Shape"/>
        <rdfs:range rdf:resource="http://www.w3.org/2001/XMLSchema#nonNegativeInteger"/>
        <rdfs:comment xml:lang="en">Property &quot;theC&quot; specifies the channel this plane is for. This is numbered from 0.</rdfs:comment>
        <rdfs:label xml:lang="en">the c</rdfs:label>
    </owl:DatatypeProperty>
    


    <!-- http://www.openmicroscopy.org/rdf/2016-06/ome_core/theT -->

    <owl:DatatypeProperty rdf:about="http://www.openmicroscopy.org/rdf/2016-06/ome_core/theT">
        <rdfs:domain rdf:resource="http://www.openmicroscopy.org/rdf/2016-06/ome_core/Plane"/>
        <rdfs:domain rdf:resource="http://www.openmicroscopy.org/rdf/2016-06/ome_core/Shape"/>
        <rdfs:range rdf:resource="http://www.w3.org/2001/XMLSchema#nonNegativeInteger"/>
        <rdfs:comment xml:lang="en">Property &quot;theT&quot; specifies the timepoint this plane is for. This is numbered from 0.</rdfs:comment>
        <rdfs:label xml:lang="en">the t</rdfs:label>
    </owl:DatatypeProperty>
    


    <!-- http://www.openmicroscopy.org/rdf/2016-06/ome_core/theZ -->

    <owl:DatatypeProperty rdf:about="http://www.openmicroscopy.org/rdf/2016-06/ome_core/theZ">
        <rdfs:domain rdf:resource="http://www.openmicroscopy.org/rdf/2016-06/ome_core/Plane"/>
        <rdfs:domain rdf:resource="http://www.openmicroscopy.org/rdf/2016-06/ome_core/Shape"/>
        <rdfs:range rdf:resource="http://www.w3.org/2001/XMLSchema#nonNegativeInteger"/>
        <rdfs:comment xml:lang="en">Property &quot;theZ&quot; specifies the Z-section this plane is for. This is numbered from 0.</rdfs:comment>
        <rdfs:label xml:lang="en">the z</rdfs:label>
    </owl:DatatypeProperty>
    


    <!-- http://www.openmicroscopy.org/rdf/2016-06/ome_core/timePoint -->

    <owl:DatatypeProperty rdf:about="http://www.openmicroscopy.org/rdf/2016-06/ome_core/timePoint">
        <rdfs:domain rdf:resource="http://www.openmicroscopy.org/rdf/2016-06/ome_core/WellSample"/>
        <rdfs:range rdf:resource="http://www.w3.org/2001/XMLSchema#dateTime"/>
        <rdfs:comment xml:lang="en">Property &quot;timePoint&quot; specifies the time-point at which the image started to be collected.</rdfs:comment>
        <rdfs:label xml:lang="en">time point</rdfs:label>
    </owl:DatatypeProperty>
    


    <!-- http://www.openmicroscopy.org/rdf/2016-06/ome_core/timestampAnnotationValue -->

    <owl:DatatypeProperty rdf:about="http://www.openmicroscopy.org/rdf/2016-06/ome_core/timestampAnnotationValue">
        <rdfs:domain rdf:resource="http://www.openmicroscopy.org/rdf/2016-06/ome_core/TimestampAnnotation"/>
        <rdfs:range rdf:resource="http://www.w3.org/2001/XMLSchema#dateTime"/>
        <rdfs:comment xml:lang="en">Property &quot;timestampAnnotationValue&quot; specifies the date/time annotation of type xsd:dateTime.</rdfs:comment>
        <rdfs:label xml:lang="en">timestamp annotation value</rdfs:label>
    </owl:DatatypeProperty>
    


    <!-- http://www.openmicroscopy.org/rdf/2016-06/ome_core/transmittance -->

    <owl:DatatypeProperty rdf:about="http://www.openmicroscopy.org/rdf/2016-06/ome_core/transmittance">
        <rdfs:domain rdf:resource="http://www.openmicroscopy.org/rdf/2016-06/ome_core/TransmittanceRange"/>
        <rdfs:range rdf:resource="http://www.w3.org/2001/XMLSchema#float"/>
        <rdfs:comment xml:lang="en">Property &quot;transmittance&quot; specifies the amount of light the filter transmits at a maximum. A fraction, as a value from 0.0 to 1.0.</rdfs:comment>
        <rdfs:label xml:lang="en">transmittance</rdfs:label>
    </owl:DatatypeProperty>
    


    <!-- http://www.openmicroscopy.org/rdf/2016-06/ome_core/tuneable -->

    <owl:DatatypeProperty rdf:about="http://www.openmicroscopy.org/rdf/2016-06/ome_core/tuneable">
        <rdfs:domain rdf:resource="http://www.openmicroscopy.org/rdf/2016-06/ome_core/Laser"/>
        <rdfs:range rdf:resource="http://www.w3.org/2001/XMLSchema#boolean"/>
        <rdfs:comment xml:lang="en">Property &quot;tuneable&quot; specifies whether or not the laser is tuneable.</rdfs:comment>
        <rdfs:label xml:lang="en">tuneable</rdfs:label>
    </owl:DatatypeProperty>
    


    <!-- http://www.openmicroscopy.org/rdf/2016-06/ome_core/uuid -->

    <owl:DatatypeProperty rdf:about="http://www.openmicroscopy.org/rdf/2016-06/ome_core/uuid">
        <rdfs:domain rdf:resource="http://www.openmicroscopy.org/rdf/2016-06/ome_core/TiffData"/>
        <rdfs:range rdf:resource="http://www.w3.org/2001/XMLSchema#anyURI"/>
        <rdfs:comment xml:lang="en">Property &quot;uuid&quot; specifies the unique identifier.</rdfs:comment>
        <rdfs:label xml:lang="en">uuid</rdfs:label>
    </owl:DatatypeProperty>
    


    <!-- http://www.openmicroscopy.org/rdf/2016-06/ome_core/value -->

    <owl:DatatypeProperty rdf:about="http://www.openmicroscopy.org/rdf/2016-06/ome_core/value">
        <rdfs:domain rdf:resource="http://www.openmicroscopy.org/rdf/2016-06/ome_core/Map"/>
        <rdfs:range rdf:resource="http://www.w3.org/2001/XMLSchema#string"/>
        <rdfs:comment xml:lang="en">Property &quot;value&quot; specifies the value of the map.</rdfs:comment>
        <rdfs:label xml:lang="en">value</rdfs:label>
    </owl:DatatypeProperty>
    


    <!-- http://www.openmicroscopy.org/rdf/2016-06/ome_core/wellType -->

    <owl:DatatypeProperty rdf:about="http://www.openmicroscopy.org/rdf/2016-06/ome_core/wellType">
        <rdfs:domain rdf:resource="http://www.openmicroscopy.org/rdf/2016-06/ome_core/Well"/>
        <rdfs:range rdf:resource="http://www.w3.org/2001/XMLSchema#string"/>
        <rdfs:comment xml:lang="en">Property &quot;wellType&quot; specifies the well type for the screening status.</rdfs:comment>
        <rdfs:label xml:lang="en">well type</rdfs:label>
    </owl:DatatypeProperty>
    


    <!-- http://www.openmicroscopy.org/rdf/2016-06/ome_core/width -->

    <owl:DatatypeProperty rdf:about="http://www.openmicroscopy.org/rdf/2016-06/ome_core/width">
        <rdfs:domain rdf:resource="http://www.openmicroscopy.org/rdf/2016-06/ome_core/Mask"/>
        <rdfs:domain rdf:resource="http://www.openmicroscopy.org/rdf/2016-06/ome_core/Rectangle"/>
        <rdfs:range rdf:resource="http://www.w3.org/2001/XMLSchema#float"/>
        <rdfs:comment xml:lang="en">Property &quot;width&quot; specifies the width of the object.</rdfs:comment>
        <rdfs:label xml:lang="en">width</rdfs:label>
    </owl:DatatypeProperty>
    


    <!-- http://www.openmicroscopy.org/rdf/2016-06/ome_core/x -->

    <owl:DatatypeProperty rdf:about="http://www.openmicroscopy.org/rdf/2016-06/ome_core/x">
        <rdfs:domain rdf:resource="http://www.openmicroscopy.org/rdf/2016-06/ome_core/Ellipse"/>
        <rdfs:domain rdf:resource="http://www.openmicroscopy.org/rdf/2016-06/ome_core/Label"/>
        <rdfs:domain rdf:resource="http://www.openmicroscopy.org/rdf/2016-06/ome_core/Mask"/>
        <rdfs:domain rdf:resource="http://www.openmicroscopy.org/rdf/2016-06/ome_core/Point"/>
        <rdfs:domain rdf:resource="http://www.openmicroscopy.org/rdf/2016-06/ome_core/Rectangle"/>
        <rdfs:range rdf:resource="http://www.w3.org/2001/XMLSchema#float"/>
        <rdfs:comment xml:lang="en">Property &quot;x&quot; specifies the x value of the object.</rdfs:comment>
        <rdfs:label xml:lang="en">x</rdfs:label>
    </owl:DatatypeProperty>
    


    <!-- http://www.openmicroscopy.org/rdf/2016-06/ome_core/x1 -->

    <owl:DatatypeProperty rdf:about="http://www.openmicroscopy.org/rdf/2016-06/ome_core/x1">
        <rdfs:domain rdf:resource="http://www.openmicroscopy.org/rdf/2016-06/ome_core/Line"/>
        <rdfs:range rdf:resource="http://www.w3.org/2001/XMLSchema#float"/>
        <rdfs:comment xml:lang="en">Property &quot;x1&quot; specifies the x coordinate of the start of the line.</rdfs:comment>
        <rdfs:label xml:lang="en">x1</rdfs:label>
    </owl:DatatypeProperty>
    


    <!-- http://www.openmicroscopy.org/rdf/2016-06/ome_core/x2 -->

    <owl:DatatypeProperty rdf:about="http://www.openmicroscopy.org/rdf/2016-06/ome_core/x2">
        <rdfs:domain rdf:resource="http://www.openmicroscopy.org/rdf/2016-06/ome_core/Line"/>
        <rdfs:range rdf:resource="http://www.w3.org/2001/XMLSchema#float"/>
        <rdfs:comment xml:lang="en">Property &quot;x2&quot; specifies the x coordinate of the end of the line.</rdfs:comment>
        <rdfs:label xml:lang="en">x2</rdfs:label>
    </owl:DatatypeProperty>
    


    <!-- http://www.openmicroscopy.org/rdf/2016-06/ome_core/y -->

    <owl:DatatypeProperty rdf:about="http://www.openmicroscopy.org/rdf/2016-06/ome_core/y">
        <rdfs:domain rdf:resource="http://www.openmicroscopy.org/rdf/2016-06/ome_core/Ellipse"/>
        <rdfs:domain rdf:resource="http://www.openmicroscopy.org/rdf/2016-06/ome_core/Label"/>
        <rdfs:domain rdf:resource="http://www.openmicroscopy.org/rdf/2016-06/ome_core/Mask"/>
        <rdfs:domain rdf:resource="http://www.openmicroscopy.org/rdf/2016-06/ome_core/Point"/>
        <rdfs:domain rdf:resource="http://www.openmicroscopy.org/rdf/2016-06/ome_core/Rectangle"/>
        <rdfs:range rdf:resource="http://www.w3.org/2001/XMLSchema#float"/>
        <rdfs:comment xml:lang="en">Property &quot;y&quot; specifies the y value of the object.</rdfs:comment>
        <rdfs:comment xml:lang="en">Property &quot;z&quot; specifies the z value of the object.</rdfs:comment>
        <rdfs:label xml:lang="en">y</rdfs:label>
        <rdfs:label xml:lang="en">z</rdfs:label>
    </owl:DatatypeProperty>
    


    <!-- http://www.openmicroscopy.org/rdf/2016-06/ome_core/y1 -->

    <owl:DatatypeProperty rdf:about="http://www.openmicroscopy.org/rdf/2016-06/ome_core/y1">
        <rdfs:domain rdf:resource="http://www.openmicroscopy.org/rdf/2016-06/ome_core/Line"/>
        <rdfs:range rdf:resource="http://www.w3.org/2001/XMLSchema#float"/>
        <rdfs:comment xml:lang="en">Property &quot;y1&quot; specifies the y coordinate of the start of the line.</rdfs:comment>
        <rdfs:label xml:lang="en">y1</rdfs:label>
    </owl:DatatypeProperty>
    


    <!-- http://www.openmicroscopy.org/rdf/2016-06/ome_core/y2 -->

    <owl:DatatypeProperty rdf:about="http://www.openmicroscopy.org/rdf/2016-06/ome_core/y2">
        <rdfs:domain rdf:resource="http://www.openmicroscopy.org/rdf/2016-06/ome_core/Line"/>
        <rdfs:range rdf:resource="http://www.w3.org/2001/XMLSchema#float"/>
        <rdfs:comment xml:lang="en">Property &quot;y2&quot; specifies the y coordinate of the end of the line.</rdfs:comment>
        <rdfs:label xml:lang="en">y2</rdfs:label>
    </owl:DatatypeProperty>
    


    <!-- http://www.openmicroscopy.org/rdf/2016-06/ome_core/zoom -->

    <owl:DatatypeProperty rdf:about="http://www.openmicroscopy.org/rdf/2016-06/ome_core/zoom">
        <rdfs:domain rdf:resource="http://www.openmicroscopy.org/rdf/2016-06/ome_core/Detector"/>
        <rdfs:domain rdf:resource="http://www.openmicroscopy.org/rdf/2016-06/ome_core/DetectorSettings"/>
        <rdfs:range rdf:resource="http://www.w3.org/2001/XMLSchema#float"/>
        <rdfs:comment xml:lang="en">Property &quot;zoom&quot; specifies the fixed Zoom for a detector.</rdfs:comment>
        <rdfs:label xml:lang="en">zoom</rdfs:label>
    </owl:DatatypeProperty>
    


    <!-- http://www.w3.org/1999/02/22-rdf-syntax-ns#value -->

    <owl:DatatypeProperty rdf:about="http://www.w3.org/1999/02/22-rdf-syntax-ns#value">
        <rdfs:comment xml:lang="en">Property &quot;value&quot; specifies the value of the entity.</rdfs:comment>
        <rdfs:label xml:lang="en">value</rdfs:label>
    </owl:DatatypeProperty>
    


    <!-- 
    ///////////////////////////////////////////////////////////////////////////////////////
    //
    // Classes
    //
    ///////////////////////////////////////////////////////////////////////////////////////
     -->

    


    <!-- http://purl.org/dc/terms/FileFormat -->

    <owl:Class rdf:about="http://purl.org/dc/terms/FileFormat">
        <rdfs:label xml:lang="en">File Format</rdfs:label>
    </owl:Class>
    


    <!-- http://www.openmicroscopy.org/rdf/2016-06/ome_core/AcquisitionMode -->

    <owl:Class rdf:about="http://www.openmicroscopy.org/rdf/2016-06/ome_core/AcquisitionMode">
        <rdfs:comment xml:lang="en">Class &quot;AcquisitionMode&quot; is a type of microscopy performed for each channel.</rdfs:comment>
        <rdfs:label xml:lang="en">Acquisition Mode</rdfs:label>
    </owl:Class>
    


    <!-- http://www.openmicroscopy.org/rdf/2016-06/ome_core/AffineTransform -->

    <owl:Class rdf:about="http://www.openmicroscopy.org/rdf/2016-06/ome_core/AffineTransform">
        <rdfs:subClassOf rdf:resource="http://www.openmicroscopy.org/rdf/2016-06/ome_core/Transform"/>
        <rdfs:comment xml:lang="en">Class &quot;AffineTransform&quot; is a matrix used to transform the shape. The element has 6 xsd:float attributes. If the element is present then all 6 values must be included.</rdfs:comment>
        <rdfs:label xml:lang="en">AffineTransform</rdfs:label>
    </owl:Class>
    


    <!-- http://www.openmicroscopy.org/rdf/2016-06/ome_core/Annotation -->

    <owl:Class rdf:about="http://www.openmicroscopy.org/rdf/2016-06/ome_core/Annotation">
        <rdfs:comment xml:lang="en">Class &quot;Annotation&quot; is an annotation from which all others are ultimately derived.</rdfs:comment>
        <rdfs:label xml:lang="en">Annotation</rdfs:label>
    </owl:Class>
    


    <!-- http://www.openmicroscopy.org/rdf/2016-06/ome_core/Arc -->

    <owl:Class rdf:about="http://www.openmicroscopy.org/rdf/2016-06/ome_core/Arc">
        <rdfs:subClassOf rdf:resource="http://www.openmicroscopy.org/rdf/2016-06/ome_core/LightSource"/>
        <rdfs:comment xml:lang="en">Class &quot;Arc&quot; is various kinds of Arc lamps - Hg, Xe, HgXe.</rdfs:comment>
        <rdfs:label xml:lang="en">Arc</rdfs:label>
    </owl:Class>
    


    <!-- http://www.openmicroscopy.org/rdf/2016-06/ome_core/ArcType -->

    <owl:Class rdf:about="http://www.openmicroscopy.org/rdf/2016-06/ome_core/ArcType">
        <rdfs:comment xml:lang="en">Class &quot;ArcType&quot; is types of Arc lamp.</rdfs:comment>
        <rdfs:label xml:lang="en">ArcType</rdfs:label>
    </owl:Class>
    


    <!-- http://www.openmicroscopy.org/rdf/2016-06/ome_core/BinData -->

    <owl:Class rdf:about="http://www.openmicroscopy.org/rdf/2016-06/ome_core/BinData">
        <rdfs:comment xml:lang="en">Class &quot;ArcType&quot; is contents of this element are base64-encoded.</rdfs:comment>
        <rdfs:label xml:lang="en">Binary Data</rdfs:label>
    </owl:Class>
    


    <!-- http://www.openmicroscopy.org/rdf/2016-06/ome_core/BinFile -->

    <owl:Class rdf:about="http://www.openmicroscopy.org/rdf/2016-06/ome_core/BinFile">
        <rdfs:comment xml:lang="en">Class &quot;BinFile&quot; is binary files.</rdfs:comment>
        <rdfs:label xml:lang="en">Binary File</rdfs:label>
    </owl:Class>
    


    <!-- http://www.openmicroscopy.org/rdf/2016-06/ome_core/Binning -->

    <owl:Class rdf:about="http://www.openmicroscopy.org/rdf/2016-06/ome_core/Binning">
        <rdfs:comment xml:lang="en">Class &quot;Binning&quot; is numbers of pixels that are combined to form larger pixels. {used:CCD,EMCCD}.</rdfs:comment>
        <rdfs:label xml:lang="en">Binning</rdfs:label>
    </owl:Class>
    


    <!-- http://www.openmicroscopy.org/rdf/2016-06/ome_core/BooleanAnnotation -->

    <owl:Class rdf:about="http://www.openmicroscopy.org/rdf/2016-06/ome_core/BooleanAnnotation">
        <rdfs:subClassOf rdf:resource="http://www.openmicroscopy.org/rdf/2016-06/ome_core/StructuredAnnotation"/>
        <rdfs:comment xml:lang="en">Class &quot;BooleanAnnotation&quot; is simple boolean annotations of type xsd:boolean.</rdfs:comment>
        <rdfs:label xml:lang="en">Boolean Annotation</rdfs:label>
    </owl:Class>
    


    <!-- http://www.openmicroscopy.org/rdf/2016-06/ome_core/Channel -->

    <owl:Class rdf:about="http://www.openmicroscopy.org/rdf/2016-06/ome_core/Channel">
        <rdfs:comment xml:lang="en">Class &quot;Channel&quot; is channels in the Image, even for a single-plane image.</rdfs:comment>
        <rdfs:label xml:lang="en">Channel</rdfs:label>
    </owl:Class>
    


    <!-- http://www.openmicroscopy.org/rdf/2016-06/ome_core/Color -->

    <owl:Class rdf:about="http://www.openmicroscopy.org/rdf/2016-06/ome_core/Color">
        <rdfs:comment xml:lang="en">Class &quot;Color&quot; is colrs. The value is an integer between -2,147,483,648 and 2,147,483,647 (inclusive). The value is a signed 32 bit encoding of RGBA so &quot;-1&quot; is #FFFFFFFF or solid white.</rdfs:comment>
        <rdfs:label xml:lang="en">Color</rdfs:label>
    </owl:Class>
    


    <!-- http://www.openmicroscopy.org/rdf/2016-06/ome_core/CommentAnnotation -->

    <owl:Class rdf:about="http://www.openmicroscopy.org/rdf/2016-06/ome_core/CommentAnnotation">
        <rdfs:subClassOf rdf:resource="http://www.openmicroscopy.org/rdf/2016-06/ome_core/StructuredAnnotation"/>
        <rdfs:comment xml:lang="en">Class &quot;CommentAnnotation&quot; is simple comment annotations.</rdfs:comment>
        <rdfs:label xml:lang="en">Comment Annotation</rdfs:label>
    </owl:Class>
    


    <!-- http://www.openmicroscopy.org/rdf/2016-06/ome_core/Compression -->

    <owl:Class rdf:about="http://www.openmicroscopy.org/rdf/2016-06/ome_core/Compression">
        <rdfs:comment xml:lang="en">Class &quot;Compression&quot; is compression schemes used to encode the data.</rdfs:comment>
        <rdfs:label xml:lang="en">Compression</rdfs:label>
    </owl:Class>
    


    <!-- http://www.openmicroscopy.org/rdf/2016-06/ome_core/ContrastMethod -->

    <owl:Class rdf:about="http://www.openmicroscopy.org/rdf/2016-06/ome_core/ContrastMethod">
        <rdfs:comment xml:lang="en">Class &quot;ContrastMethod&quot; is the techniques used to achieve contrast for each channel.</rdfs:comment>
        <rdfs:label xml:lang="en">Contrast Method</rdfs:label>
    </owl:Class>
    


    <!-- http://www.openmicroscopy.org/rdf/2016-06/ome_core/Correction -->

    <owl:Class rdf:about="http://www.openmicroscopy.org/rdf/2016-06/ome_core/Correction">
        <rdfs:comment xml:lang="en">Class &quot;Correction&quot; is the collections applied to the lens.</rdfs:comment>
        <rdfs:label xml:lang="en">Correction</rdfs:label>
    </owl:Class>
    


    <!-- http://www.openmicroscopy.org/rdf/2016-06/ome_core/Dataset -->

    <owl:Class rdf:about="http://www.openmicroscopy.org/rdf/2016-06/ome_core/Dataset">
        <rdfs:subClassOf rdf:resource="http://www.w3.org/2002/07/owl#Thing"/>
        <rdfs:comment xml:lang="en">Class &quot;Dataset&quot; is collections of images that are always processed together. Images can belong to more than one Dataset, and a Dataset may contain more than one Image.</rdfs:comment>
        <rdfs:label xml:lang="en">Dataset</rdfs:label>
    </owl:Class>
    


    <!-- http://www.openmicroscopy.org/rdf/2016-06/ome_core/Detector -->

    <owl:Class rdf:about="http://www.openmicroscopy.org/rdf/2016-06/ome_core/Detector">
        <rdfs:comment xml:lang="en">Class &quot;Detector&quot; is types of detectors used to capture the image.</rdfs:comment>
        <rdfs:label xml:lang="en">Detector</rdfs:label>
    </owl:Class>
    


    <!-- http://www.openmicroscopy.org/rdf/2016-06/ome_core/DetectorSettings -->

    <owl:Class rdf:about="http://www.openmicroscopy.org/rdf/2016-06/ome_core/DetectorSettings">
        <rdfs:subClassOf rdf:resource="http://www.openmicroscopy.org/rdf/2016-06/ome_core/Settings"/>
        <rdfs:comment xml:lang="en">Class &quot;DetectorSettings&quot; is settings applied to a detector as well as a reference to the detector.</rdfs:comment>
        <rdfs:label xml:lang="en">Detector Settings</rdfs:label>
    </owl:Class>
    


    <!-- http://www.openmicroscopy.org/rdf/2016-06/ome_core/DetectorType -->

    <owl:Class rdf:about="http://www.openmicroscopy.org/rdf/2016-06/ome_core/DetectorType">
        <rdfs:comment xml:lang="en">Class &quot;DetectorType&quot; is the types of detectors. E.g. CCD, PMT, EMCCD etc.</rdfs:comment>
        <rdfs:label xml:lang="en">DetectorType</rdfs:label>
    </owl:Class>
    


    <!-- http://www.openmicroscopy.org/rdf/2016-06/ome_core/Dichroic -->

    <owl:Class rdf:about="http://www.openmicroscopy.org/rdf/2016-06/ome_core/Dichroic">
        <rdfs:subClassOf rdf:resource="http://www.openmicroscopy.org/rdf/2016-06/ome_core/ManufacturerSpec"/>
        <rdfs:comment xml:lang="en">Class &quot;Dichroic&quot; is dichromatic beamsplitters or dichroic mirrors used for this filter combination.</rdfs:comment>
        <rdfs:label xml:lang="en">Dichroic</rdfs:label>
    </owl:Class>
    


    <!-- http://www.openmicroscopy.org/rdf/2016-06/ome_core/DimensionOrder -->

    <owl:Class rdf:about="http://www.openmicroscopy.org/rdf/2016-06/ome_core/DimensionOrder">
        <rdfs:comment xml:lang="en">Class &quot;DimensionOrder&quot; is the orders in which the individual planes of data are interleaved.</rdfs:comment>
        <rdfs:label xml:lang="en">DimensionOrder</rdfs:label>
    </owl:Class>
    


    <!-- http://www.openmicroscopy.org/rdf/2016-06/ome_core/DoubleAnnotation -->

    <owl:Class rdf:about="http://www.openmicroscopy.org/rdf/2016-06/ome_core/DoubleAnnotation">
        <rdfs:subClassOf rdf:resource="http://www.openmicroscopy.org/rdf/2016-06/ome_core/StructuredAnnotation"/>
        <rdfs:comment xml:lang="en">Class &quot;DoubleAnnotation&quot; is simple numerical annotations of type xsd:double.</rdfs:comment>
        <rdfs:label xml:lang="en">Double Annotation</rdfs:label>
    </owl:Class>
    


    <!-- http://www.openmicroscopy.org/rdf/2016-06/ome_core/Ellipse -->

    <owl:Class rdf:about="http://www.openmicroscopy.org/rdf/2016-06/ome_core/Ellipse">
        <rdfs:subClassOf rdf:resource="http://www.openmicroscopy.org/rdf/2016-06/ome_core/Shape"/>
        <rdfs:comment xml:lang="en">Class &quot;Ellipse&quot; is simple ellipse objects. If rotation is required apply a transformation at the Shape level.</rdfs:comment>
        <rdfs:label xml:lang="en">Ellipse</rdfs:label>
    </owl:Class>
    


    <!-- http://www.openmicroscopy.org/rdf/2016-06/ome_core/EmissionFilter -->

    <owl:Class rdf:about="http://www.openmicroscopy.org/rdf/2016-06/ome_core/EmissionFilter">
        <rdfs:subClassOf rdf:resource="http://www.openmicroscopy.org/rdf/2016-06/ome_core/Filter"/>
        <rdfs:comment xml:lang="en">Class &quot;EmissionFilter&quot; is a filter placed in the Emission light path.</rdfs:comment>
        <rdfs:label xml:lang="en">EmissionFilter</rdfs:label>
    </owl:Class>
    


    <!-- http://www.openmicroscopy.org/rdf/2016-06/ome_core/Experiment -->

    <owl:Class rdf:about="http://www.openmicroscopy.org/rdf/2016-06/ome_core/Experiment">
        <owl:equivalentClass>
            <owl:Restriction>
                <owl:onProperty rdf:resource="http://www.openmicroscopy.org/rdf/2016-06/ome_core/dataset"/>
                <owl:someValuesFrom rdf:resource="http://www.openmicroscopy.org/rdf/2016-06/ome_core/Dataset"/>
            </owl:Restriction>
        </owl:equivalentClass>
        <owl:equivalentClass>
            <owl:Restriction>
                <owl:onProperty rdf:resource="http://www.openmicroscopy.org/rdf/2016-06/ome_core/experimenterGroup"/>
                <owl:maxQualifiedCardinality rdf:datatype="http://www.w3.org/2001/XMLSchema#nonNegativeInteger">1</owl:maxQualifiedCardinality>
                <owl:onClass rdf:resource="http://www.openmicroscopy.org/rdf/2016-06/ome_core/ExperimenterGroup"/>
            </owl:Restriction>
        </owl:equivalentClass>
        <rdfs:comment xml:lang="en">Class &quot;Experiment&quot; is experiments.</rdfs:comment>
        <rdfs:label xml:lang="en">Experiment</rdfs:label>
    </owl:Class>
    


    <!-- http://www.openmicroscopy.org/rdf/2016-06/ome_core/ExperimentType -->

    <owl:Class rdf:about="http://www.openmicroscopy.org/rdf/2016-06/ome_core/ExperimentType">
        <rdfs:comment xml:lang="en">Class &quot;ExperimentType&quot; is the types of experiments.</rdfs:comment>
        <rdfs:label xml:lang="en">Experiment Type</rdfs:label>
    </owl:Class>
    


    <!-- http://www.openmicroscopy.org/rdf/2016-06/ome_core/ExperimenterGroup -->

    <owl:Class rdf:about="http://www.openmicroscopy.org/rdf/2016-06/ome_core/ExperimenterGroup">
        <rdfs:comment xml:lang="en">Class &quot;ExperimenterGroup&quot; is groups of experimenters. The information should ideally be specified for at least one Leader as a contact for the group. The Leaders are themselves Experimenters.the types of experiments.</rdfs:comment>
        <rdfs:label xml:lang="en">Experimenter Group</rdfs:label>
    </owl:Class>
    


    <!-- http://www.openmicroscopy.org/rdf/2016-06/ome_core/ExtractionFilter -->

    <owl:Class rdf:about="http://www.openmicroscopy.org/rdf/2016-06/ome_core/ExtractionFilter">
        <rdfs:subClassOf rdf:resource="http://www.openmicroscopy.org/rdf/2016-06/ome_core/Filter"/>
        <rdfs:comment xml:lang="en">Class &quot;ExtractionFilter&quot; is a filter placed in the Extraction light path.</rdfs:comment>
        <rdfs:label xml:lang="en">ExtractionFilter</rdfs:label>
    </owl:Class>
    


    <!-- http://www.openmicroscopy.org/rdf/2016-06/ome_core/Filament -->

    <owl:Class rdf:about="http://www.openmicroscopy.org/rdf/2016-06/ome_core/Filament">
        <rdfs:subClassOf rdf:resource="http://www.openmicroscopy.org/rdf/2016-06/ome_core/LightSource"/>
        <rdfs:comment xml:lang="en">Class &quot;Filament&quot; is various kinds of filament bulbs such as Incadescent or Halogen.</rdfs:comment>
        <rdfs:label xml:lang="en">Filament</rdfs:label>
    </owl:Class>
    


    <!-- http://www.openmicroscopy.org/rdf/2016-06/ome_core/FilamentType -->

    <owl:Class rdf:about="http://www.openmicroscopy.org/rdf/2016-06/ome_core/FilamentType">
        <rdfs:comment xml:lang="en">Class &quot;FilamentType&quot; is the types of filaments.</rdfs:comment>
        <rdfs:label xml:lang="en">FilamentType</rdfs:label>
    </owl:Class>
    


    <!-- http://www.openmicroscopy.org/rdf/2016-06/ome_core/FileAnnotation -->

    <owl:Class rdf:about="http://www.openmicroscopy.org/rdf/2016-06/ome_core/FileAnnotation">
        <rdfs:subClassOf rdf:resource="http://www.openmicroscopy.org/rdf/2016-06/ome_core/StructuredAnnotation"/>
        <rdfs:comment xml:lang="en">Class &quot;FilamentType&quot; is file object annotations.</rdfs:comment>
        <rdfs:label xml:lang="en">File Annotation</rdfs:label>
    </owl:Class>
    


    <!-- http://www.openmicroscopy.org/rdf/2016-06/ome_core/FillRule -->

    <owl:Class rdf:about="http://www.openmicroscopy.org/rdf/2016-06/ome_core/FillRule">
        <owl:equivalentClass>
            <owl:Restriction>
                <owl:onProperty rdf:resource="http://www.openmicroscopy.org/rdf/2016-06/ome_core/fillRule"/>
                <owl:maxQualifiedCardinality rdf:datatype="http://www.w3.org/2001/XMLSchema#nonNegativeInteger">1</owl:maxQualifiedCardinality>
                <owl:onClass rdf:resource="http://www.openmicroscopy.org/rdf/2016-06/ome_core/FillRule"/>
            </owl:Restriction>
        </owl:equivalentClass>
        <rdfs:comment xml:lang="en">Class &quot;FillRule&quot; is fill ruless.</rdfs:comment>
        <rdfs:label xml:lang="en">Fill Rule</rdfs:label>
    </owl:Class>
    


    <!-- http://www.openmicroscopy.org/rdf/2016-06/ome_core/Filter -->

    <owl:Class rdf:about="http://www.openmicroscopy.org/rdf/2016-06/ome_core/Filter">
        <rdfs:subClassOf rdf:resource="http://www.openmicroscopy.org/rdf/2016-06/ome_core/ManufacturerSpec"/>
        <rdfs:comment xml:lang="en">Class &quot;Filter&quot; is filters. A filter is either an excitation or emission filters. There should be one filter element specified per wavelength in the image. The channel number associated with a filter set is specified in Channel. It is based on the FilterSpec type, so has the required attributes Manufacturer, Model, and LotNumber.</rdfs:comment>
        <rdfs:label xml:lang="en">Filter</rdfs:label>
    </owl:Class>
    


    <!-- http://www.openmicroscopy.org/rdf/2016-06/ome_core/FilterSet -->

    <owl:Class rdf:about="http://www.openmicroscopy.org/rdf/2016-06/ome_core/FilterSet">
        <rdfs:subClassOf rdf:resource="http://www.openmicroscopy.org/rdf/2016-06/ome_core/ManufacturerSpec"/>
        <rdfs:comment xml:lang="en">Class &quot;FilterSet&quot; is filter set manufacturer specifications.</rdfs:comment>
        <rdfs:label xml:lang="en">Filter Set</rdfs:label>
    </owl:Class>
    


    <!-- http://www.openmicroscopy.org/rdf/2016-06/ome_core/FilterType -->

    <owl:Class rdf:about="http://www.openmicroscopy.org/rdf/2016-06/ome_core/FilterType">
        <rdfs:comment xml:lang="en">Class &quot;FilterType&quot; is the types of filters.</rdfs:comment>
        <rdfs:label xml:lang="en">Filter Type</rdfs:label>
    </owl:Class>
    


    <!-- http://www.openmicroscopy.org/rdf/2016-06/ome_core/Folder -->

    <owl:Class rdf:about="http://www.openmicroscopy.org/rdf/2016-06/ome_core/Folder">
        <rdfs:comment xml:lang="en">Class &quot;Folder&quot; is possibly heterogeneous collections of data. Folders may contain Folders so that data may be organized within a tree of Folders. Data may be in multiple Folders but a Folder may not be in more than one other Folder.</rdfs:comment>
        <rdfs:label xml:lang="en">Folder</rdfs:label>
    </owl:Class>
    


    <!-- http://www.openmicroscopy.org/rdf/2016-06/ome_core/Font -->

    <owl:Class rdf:about="http://www.openmicroscopy.org/rdf/2016-06/ome_core/Font">
        <rdfs:comment xml:lang="en">Class &quot;Font&quot; is fonts used to draw the texts.</rdfs:comment>
        <rdfs:label xml:lang="en">Font</rdfs:label>
    </owl:Class>
    


    <!-- http://www.openmicroscopy.org/rdf/2016-06/ome_core/FontFamily -->

    <owl:Class rdf:about="http://www.openmicroscopy.org/rdf/2016-06/ome_core/FontFamily">
        <rdfs:comment xml:lang="en">Class &quot;FontFamily&quot; is font families used to draw the texts.</rdfs:comment>
        <rdfs:label xml:lang="en">Font Family</rdfs:label>
    </owl:Class>
    


    <!-- http://www.openmicroscopy.org/rdf/2016-06/ome_core/FontStyle -->

    <owl:Class rdf:about="http://www.openmicroscopy.org/rdf/2016-06/ome_core/FontStyle">
        <rdfs:comment xml:lang="en">Class &quot;FontStyle&quot; is font styles used to draw the texts.</rdfs:comment>
        <rdfs:label xml:lang="en">Font Style</rdfs:label>
    </owl:Class>
    


    <!-- http://www.openmicroscopy.org/rdf/2016-06/ome_core/GenericExcitationSource -->

    <owl:Class rdf:about="http://www.openmicroscopy.org/rdf/2016-06/ome_core/GenericExcitationSource">
        <rdfs:comment xml:lang="en">Class &quot;Font&quot; is sources as collections of key/value pairs, stored in Maps. The other lightsource objects should always be used in preference to this if possible..</rdfs:comment>
        <rdfs:label xml:lang="en">General Excitation Source</rdfs:label>
    </owl:Class>
    


    <!-- http://www.openmicroscopy.org/rdf/2016-06/ome_core/IlluminationType -->

    <owl:Class rdf:about="http://www.openmicroscopy.org/rdf/2016-06/ome_core/IlluminationType">
        <rdfs:comment xml:lang="en">Class &quot;Illumination&quot; is methods of illumination used to capture the channel.</rdfs:comment>
        <rdfs:label xml:lang="en">Illumination Type</rdfs:label>
    </owl:Class>
    


    <!-- http://www.openmicroscopy.org/rdf/2016-06/ome_core/Image -->

    <owl:Class rdf:about="http://www.openmicroscopy.org/rdf/2016-06/ome_core/Image">
        <rdfs:comment xml:lang="en">Class &quot;Image&quot; is actual images and their meta-data.</rdfs:comment>
        <rdfs:label xml:lang="en">Image</rdfs:label>
    </owl:Class>
    


    <!-- http://www.openmicroscopy.org/rdf/2016-06/ome_core/ImageFile -->

    <owl:Class rdf:about="http://www.openmicroscopy.org/rdf/2016-06/ome_core/ImageFile">
        <rdfs:comment xml:lang="en">Class &quot;ImageFile&quot; is actual image files.</rdfs:comment>
        <rdfs:label xml:lang="en">Image File</rdfs:label>
    </owl:Class>
    


    <!-- http://www.openmicroscopy.org/rdf/2016-06/ome_core/ImagingCondition -->

    <owl:Class rdf:about="http://www.openmicroscopy.org/rdf/2016-06/ome_core/ImagingCondition">
        <rdfs:comment xml:lang="en">Class &quot;ImageCondition&quot; is image conditions introsuced in the OWL ontology.</rdfs:comment>
        <rdfs:label xml:lang="en">Imaging Condition</rdfs:label>
    </owl:Class>
    


    <!-- http://www.openmicroscopy.org/rdf/2016-06/ome_core/ImagingEnvironment -->

    <owl:Class rdf:about="http://www.openmicroscopy.org/rdf/2016-06/ome_core/ImagingEnvironment">
        <rdfs:comment xml:lang="en">Class &quot;ImageEnvironment&quot; is environments that the biological samples were in during the experiments.</rdfs:comment>
        <rdfs:label xml:lang="en">Imaging Environment</rdfs:label>
    </owl:Class>
    


    <!-- http://www.openmicroscopy.org/rdf/2016-06/ome_core/Immersion -->

    <owl:Class rdf:about="http://www.openmicroscopy.org/rdf/2016-06/ome_core/Immersion">
        <rdfs:comment xml:lang="en">Class &quot;Immersion&quot; is immersion mediums the lens are designed for.</rdfs:comment>
        <rdfs:label xml:lang="en">Immersion</rdfs:label>
    </owl:Class>
    


    <!-- http://www.openmicroscopy.org/rdf/2016-06/ome_core/Instrument -->

    <owl:Class rdf:about="http://www.openmicroscopy.org/rdf/2016-06/ome_core/Instrument">
        <rdfs:comment xml:lang="en">Class &quot;Instrument&quot; is instruments used to capture the Images. It is primarily a container for manufacturer&apos;s model and catalog numbers for the Microscope, LightSource, Detector, Objective and Filters components.</rdfs:comment>
        <rdfs:label xml:lang="en">Instrument</rdfs:label>
    </owl:Class>
    


    <!-- http://www.openmicroscopy.org/rdf/2016-06/ome_core/Label -->

    <owl:Class rdf:about="http://www.openmicroscopy.org/rdf/2016-06/ome_core/Label">
        <rdfs:subClassOf rdf:resource="http://www.openmicroscopy.org/rdf/2016-06/ome_core/Shape"/>
        <rdfs:comment xml:lang="en">Class &quot;Label&quot; is text labels. Any transformation should be applied at the shape level.</rdfs:comment>
        <rdfs:label xml:lang="en">Label</rdfs:label>
    </owl:Class>
    


    <!-- http://www.openmicroscopy.org/rdf/2016-06/ome_core/Laser -->

    <owl:Class rdf:about="http://www.openmicroscopy.org/rdf/2016-06/ome_core/Laser">
        <rdfs:subClassOf rdf:resource="http://www.openmicroscopy.org/rdf/2016-06/ome_core/LightSource"/>
        <rdfs:comment xml:lang="en">Class &quot;Laser&quot; is laser types.</rdfs:comment>
        <rdfs:label xml:lang="en">Laser</rdfs:label>
    </owl:Class>
    


    <!-- http://www.openmicroscopy.org/rdf/2016-06/ome_core/LaserMedium -->

    <owl:Class rdf:about="http://www.openmicroscopy.org/rdf/2016-06/ome_core/LaserMedium">
        <rdfs:subClassOf rdf:resource="http://www.openmicroscopy.org/rdf/2016-06/ome_core/Medium"/>
        <rdfs:comment xml:lang="en">Class &quot;LaserMedium&quot; is actual lasing mediums for given laser types.</rdfs:comment>
        <rdfs:label xml:lang="en">Laser Medium</rdfs:label>
    </owl:Class>
    


    <!-- http://www.openmicroscopy.org/rdf/2016-06/ome_core/LightEmittingDiode -->

    <owl:Class rdf:about="http://www.openmicroscopy.org/rdf/2016-06/ome_core/LightEmittingDiode">
        <rdfs:comment xml:lang="en">Class &quot;LightEmittingDiode&quot; is various kinds of LED lamps.</rdfs:comment>
        <rdfs:label xml:lang="en">LED</rdfs:label>
        <rdfs:label xml:lang="en">Light Emitting Diode</rdfs:label>
    </owl:Class>
    


    <!-- http://www.openmicroscopy.org/rdf/2016-06/ome_core/LightPath -->

    <owl:Class rdf:about="http://www.openmicroscopy.org/rdf/2016-06/ome_core/LightPath">
        <rdfs:comment xml:lang="en">Class &quot;LightPath&quot; is light paths.</rdfs:comment>
        <rdfs:label xml:lang="en">Lignt Path</rdfs:label>
    </owl:Class>
    


    <!-- http://www.openmicroscopy.org/rdf/2016-06/ome_core/LightSource -->

    <owl:Class rdf:about="http://www.openmicroscopy.org/rdf/2016-06/ome_core/LightSource">
        <rdfs:subClassOf rdf:resource="http://www.openmicroscopy.org/rdf/2016-06/ome_core/ManufacturerSpec"/>
        <rdfs:comment xml:lang="en">Class &quot;LightSource&quot; is light sources for the instruments.</rdfs:comment>
        <rdfs:label xml:lang="en">Light Source</rdfs:label>
    </owl:Class>
    


    <!-- http://www.openmicroscopy.org/rdf/2016-06/ome_core/LightSourceSettings -->

    <owl:Class rdf:about="http://www.openmicroscopy.org/rdf/2016-06/ome_core/LightSourceSettings">
        <rdfs:subClassOf rdf:resource="http://www.openmicroscopy.org/rdf/2016-06/ome_core/Settings"/>
        <rdfs:comment xml:lang="en">Class &quot;LightSourceSettings&quot; is settings of light sources for the instruments.</rdfs:comment>
        <rdfs:label xml:lang="en">Light Source Settings</rdfs:label>
    </owl:Class>
    


    <!-- http://www.openmicroscopy.org/rdf/2016-06/ome_core/Line -->

    <owl:Class rdf:about="http://www.openmicroscopy.org/rdf/2016-06/ome_core/Line">
        <rdfs:subClassOf rdf:resource="http://www.openmicroscopy.org/rdf/2016-06/ome_core/Shape"/>
        <rdfs:comment xml:lang="en">Class &quot;Line&quot; is straight lines defined by their end points.</rdfs:comment>
        <rdfs:label xml:lang="en">Line</rdfs:label>
    </owl:Class>
    


    <!-- http://www.openmicroscopy.org/rdf/2016-06/ome_core/ListAnnotation -->

    <owl:Class rdf:about="http://www.openmicroscopy.org/rdf/2016-06/ome_core/ListAnnotation">
        <rdfs:subClassOf rdf:resource="http://www.openmicroscopy.org/rdf/2016-06/ome_core/StructuredAnnotation"/>
        <rdfs:comment xml:lang="en">Class &quot;ListAnnotation&quot; is groups of annotation objects. It uses the sequence of annotation refs from the base Annotation to form the list.</rdfs:comment>
        <rdfs:label xml:lang="en">List Annotation</rdfs:label>
    </owl:Class>
    


    <!-- http://www.openmicroscopy.org/rdf/2016-06/ome_core/LongAnnotation -->

    <owl:Class rdf:about="http://www.openmicroscopy.org/rdf/2016-06/ome_core/LongAnnotation">
        <rdfs:subClassOf rdf:resource="http://www.openmicroscopy.org/rdf/2016-06/ome_core/StructuredAnnotation"/>
        <rdfs:comment xml:lang="en">Class &quot;LongAnnotation&quot; is simple numerical annotations of type xsd:long</rdfs:comment>
        <rdfs:label xml:lang="en">Long Annotation</rdfs:label>
    </owl:Class>
    


    <!-- http://www.openmicroscopy.org/rdf/2016-06/ome_core/Manufacturer -->

    <owl:Class rdf:about="http://www.openmicroscopy.org/rdf/2016-06/ome_core/Manufacturer">
        <rdfs:comment xml:lang="en">Class &quot;Manufacturer&quot; is manufacturers of the components.</rdfs:comment>
        <rdfs:label xml:lang="en">Manufacturer</rdfs:label>
    </owl:Class>
    


    <!-- http://www.openmicroscopy.org/rdf/2016-06/ome_core/ManufacturerSpec -->

    <owl:Class rdf:about="http://www.openmicroscopy.org/rdf/2016-06/ome_core/ManufacturerSpec">
        <rdfs:comment xml:lang="en">Class &quot;ManufacturerSpec&quot; is the base from which many microscope components are extended. E.g Objective, Filter etc. Provides attributes for recording common properties of these components such as Manufacturer name, Model etc, all of which are optional.</rdfs:comment>
        <rdfs:label xml:lang="en">Manufacture Spec</rdfs:label>
    </owl:Class>
    


    <!-- http://www.openmicroscopy.org/rdf/2016-06/ome_core/Map -->

    <owl:Class rdf:about="http://www.openmicroscopy.org/rdf/2016-06/ome_core/Map">
        <rdfs:comment xml:lang="en">Class &quot;Map&quot; is mappings of key/value pairs.</rdfs:comment>
        <rdfs:label xml:lang="en">Map</rdfs:label>
    </owl:Class>
    


    <!-- http://www.openmicroscopy.org/rdf/2016-06/ome_core/MapAnnotation -->

    <owl:Class rdf:about="http://www.openmicroscopy.org/rdf/2016-06/ome_core/MapAnnotation">
        <rdfs:subClassOf rdf:resource="http://www.openmicroscopy.org/rdf/2016-06/ome_core/StructuredAnnotation"/>
        <rdfs:comment xml:lang="en">Class &quot;MapAnnotation&quot; is map annotations. The contents of this is a list of key/value pairs.</rdfs:comment>
        <rdfs:label xml:lang="en">Map Annotation</rdfs:label>
    </owl:Class>
    


    <!-- http://www.openmicroscopy.org/rdf/2016-06/ome_core/Marker -->

    <owl:Class rdf:about="http://www.openmicroscopy.org/rdf/2016-06/ome_core/Marker">
        <rdfs:comment xml:lang="en">Class &quot;Marker&quot; is shapes of marker on the ends of lines.</rdfs:comment>
        <rdfs:label xml:lang="en">Marker</rdfs:label>
    </owl:Class>
    


    <!-- http://www.openmicroscopy.org/rdf/2016-06/ome_core/Mask -->

    <owl:Class rdf:about="http://www.openmicroscopy.org/rdf/2016-06/ome_core/Mask">
        <rdfs:subClassOf rdf:resource="http://www.openmicroscopy.org/rdf/2016-06/ome_core/Shape"/>
        <rdfs:comment xml:lang="en">Class &quot;Mask&quot; is masks. A mask ROI shape is a link to a BinData object that is a BIT mask drawn on top of the image as an ROI. It is applied at the same scale, pixel to pixel, as the Image the ROI is applied to, unless a transform is applied at the shape level.shapes of marker on the ends of lines.</rdfs:comment>
        <rdfs:label xml:lang="en">Mask</rdfs:label>
    </owl:Class>
    


    <!-- http://www.openmicroscopy.org/rdf/2016-06/ome_core/Medium -->

    <owl:Class rdf:about="http://www.openmicroscopy.org/rdf/2016-06/ome_core/Medium">
        <rdfs:comment xml:lang="en">Class &quot;Medium&quot; is the mediums used for lenses.</rdfs:comment>
        <rdfs:label xml:lang="en">Medium</rdfs:label>
    </owl:Class>
    


    <!-- http://www.openmicroscopy.org/rdf/2016-06/ome_core/MicrobeamManipuration -->

    <owl:Class rdf:about="http://www.openmicroscopy.org/rdf/2016-06/ome_core/MicrobeamManipuration">
        <rdfs:comment xml:lang="en">Class &quot;MicrobeamManipuration&quot; is microbeam operation types and the regions of the images.</rdfs:comment>
        <rdfs:label xml:lang="en">Microbeam Manipuration</rdfs:label>
    </owl:Class>
    


    <!-- http://www.openmicroscopy.org/rdf/2016-06/ome_core/Microscope -->

    <owl:Class rdf:about="http://www.openmicroscopy.org/rdf/2016-06/ome_core/Microscope">
        <rdfs:comment xml:lang="en">Class &quot;Microscope&quot; is microscopes&apos; manufacturer specifications.</rdfs:comment>
        <rdfs:label xml:lang="en">Microscope</rdfs:label>
    </owl:Class>
    


    <!-- http://www.openmicroscopy.org/rdf/2016-06/ome_core/Model -->

    <owl:Class rdf:about="http://www.openmicroscopy.org/rdf/2016-06/ome_core/Model">
        <rdfs:comment xml:lang="en">Class &quot;Model&quot; is models of the components.</rdfs:comment>
        <rdfs:label xml:lang="en">Model</rdfs:label>
    </owl:Class>
    


    <!-- http://www.openmicroscopy.org/rdf/2016-06/ome_core/NamingConvention -->

    <owl:Class rdf:about="http://www.openmicroscopy.org/rdf/2016-06/ome_core/NamingConvention">
        <rdfs:comment xml:lang="en">Class &quot;NamingConvention&quot; is predefined lists of values for the well labels.</rdfs:comment>
        <rdfs:label xml:lang="en">Naming Convention</rdfs:label>
    </owl:Class>
    


    <!-- http://www.openmicroscopy.org/rdf/2016-06/ome_core/Objective -->

    <owl:Class rdf:about="http://www.openmicroscopy.org/rdf/2016-06/ome_core/Objective">
        <rdfs:subClassOf rdf:resource="http://www.openmicroscopy.org/rdf/2016-06/ome_core/ManufacturerSpec"/>
        <rdfs:comment xml:lang="en">Class &quot;Objective&quot; is microscopes&apos; objective lens.</rdfs:comment>
        <rdfs:label xml:lang="en">Objective</rdfs:label>
    </owl:Class>
    


    <!-- http://www.openmicroscopy.org/rdf/2016-06/ome_core/ObjectiveMedium -->

    <owl:Class rdf:about="http://www.openmicroscopy.org/rdf/2016-06/ome_core/ObjectiveMedium">
        <rdfs:subClassOf rdf:resource="http://www.openmicroscopy.org/rdf/2016-06/ome_core/Medium"/>
        <rdfs:comment xml:lang="en">Class &quot;ObjectiveMedium&quot; is a description of a Medium used for the lens. The Medium is the actual immersion medium used in this case.</rdfs:comment>
        <rdfs:label xml:lang="en">Objective Medium</rdfs:label>
    </owl:Class>
    


    <!-- http://www.openmicroscopy.org/rdf/2016-06/ome_core/ObjectiveSettings -->

    <owl:Class rdf:about="http://www.openmicroscopy.org/rdf/2016-06/ome_core/ObjectiveSettings">
        <rdfs:subClassOf rdf:resource="http://www.openmicroscopy.org/rdf/2016-06/ome_core/Settings"/>
        <rdfs:comment xml:lang="en">Class &quot;ObjectiveSettings&quot; is settings applied to an objective as well as a reference to the objective.</rdfs:comment>
        <rdfs:label xml:lang="en">Objective Settings</rdfs:label>
    </owl:Class>
    


    <!-- http://www.openmicroscopy.org/rdf/2016-06/ome_core/PixelType -->

    <owl:Class rdf:about="http://www.openmicroscopy.org/rdf/2016-06/ome_core/PixelType">
        <rdfs:comment xml:lang="en">Class &quot;PixelType&quot; is numbers size/kind used to represent pixels.</rdfs:comment>
        <rdfs:label xml:lang="en">Pixel Type</rdfs:label>
    </owl:Class>
    


    <!-- http://www.openmicroscopy.org/rdf/2016-06/ome_core/Pixels -->

    <owl:Class rdf:about="http://www.openmicroscopy.org/rdf/2016-06/ome_core/Pixels">
        <rdfs:comment xml:lang="en">Class &quot;Pixels&quot; is pixels. Pixels is going to be removed in the future, but it is still required.</rdfs:comment>
        <rdfs:label xml:lang="en">Pixels</rdfs:label>
    </owl:Class>
    


    <!-- http://www.openmicroscopy.org/rdf/2016-06/ome_core/Plane -->

    <owl:Class rdf:about="http://www.openmicroscopy.org/rdf/2016-06/ome_core/Plane">
        <rdfs:comment xml:lang="en">Class &quot;Plane&quot; is microscope stages and image timing data for given channels/z-sections/timepoints.</rdfs:comment>
        <rdfs:label xml:lang="en">Plane</rdfs:label>
    </owl:Class>
    


    <!-- http://www.openmicroscopy.org/rdf/2016-06/ome_core/Plate -->

    <owl:Class rdf:about="http://www.openmicroscopy.org/rdf/2016-06/ome_core/Plate">
        <rdfs:comment xml:lang="en">Class &quot;Plate&quot; is microtiter plates within a screen. A plate can belong to more than one screen. The Screen(s) that a plate belongs to are specified by the ScreenRef element. The Plate ID and Name attributes are required.The Wells in a plate are numbers from the top-left corner in a grid starting at zero. i.e. The top-left well of a plate is index (0,0).</rdfs:comment>
        <rdfs:label xml:lang="en">Plate</rdfs:label>
    </owl:Class>
    


    <!-- http://www.openmicroscopy.org/rdf/2016-06/ome_core/PlateAcquisition -->

    <owl:Class rdf:about="http://www.openmicroscopy.org/rdf/2016-06/ome_core/PlateAcquisition">
        <rdfs:comment xml:lang="en">Class &quot;PlateAcquisition&quot; is single acquisition runs for plates. This object is used to record the set of images acquired in a single acquisition run. The Images for this run are linked to PlateAcquisition through WellSample.</rdfs:comment>
        <rdfs:label xml:lang="en">Plate Acquision</rdfs:label>
    </owl:Class>
    


    <!-- http://www.openmicroscopy.org/rdf/2016-06/ome_core/Point -->

    <owl:Class rdf:about="http://www.openmicroscopy.org/rdf/2016-06/ome_core/Point">
        <rdfs:subClassOf rdf:resource="http://www.openmicroscopy.org/rdf/2016-06/ome_core/Shape"/>
        <rdfs:comment xml:lang="en">Class &quot;Point&quot; is points.</rdfs:comment>
        <rdfs:label xml:lang="en">Point</rdfs:label>
    </owl:Class>
    


    <!-- http://www.openmicroscopy.org/rdf/2016-06/ome_core/Polygon -->

    <owl:Class rdf:about="http://www.openmicroscopy.org/rdf/2016-06/ome_core/Polygon">
        <rdfs:subClassOf rdf:resource="http://www.openmicroscopy.org/rdf/2016-06/ome_core/Shape"/>
        <rdfs:comment xml:lang="en">Class &quot;Polygon&quot; is closed shapes formed of straight lines. Note: Polygon uses counterclockwise winding (this is the default OpenGL behavior).</rdfs:comment>
        <rdfs:label xml:lang="en">Polygon</rdfs:label>
    </owl:Class>
    


    <!-- http://www.openmicroscopy.org/rdf/2016-06/ome_core/Polyline -->

    <owl:Class rdf:about="http://www.openmicroscopy.org/rdf/2016-06/ome_core/Polyline">
        <rdfs:subClassOf rdf:resource="http://www.openmicroscopy.org/rdf/2016-06/ome_core/Shape"/>
        <rdfs:comment xml:lang="en">Class &quot;Polyline&quot; is  open shapes formed of straight lines. Note: Polyline uses counterclockwise winding (this is the default OpenGL behavior).</rdfs:comment>
        <rdfs:label xml:lang="en">Polyline</rdfs:label>
    </owl:Class>
    


    <!-- http://www.openmicroscopy.org/rdf/2016-06/ome_core/Project -->

    <owl:Class rdf:about="http://www.openmicroscopy.org/rdf/2016-06/ome_core/Project">
        <owl:equivalentClass>
            <owl:Restriction>
                <owl:onProperty rdf:resource="http://www.openmicroscopy.org/rdf/2016-06/ome_core/experiment"/>
                <owl:someValuesFrom rdf:resource="http://www.openmicroscopy.org/rdf/2016-06/ome_core/Experiment"/>
            </owl:Restriction>
        </owl:equivalentClass>
        <rdfs:comment xml:lang="en">Class &quot;Project&quot; is projects. Datasets can be grouped into projects using a many-to-many relationship. A Dataset may belong to one or more Projects. Projects do not directly contain images - only by virtue of containing datasets, which themselves contain images.</rdfs:comment>
        <rdfs:label xml:lang="en">Project</rdfs:label>
    </owl:Class>
    


    <!-- http://www.openmicroscopy.org/rdf/2016-06/ome_core/Protocol -->

    <owl:Class rdf:about="http://www.openmicroscopy.org/rdf/2016-06/ome_core/Protocol">
        <rdfs:comment xml:lang="en">Class &quot;Protocol&quot; is screen protocols.</rdfs:comment>
        <rdfs:label xml:lang="en">Protocol</rdfs:label>
    </owl:Class>
    


    <!-- http://www.openmicroscopy.org/rdf/2016-06/ome_core/Pulse -->

    <owl:Class rdf:about="http://www.openmicroscopy.org/rdf/2016-06/ome_core/Pulse">
        <rdfs:comment xml:lang="en">Class &quot;Pulse&quot; is the pulse modes of the lasers.</rdfs:comment>
        <rdfs:label xml:lang="en">Pulse</rdfs:label>
    </owl:Class>
    


    <!-- http://www.openmicroscopy.org/rdf/2016-06/ome_core/Pump -->

    <owl:Class rdf:about="http://www.openmicroscopy.org/rdf/2016-06/ome_core/Pump">
        <rdfs:comment xml:lang="en">Class &quot;Pump&quot; is references to the light sources.  It is used within the Laser element to specify the light source for the laser&apos;s pump (if any).</rdfs:comment>
        <rdfs:label xml:lang="en">Pump</rdfs:label>
    </owl:Class>
    


    <!-- http://www.openmicroscopy.org/rdf/2016-06/ome_core/Reagent -->

    <owl:Class rdf:about="http://www.openmicroscopy.org/rdf/2016-06/ome_core/Reagent">
        <rdfs:comment xml:lang="en">Class &quot;Reagent&quot; is chemical or some other physical experimental parameters.</rdfs:comment>
        <rdfs:label xml:lang="en">Reagent</rdfs:label>
    </owl:Class>
    


    <!-- http://www.openmicroscopy.org/rdf/2016-06/ome_core/ReagentSet -->

    <owl:Class rdf:about="http://www.openmicroscopy.org/rdf/2016-06/ome_core/ReagentSet">
        <rdfs:comment xml:lang="en">Class &quot;ReagentSet&quot; is sets of reagents; may contain very detailed information toreproduce some of that information found in a screening database.</rdfs:comment>
        <rdfs:label xml:lang="en">Reagent Set</rdfs:label>
    </owl:Class>
    


    <!-- http://www.openmicroscopy.org/rdf/2016-06/ome_core/Rectangle -->

    <owl:Class rdf:about="http://www.openmicroscopy.org/rdf/2016-06/ome_core/Rectangle">
        <rdfs:subClassOf rdf:resource="http://www.openmicroscopy.org/rdf/2016-06/ome_core/Shape"/>
        <rdfs:comment xml:lang="en">Class &quot;Rectangle&quot; is simple rectangle objects. If rotation is required apply a transformation at the Shape level.</rdfs:comment>
        <rdfs:label xml:lang="en">Rectangle</rdfs:label>
    </owl:Class>
    


    <!-- http://www.openmicroscopy.org/rdf/2016-06/ome_core/RegionOfInterest -->

    <owl:Class rdf:about="http://www.openmicroscopy.org/rdf/2016-06/ome_core/RegionOfInterest">
        <rdfs:comment xml:lang="en">Class &quot;RigionOfInterest&quot; is four dimensional &apos;Region of Interests&apos;. If they are not used, and the Image has more than one plane, the entire set of planes is assumed to be included in the ROI. Multiple ROIs may be specified.</rdfs:comment>
        <rdfs:label xml:lang="en">Region of Interest</rdfs:label>
    </owl:Class>
    


    <!-- http://www.openmicroscopy.org/rdf/2016-06/ome_core/Rights -->

    <owl:Class rdf:about="http://www.openmicroscopy.org/rdf/2016-06/ome_core/Rights"/>
    


    <!-- http://www.openmicroscopy.org/rdf/2016-06/ome_core/Screen -->

    <owl:Class rdf:about="http://www.openmicroscopy.org/rdf/2016-06/ome_core/Screen">
        <rdfs:comment xml:lang="en">Class &quot;Screen&quot; is groupings for Plates..</rdfs:comment>
        <rdfs:label xml:lang="en">Screen</rdfs:label>
    </owl:Class>
    


    <!-- http://www.openmicroscopy.org/rdf/2016-06/ome_core/Settings -->

    <owl:Class rdf:about="http://www.openmicroscopy.org/rdf/2016-06/ome_core/Settings">
        <rdfs:comment xml:lang="en">Class &quot;Settings&quot; is a super class of &quot;DetectorSettings&quot;, &quot;LightSourceSettings&quot; and &quot;ObjectiveSettings&quot;.</rdfs:comment>
        <rdfs:label xml:lang="en">Settings</rdfs:label>
    </owl:Class>
    


    <!-- http://www.openmicroscopy.org/rdf/2016-06/ome_core/Shape -->

    <owl:Class rdf:about="http://www.openmicroscopy.org/rdf/2016-06/ome_core/Shape">
        <rdfs:comment xml:lang="en">Class &quot;Shape&quot; is single specific ROI shapes and links that to any channels, and timepoints and z-sections. It alsorecords any transform applied to the ROI shape.</rdfs:comment>
        <rdfs:label xml:lang="en">Shape</rdfs:label>
    </owl:Class>
    


    <!-- http://www.openmicroscopy.org/rdf/2016-06/ome_core/StageLabel -->

    <owl:Class rdf:about="http://www.openmicroscopy.org/rdf/2016-06/ome_core/StageLabel">
        <rdfs:comment xml:lang="en">Class &quot;StageLabel&quot; is used to specify a name and position for a stage position in the microscope&apos;s reference frame.</rdfs:comment>
        <rdfs:label xml:lang="en">StageLabel</rdfs:label>
    </owl:Class>
    


    <!-- http://www.openmicroscopy.org/rdf/2016-06/ome_core/StructuredAnnotation -->

    <owl:Class rdf:about="http://www.openmicroscopy.org/rdf/2016-06/ome_core/StructuredAnnotation">
        <rdfs:comment xml:lang="en">Class &quot;StructuredAnnotation&quot; is unordered collections of annotations attached to objects in the OME data model.</rdfs:comment>
        <rdfs:label xml:lang="en">Structured Annimation</rdfs:label>
    </owl:Class>
    


    <!-- http://www.openmicroscopy.org/rdf/2016-06/ome_core/TagAnnotation -->

    <owl:Class rdf:about="http://www.openmicroscopy.org/rdf/2016-06/ome_core/TagAnnotation">
        <rdfs:comment xml:lang="en">Class &quot;TagAnnotation&quot; is .</rdfs:comment>
        <rdfs:label xml:lang="en">Tag Annotation</rdfs:label>
    </owl:Class>
    


    <!-- http://www.openmicroscopy.org/rdf/2016-06/ome_core/TermAnnotation -->

    <owl:Class rdf:about="http://www.openmicroscopy.org/rdf/2016-06/ome_core/TermAnnotation">
        <rdfs:comment xml:lang="en">Class &quot;TermAnnotation&quot; is tag annotations. A tag annotation represents a tag or a tagset.</rdfs:comment>
        <rdfs:label xml:lang="en">Term Annotation</rdfs:label>
    </owl:Class>
    


    <!-- http://www.openmicroscopy.org/rdf/2016-06/ome_core/TiffData -->

    <owl:Class rdf:about="http://www.openmicroscopy.org/rdf/2016-06/ome_core/TiffData">
        <rdfs:subClassOf rdf:resource="http://www.openmicroscopy.org/rdf/2016-06/ome_core/BinData"/>
        <rdfs:comment xml:lang="en">Class &quot;TiffData&quot; is locations of the pixel data in tiff files.</rdfs:comment>
        <rdfs:label xml:lang="en">Tiff Data</rdfs:label>
    </owl:Class>
    


    <!-- http://www.openmicroscopy.org/rdf/2016-06/ome_core/TimestampAnnotation -->

    <owl:Class rdf:about="http://www.openmicroscopy.org/rdf/2016-06/ome_core/TimestampAnnotation">
        <rdfs:comment xml:lang="en">Class &quot;TimestampAnnotation&quot; is date/time annotations of type xsd:dateTime</rdfs:comment>
        <rdfs:label xml:lang="en">Timestamp Annotation</rdfs:label>
    </owl:Class>
    


    <!-- http://www.openmicroscopy.org/rdf/2016-06/ome_core/Transform -->

    <owl:Class rdf:about="http://www.openmicroscopy.org/rdf/2016-06/ome_core/Transform">
        <rdfs:comment xml:lang="en">Class &quot;Transform&quot; is matrixes used to transform the shapes.</rdfs:comment>
        <rdfs:label xml:lang="en">Transform</rdfs:label>
    </owl:Class>
    


    <!-- http://www.openmicroscopy.org/rdf/2016-06/ome_core/TransmittanceRange -->

    <owl:Class rdf:about="http://www.openmicroscopy.org/rdf/2016-06/ome_core/TransmittanceRange">
        <rdfs:comment xml:lang="en">Class &quot;TransmittanceRange&quot; is ranges of wavelengths that are transmitted by the filters. It also records the maximum amount of light transmitted.</rdfs:comment>
        <rdfs:label xml:lang="en">Transmittance Range</rdfs:label>
    </owl:Class>
    


    <!-- http://www.openmicroscopy.org/rdf/2016-06/ome_core/Well -->

    <owl:Class rdf:about="http://www.openmicroscopy.org/rdf/2016-06/ome_core/Well">
        <rdfs:comment xml:lang="en">Class &quot;Well&quot; is components of the Well/Plate/Screen constructs to describe screening applications. A Well has a number of WellSample elements that link to the Images collected in this well. The ReagentRef links any Reagents that were used in this Well. A well is part of only one Plate. The origin for the row and column identifiers is the top left corner of the plate starting at zero. i.e The top left well of a plate is index (0,0).</rdfs:comment>
        <rdfs:label xml:lang="en">Well</rdfs:label>
    </owl:Class>
    


    <!-- http://www.openmicroscopy.org/rdf/2016-06/ome_core/WellSample -->

    <owl:Class rdf:about="http://www.openmicroscopy.org/rdf/2016-06/ome_core/WellSample">
        <rdfs:comment xml:lang="en">Class &quot;WellSample&quot; is individual images that have been captured within Wells.</rdfs:comment>
        <rdfs:label xml:lang="en">Well Sample</rdfs:label>
    </owl:Class>
    


    <!-- http://www.openmicroscopy.org/rdf/2016-06/ome_core/XMLAnnotation -->

    <owl:Class rdf:about="http://www.openmicroscopy.org/rdf/2016-06/ome_core/XMLAnnotation">
        <rdfs:comment xml:lang="en">Class &quot;XMLAnnotation&quot; is general xml annotations. The contents of this is not processed as OME XML but should still be well-formed XML.</rdfs:comment>
        <rdfs:label xml:lang="en">XML Annotation</rdfs:label>
    </owl:Class>
    


    <!-- http://www.w3.org/1999/02/22-rdf-syntax-ns#Bag -->

    <owl:Class rdf:about="http://www.w3.org/1999/02/22-rdf-syntax-ns#Bag">
        <rdfs:label xml:lang="en">Bag</rdfs:label>
    </owl:Class>
    


    <!-- http://www.w3.org/1999/02/22-rdf-syntax-ns#Seq -->

    <owl:Class rdf:about="http://www.w3.org/1999/02/22-rdf-syntax-ns#Seq">
        <rdfs:label xml:lang="en">Seq</rdfs:label>
    </owl:Class>
    


    <!-- http://xmlns.com/foaf/0.1/Person -->

    <owl:Class rdf:about="http://xmlns.com/foaf/0.1/Person">
        <rdfs:label xml:lang="en">Person</rdfs:label>
    </owl:Class>
    


    <!-- 
    ///////////////////////////////////////////////////////////////////////////////////////
    //
    // Individuals
    //
    ///////////////////////////////////////////////////////////////////////////////////////
     -->

    


    <!-- http://www.openmicroscopy.org/rdf/2016-06/ome_core/AcquisitionMode#FSM -->

    <owl:NamedIndividual rdf:about="http://www.openmicroscopy.org/rdf/2016-06/ome_core/AcquisitionMode#FSM">
        <rdf:type rdf:resource="http://www.openmicroscopy.org/rdf/2016-06/ome_core/AcquisitionMode"/>
        <rdfs:label xml:lang="en">FSM</rdfs:label>
    </owl:NamedIndividual>
    


    <!-- http://www.openmicroscopy.org/rdf/2016-06/ome_core/AcquisitionMode#LCM -->

    <owl:NamedIndividual rdf:about="http://www.openmicroscopy.org/rdf/2016-06/ome_core/AcquisitionMode#LCM">
        <rdf:type rdf:resource="http://www.openmicroscopy.org/rdf/2016-06/ome_core/AcquisitionMode"/>
        <rdfs:label xml:lang="en">LCM</rdfs:label>
    </owl:NamedIndividual>
    


    <!-- http://www.openmicroscopy.org/rdf/2016-06/ome_core/AcquisitionMode#PALM -->

    <owl:NamedIndividual rdf:about="http://www.openmicroscopy.org/rdf/2016-06/ome_core/AcquisitionMode#PALM">
        <rdf:type rdf:resource="http://www.openmicroscopy.org/rdf/2016-06/ome_core/AcquisitionMode"/>
        <rdfs:label xml:lang="en">PALM</rdfs:label>
    </owl:NamedIndividual>
    


    <!-- http://www.openmicroscopy.org/rdf/2016-06/ome_core/AcquisitionMode#SPIM -->

    <owl:NamedIndividual rdf:about="http://www.openmicroscopy.org/rdf/2016-06/ome_core/AcquisitionMode#SPIM">
        <rdf:type rdf:resource="http://www.openmicroscopy.org/rdf/2016-06/ome_core/AcquisitionMode"/>
        <rdfs:label xml:lang="en">SPIM</rdfs:label>
    </owl:NamedIndividual>
    


    <!-- http://www.openmicroscopy.org/rdf/2016-06/ome_core/AcquisitionMode#STED -->

    <owl:NamedIndividual rdf:about="http://www.openmicroscopy.org/rdf/2016-06/ome_core/AcquisitionMode#STED">
        <rdf:type rdf:resource="http://www.openmicroscopy.org/rdf/2016-06/ome_core/AcquisitionMode"/>
        <rdfs:label xml:lang="en">STED</rdfs:label>
    </owl:NamedIndividual>
    


    <!-- http://www.openmicroscopy.org/rdf/2016-06/ome_core/AcquisitionMode#STORM -->

    <owl:NamedIndividual rdf:about="http://www.openmicroscopy.org/rdf/2016-06/ome_core/AcquisitionMode#STORM">
        <rdf:type rdf:resource="http://www.openmicroscopy.org/rdf/2016-06/ome_core/AcquisitionMode"/>
        <rdfs:label xml:lang="en">STORM</rdfs:label>
    </owl:NamedIndividual>
    


    <!-- http://www.openmicroscopy.org/rdf/2016-06/ome_core/AcquisitionMode#TIRF -->

    <owl:NamedIndividual rdf:about="http://www.openmicroscopy.org/rdf/2016-06/ome_core/AcquisitionMode#TIRF">
        <rdf:type rdf:resource="http://www.openmicroscopy.org/rdf/2016-06/ome_core/AcquisitionMode"/>
        <rdfs:label xml:lang="en">TIRF</rdfs:label>
    </owl:NamedIndividual>
    


    <!-- http://www.openmicroscopy.org/rdf/2016-06/ome_core/AcquisitionMode#brightField -->

    <owl:NamedIndividual rdf:about="http://www.openmicroscopy.org/rdf/2016-06/ome_core/AcquisitionMode#brightField">
        <rdf:type rdf:resource="http://www.openmicroscopy.org/rdf/2016-06/ome_core/AcquisitionMode"/>
        <rdfs:label xml:lang="en">bright field</rdfs:label>
    </owl:NamedIndividual>
    


    <!-- http://www.openmicroscopy.org/rdf/2016-06/ome_core/AcquisitionMode#fluorescenceCorrelationSpectroscopy -->

    <owl:NamedIndividual rdf:about="http://www.openmicroscopy.org/rdf/2016-06/ome_core/AcquisitionMode#fluorescenceCorrelationSpectroscopy">
        <rdf:type rdf:resource="http://www.openmicroscopy.org/rdf/2016-06/ome_core/AcquisitionMode"/>
        <rdfs:label xml:lang="en">fluorescence correlation spectroscopy</rdfs:label>
    </owl:NamedIndividual>
    


    <!-- http://www.openmicroscopy.org/rdf/2016-06/ome_core/AcquisitionMode#fluorescenceLifetime -->

    <owl:NamedIndividual rdf:about="http://www.openmicroscopy.org/rdf/2016-06/ome_core/AcquisitionMode#fluorescenceLifetime">
        <rdf:type rdf:resource="http://www.openmicroscopy.org/rdf/2016-06/ome_core/AcquisitionMode"/>
        <rdfs:label xml:lang="en">fluorescence lifetime</rdfs:label>
    </owl:NamedIndividual>
    


    <!-- http://www.openmicroscopy.org/rdf/2016-06/ome_core/AcquisitionMode#laserScanningConfocalMicroscopy -->

    <owl:NamedIndividual rdf:about="http://www.openmicroscopy.org/rdf/2016-06/ome_core/AcquisitionMode#laserScanningConfocalMicroscopy">
        <rdf:type rdf:resource="http://www.openmicroscopy.org/rdf/2016-06/ome_core/AcquisitionMode"/>
        <rdfs:label xml:lang="en">laser scanning confocal microscopy</rdfs:label>
    </owl:NamedIndividual>
    


    <!-- http://www.openmicroscopy.org/rdf/2016-06/ome_core/AcquisitionMode#multiPhotonMicroscopy -->

    <owl:NamedIndividual rdf:about="http://www.openmicroscopy.org/rdf/2016-06/ome_core/AcquisitionMode#multiPhotonMicroscopy">
        <rdf:type rdf:resource="http://www.openmicroscopy.org/rdf/2016-06/ome_core/AcquisitionMode"/>
        <rdfs:label xml:lang="en">multi photon microscopy</rdfs:label>
    </owl:NamedIndividual>
    


    <!-- http://www.openmicroscopy.org/rdf/2016-06/ome_core/AcquisitionMode#nearFieldScanningOpticalMicroscopy -->

    <owl:NamedIndividual rdf:about="http://www.openmicroscopy.org/rdf/2016-06/ome_core/AcquisitionMode#nearFieldScanningOpticalMicroscopy">
        <rdf:type rdf:resource="http://www.openmicroscopy.org/rdf/2016-06/ome_core/AcquisitionMode"/>
        <rdfs:label xml:lang="en">near field scanning optical microscopy</rdfs:label>
    </owl:NamedIndividual>
    


    <!-- http://www.openmicroscopy.org/rdf/2016-06/ome_core/AcquisitionMode#secondHarmonicGenerationImaging -->

    <owl:NamedIndividual rdf:about="http://www.openmicroscopy.org/rdf/2016-06/ome_core/AcquisitionMode#secondHarmonicGenerationImaging">
        <rdf:type rdf:resource="http://www.openmicroscopy.org/rdf/2016-06/ome_core/AcquisitionMode"/>
        <rdfs:label xml:lang="en">second harmonic generation imaging</rdfs:label>
    </owl:NamedIndividual>
    


    <!-- http://www.openmicroscopy.org/rdf/2016-06/ome_core/AcquisitionMode#singleMoleculeImaging -->

    <owl:NamedIndividual rdf:about="http://www.openmicroscopy.org/rdf/2016-06/ome_core/AcquisitionMode#singleMoleculeImaging">
        <rdf:type rdf:resource="http://www.openmicroscopy.org/rdf/2016-06/ome_core/AcquisitionMode"/>
        <rdfs:label xml:lang="en">single molecule imaging</rdfs:label>
    </owl:NamedIndividual>
    


    <!-- http://www.openmicroscopy.org/rdf/2016-06/ome_core/AcquisitionMode#slitScanConfocal -->

    <owl:NamedIndividual rdf:about="http://www.openmicroscopy.org/rdf/2016-06/ome_core/AcquisitionMode#slitScanConfocal">
        <rdf:type rdf:resource="http://www.openmicroscopy.org/rdf/2016-06/ome_core/AcquisitionMode"/>
        <rdfs:label xml:lang="en">slit scan confocal</rdfs:label>
    </owl:NamedIndividual>
    


    <!-- http://www.openmicroscopy.org/rdf/2016-06/ome_core/AcquisitionMode#spectralImaging -->

    <owl:NamedIndividual rdf:about="http://www.openmicroscopy.org/rdf/2016-06/ome_core/AcquisitionMode#spectralImaging">
        <rdf:type rdf:resource="http://www.openmicroscopy.org/rdf/2016-06/ome_core/AcquisitionMode"/>
        <rdfs:label xml:lang="en">spectral imaging</rdfs:label>
    </owl:NamedIndividual>
    


    <!-- http://www.openmicroscopy.org/rdf/2016-06/ome_core/AcquisitionMode#spinningDiskConfocal -->

    <owl:NamedIndividual rdf:about="http://www.openmicroscopy.org/rdf/2016-06/ome_core/AcquisitionMode#spinningDiskConfocal">
        <rdf:type rdf:resource="http://www.openmicroscopy.org/rdf/2016-06/ome_core/AcquisitionMode"/>
        <rdfs:label xml:lang="en">spinning disk confocal</rdfs:label>
    </owl:NamedIndividual>
    


    <!-- http://www.openmicroscopy.org/rdf/2016-06/ome_core/AcquisitionMode#structuredIllumination -->

    <owl:NamedIndividual rdf:about="http://www.openmicroscopy.org/rdf/2016-06/ome_core/AcquisitionMode#structuredIllumination">
        <rdf:type rdf:resource="http://www.openmicroscopy.org/rdf/2016-06/ome_core/AcquisitionMode"/>
        <rdfs:label xml:lang="en">structured illumination</rdfs:label>
    </owl:NamedIndividual>
    


    <!-- http://www.openmicroscopy.org/rdf/2016-06/ome_core/AcquisitionMode#sweptFieldConfocal -->

    <owl:NamedIndividual rdf:about="http://www.openmicroscopy.org/rdf/2016-06/ome_core/AcquisitionMode#sweptFieldConfocal">
        <rdf:type rdf:resource="http://www.openmicroscopy.org/rdf/2016-06/ome_core/AcquisitionMode"/>
        <rdfs:label xml:lang="en">swept field confocal</rdfs:label>
    </owl:NamedIndividual>
    


    <!-- http://www.openmicroscopy.org/rdf/2016-06/ome_core/AcquisitionMode#totalInternalReflection -->

    <owl:NamedIndividual rdf:about="http://www.openmicroscopy.org/rdf/2016-06/ome_core/AcquisitionMode#totalInternalReflection">
        <rdf:type rdf:resource="http://www.openmicroscopy.org/rdf/2016-06/ome_core/AcquisitionMode"/>
        <rdfs:label xml:lang="en">total internal reflection</rdfs:label>
    </owl:NamedIndividual>
    


    <!-- http://www.openmicroscopy.org/rdf/2016-06/ome_core/AcquisitionMode#wideField -->

    <owl:NamedIndividual rdf:about="http://www.openmicroscopy.org/rdf/2016-06/ome_core/AcquisitionMode#wideField">
        <rdf:type rdf:resource="http://www.openmicroscopy.org/rdf/2016-06/ome_core/AcquisitionMode"/>
        <rdfs:label xml:lang="en">wide field</rdfs:label>
    </owl:NamedIndividual>
    


    <!-- http://www.openmicroscopy.org/rdf/2016-06/ome_core/ArcType#Hg -->

    <owl:NamedIndividual rdf:about="http://www.openmicroscopy.org/rdf/2016-06/ome_core/ArcType#Hg">
        <rdf:type rdf:resource="http://www.openmicroscopy.org/rdf/2016-06/ome_core/ArcType"/>
        <rdfs:label xml:lang="en">Hg</rdfs:label>
    </owl:NamedIndividual>
    


    <!-- http://www.openmicroscopy.org/rdf/2016-06/ome_core/ArcType#HgXe -->

    <owl:NamedIndividual rdf:about="http://www.openmicroscopy.org/rdf/2016-06/ome_core/ArcType#HgXe">
        <rdf:type rdf:resource="http://www.openmicroscopy.org/rdf/2016-06/ome_core/ArcType"/>
        <rdfs:label xml:lang="en">HgXe</rdfs:label>
    </owl:NamedIndividual>
    


    <!-- http://www.openmicroscopy.org/rdf/2016-06/ome_core/ArcType#Xe -->

    <owl:NamedIndividual rdf:about="http://www.openmicroscopy.org/rdf/2016-06/ome_core/ArcType#Xe">
        <rdf:type rdf:resource="http://www.openmicroscopy.org/rdf/2016-06/ome_core/ArcType"/>
        <rdfs:label xml:lang="en">Xe</rdfs:label>
    </owl:NamedIndividual>
    


    <!-- http://www.openmicroscopy.org/rdf/2016-06/ome_core/Binning#eightXEight -->

    <owl:NamedIndividual rdf:about="http://www.openmicroscopy.org/rdf/2016-06/ome_core/Binning#eightXEight">
        <rdf:type rdf:resource="http://www.openmicroscopy.org/rdf/2016-06/ome_core/Binning"/>
        <rdfs:label xml:lang="en">8x8</rdfs:label>
    </owl:NamedIndividual>
    


    <!-- http://www.openmicroscopy.org/rdf/2016-06/ome_core/Binning#fourXFour -->

    <owl:NamedIndividual rdf:about="http://www.openmicroscopy.org/rdf/2016-06/ome_core/Binning#fourXFour">
        <rdf:type rdf:resource="http://www.openmicroscopy.org/rdf/2016-06/ome_core/Binning"/>
        <rdfs:label xml:lang="en">4x4</rdfs:label>
    </owl:NamedIndividual>
    


    <!-- http://www.openmicroscopy.org/rdf/2016-06/ome_core/Binning#oneXOne -->

    <owl:NamedIndividual rdf:about="http://www.openmicroscopy.org/rdf/2016-06/ome_core/Binning#oneXOne">
        <rdf:type rdf:resource="http://www.openmicroscopy.org/rdf/2016-06/ome_core/Binning"/>
        <rdfs:label xml:lang="en">1x1</rdfs:label>
    </owl:NamedIndividual>
    


    <!-- http://www.openmicroscopy.org/rdf/2016-06/ome_core/Binning#twoXTwo -->

    <owl:NamedIndividual rdf:about="http://www.openmicroscopy.org/rdf/2016-06/ome_core/Binning#twoXTwo">
        <rdf:type rdf:resource="http://www.openmicroscopy.org/rdf/2016-06/ome_core/Binning"/>
        <rdfs:label xml:lang="en">2x2</rdfs:label>
    </owl:NamedIndividual>
    


    <!-- http://www.openmicroscopy.org/rdf/2016-06/ome_core/Compression#bzip2 -->

    <owl:NamedIndividual rdf:about="http://www.openmicroscopy.org/rdf/2016-06/ome_core/Compression#bzip2">
        <rdf:type rdf:resource="http://www.openmicroscopy.org/rdf/2016-06/ome_core/Compression"/>
        <rdfs:label xml:lang="en">bzip2</rdfs:label>
    </owl:NamedIndividual>
    


    <!-- http://www.openmicroscopy.org/rdf/2016-06/ome_core/Compression#none -->

    <owl:NamedIndividual rdf:about="http://www.openmicroscopy.org/rdf/2016-06/ome_core/Compression#none">
        <rdf:type rdf:resource="http://www.openmicroscopy.org/rdf/2016-06/ome_core/Compression"/>
        <rdfs:label xml:lang="en">none</rdfs:label>
    </owl:NamedIndividual>
    


    <!-- http://www.openmicroscopy.org/rdf/2016-06/ome_core/Compression#zlib -->

    <owl:NamedIndividual rdf:about="http://www.openmicroscopy.org/rdf/2016-06/ome_core/Compression#zlib">
        <rdf:type rdf:resource="http://www.openmicroscopy.org/rdf/2016-06/ome_core/Compression"/>
        <rdfs:label xml:lang="en">zlib</rdfs:label>
    </owl:NamedIndividual>
    


    <!-- http://www.openmicroscopy.org/rdf/2016-06/ome_core/ContrastMethod#DIC -->

    <owl:NamedIndividual rdf:about="http://www.openmicroscopy.org/rdf/2016-06/ome_core/ContrastMethod#DIC">
        <rdf:type rdf:resource="http://www.openmicroscopy.org/rdf/2016-06/ome_core/ContrastMethod"/>
        <rdfs:label xml:lang="en">DIC</rdfs:label>
    </owl:NamedIndividual>
    


    <!-- http://www.openmicroscopy.org/rdf/2016-06/ome_core/ContrastMethod#brightfield -->

    <owl:NamedIndividual rdf:about="http://www.openmicroscopy.org/rdf/2016-06/ome_core/ContrastMethod#brightfield">
        <rdf:type rdf:resource="http://www.openmicroscopy.org/rdf/2016-06/ome_core/ContrastMethod"/>
        <rdfs:label xml:lang="en">brightfield</rdfs:label>
    </owl:NamedIndividual>
    


    <!-- http://www.openmicroscopy.org/rdf/2016-06/ome_core/ContrastMethod#darkfield -->

    <owl:NamedIndividual rdf:about="http://www.openmicroscopy.org/rdf/2016-06/ome_core/ContrastMethod#darkfield">
        <rdf:type rdf:resource="http://www.openmicroscopy.org/rdf/2016-06/ome_core/ContrastMethod"/>
        <rdfs:label xml:lang="en">darkfield</rdfs:label>
    </owl:NamedIndividual>
    


    <!-- http://www.openmicroscopy.org/rdf/2016-06/ome_core/ContrastMethod#fluorescence -->

    <owl:NamedIndividual rdf:about="http://www.openmicroscopy.org/rdf/2016-06/ome_core/ContrastMethod#fluorescence">
        <rdf:type rdf:resource="http://www.openmicroscopy.org/rdf/2016-06/ome_core/ContrastMethod"/>
        <rdfs:label xml:lang="en">fluorescence</rdfs:label>
    </owl:NamedIndividual>
    


    <!-- http://www.openmicroscopy.org/rdf/2016-06/ome_core/ContrastMethod#hoffmanModulation -->

    <owl:NamedIndividual rdf:about="http://www.openmicroscopy.org/rdf/2016-06/ome_core/ContrastMethod#hoffmanModulation">
        <rdf:type rdf:resource="http://www.openmicroscopy.org/rdf/2016-06/ome_core/ContrastMethod"/>
        <rdfs:label xml:lang="en">hoffman modulation</rdfs:label>
    </owl:NamedIndividual>
    


    <!-- http://www.openmicroscopy.org/rdf/2016-06/ome_core/ContrastMethod#obliqueIllumination -->

    <owl:NamedIndividual rdf:about="http://www.openmicroscopy.org/rdf/2016-06/ome_core/ContrastMethod#obliqueIllumination">
        <rdf:type rdf:resource="http://www.openmicroscopy.org/rdf/2016-06/ome_core/ContrastMethod"/>
        <rdfs:label xml:lang="en">oblique illumination</rdfs:label>
    </owl:NamedIndividual>
    


    <!-- http://www.openmicroscopy.org/rdf/2016-06/ome_core/ContrastMethod#phase -->

    <owl:NamedIndividual rdf:about="http://www.openmicroscopy.org/rdf/2016-06/ome_core/ContrastMethod#phase">
        <rdf:type rdf:resource="http://www.openmicroscopy.org/rdf/2016-06/ome_core/ContrastMethod"/>
        <rdfs:label xml:lang="en">phase</rdfs:label>
    </owl:NamedIndividual>
    


    <!-- http://www.openmicroscopy.org/rdf/2016-06/ome_core/ContrastMethod#polarizedLight -->

    <owl:NamedIndividual rdf:about="http://www.openmicroscopy.org/rdf/2016-06/ome_core/ContrastMethod#polarizedLight">
        <rdf:type rdf:resource="http://www.openmicroscopy.org/rdf/2016-06/ome_core/ContrastMethod"/>
        <rdfs:label xml:lang="en">polarized light</rdfs:label>
    </owl:NamedIndividual>
    


    <!-- http://www.openmicroscopy.org/rdf/2016-06/ome_core/Correction#UV -->

    <owl:NamedIndividual rdf:about="http://www.openmicroscopy.org/rdf/2016-06/ome_core/Correction#UV">
        <rdf:type rdf:resource="http://www.openmicroscopy.org/rdf/2016-06/ome_core/Correction"/>
        <rdfs:label xml:lang="en">UV</rdfs:label>
    </owl:NamedIndividual>
    


    <!-- http://www.openmicroscopy.org/rdf/2016-06/ome_core/Correction#achro -->

    <owl:NamedIndividual rdf:about="http://www.openmicroscopy.org/rdf/2016-06/ome_core/Correction#achro">
        <rdf:type rdf:resource="http://www.openmicroscopy.org/rdf/2016-06/ome_core/Correction"/>
        <rdfs:label xml:lang="en">achro</rdfs:label>
    </owl:NamedIndividual>
    


    <!-- http://www.openmicroscopy.org/rdf/2016-06/ome_core/Correction#achromat -->

    <owl:NamedIndividual rdf:about="http://www.openmicroscopy.org/rdf/2016-06/ome_core/Correction#achromat">
        <rdf:type rdf:resource="http://www.openmicroscopy.org/rdf/2016-06/ome_core/Correction"/>
        <rdfs:label xml:lang="en">achromat</rdfs:label>
    </owl:NamedIndividual>
    


    <!-- http://www.openmicroscopy.org/rdf/2016-06/ome_core/Correction#apo -->

    <owl:NamedIndividual rdf:about="http://www.openmicroscopy.org/rdf/2016-06/ome_core/Correction#apo">
        <rdf:type rdf:resource="http://www.openmicroscopy.org/rdf/2016-06/ome_core/Correction"/>
        <rdfs:label xml:lang="en">apo</rdfs:label>
    </owl:NamedIndividual>
    


    <!-- http://www.openmicroscopy.org/rdf/2016-06/ome_core/Correction#fl -->

    <owl:NamedIndividual rdf:about="http://www.openmicroscopy.org/rdf/2016-06/ome_core/Correction#fl">
        <rdf:type rdf:resource="http://www.openmicroscopy.org/rdf/2016-06/ome_core/Correction"/>
        <rdfs:label xml:lang="en">fl</rdfs:label>
    </owl:NamedIndividual>
    


    <!-- http://www.openmicroscopy.org/rdf/2016-06/ome_core/Correction#fluar -->

    <owl:NamedIndividual rdf:about="http://www.openmicroscopy.org/rdf/2016-06/ome_core/Correction#fluar">
        <rdf:type rdf:resource="http://www.openmicroscopy.org/rdf/2016-06/ome_core/Correction"/>
        <rdfs:label xml:lang="en">fluar</rdfs:label>
    </owl:NamedIndividual>
    


    <!-- http://www.openmicroscopy.org/rdf/2016-06/ome_core/Correction#fluor -->

    <owl:NamedIndividual rdf:about="http://www.openmicroscopy.org/rdf/2016-06/ome_core/Correction#fluor">
        <rdf:type rdf:resource="http://www.openmicroscopy.org/rdf/2016-06/ome_core/Correction"/>
        <rdfs:label xml:lang="en">fluor</rdfs:label>
    </owl:NamedIndividual>
    


    <!-- http://www.openmicroscopy.org/rdf/2016-06/ome_core/Correction#fluotar -->

    <owl:NamedIndividual rdf:about="http://www.openmicroscopy.org/rdf/2016-06/ome_core/Correction#fluotar">
        <rdf:type rdf:resource="http://www.openmicroscopy.org/rdf/2016-06/ome_core/Correction"/>
        <rdfs:label xml:lang="en">fluotar</rdfs:label>
    </owl:NamedIndividual>
    


    <!-- http://www.openmicroscopy.org/rdf/2016-06/ome_core/Correction#neofluar -->

    <owl:NamedIndividual rdf:about="http://www.openmicroscopy.org/rdf/2016-06/ome_core/Correction#neofluar">
        <rdf:type rdf:resource="http://www.openmicroscopy.org/rdf/2016-06/ome_core/Correction"/>
        <rdfs:label xml:lang="en">neofluar</rdfs:label>
    </owl:NamedIndividual>
    


    <!-- http://www.openmicroscopy.org/rdf/2016-06/ome_core/Correction#planApo -->

    <owl:NamedIndividual rdf:about="http://www.openmicroscopy.org/rdf/2016-06/ome_core/Correction#planApo">
        <rdf:type rdf:resource="http://www.openmicroscopy.org/rdf/2016-06/ome_core/Correction"/>
        <rdfs:label xml:lang="en">plan apo</rdfs:label>
    </owl:NamedIndividual>
    


    <!-- http://www.openmicroscopy.org/rdf/2016-06/ome_core/Correction#planFluor -->

    <owl:NamedIndividual rdf:about="http://www.openmicroscopy.org/rdf/2016-06/ome_core/Correction#planFluor">
        <rdf:type rdf:resource="http://www.openmicroscopy.org/rdf/2016-06/ome_core/Correction"/>
        <rdfs:label xml:lang="en">plan fluor</rdfs:label>
    </owl:NamedIndividual>
    


    <!-- http://www.openmicroscopy.org/rdf/2016-06/ome_core/Correction#planNeofluar -->

    <owl:NamedIndividual rdf:about="http://www.openmicroscopy.org/rdf/2016-06/ome_core/Correction#planNeofluar">
        <rdf:type rdf:resource="http://www.openmicroscopy.org/rdf/2016-06/ome_core/Correction"/>
        <rdfs:label xml:lang="en">planNeofluar</rdfs:label>
    </owl:NamedIndividual>
    


    <!-- http://www.openmicroscopy.org/rdf/2016-06/ome_core/Correction#superFluor -->

    <owl:NamedIndividual rdf:about="http://www.openmicroscopy.org/rdf/2016-06/ome_core/Correction#superFluor">
        <rdf:type rdf:resource="http://www.openmicroscopy.org/rdf/2016-06/ome_core/Correction"/>
        <rdfs:label xml:lang="en">super fluor</rdfs:label>
    </owl:NamedIndividual>
    


    <!-- http://www.openmicroscopy.org/rdf/2016-06/ome_core/Correction#violetCorrected -->

    <owl:NamedIndividual rdf:about="http://www.openmicroscopy.org/rdf/2016-06/ome_core/Correction#violetCorrected">
        <rdf:type rdf:resource="http://www.openmicroscopy.org/rdf/2016-06/ome_core/Correction"/>
        <rdfs:label xml:lang="en">violet corrected</rdfs:label>
    </owl:NamedIndividual>
    


    <!-- http://www.openmicroscopy.org/rdf/2016-06/ome_core/DetectorType#APD -->

    <owl:NamedIndividual rdf:about="http://www.openmicroscopy.org/rdf/2016-06/ome_core/DetectorType#APD">
        <rdf:type rdf:resource="http://www.openmicroscopy.org/rdf/2016-06/ome_core/DetectorType"/>
        <rdfs:label xml:lang="en">APD</rdfs:label>
    </owl:NamedIndividual>
    


    <!-- http://www.openmicroscopy.org/rdf/2016-06/ome_core/DetectorType#CCD -->

    <owl:NamedIndividual rdf:about="http://www.openmicroscopy.org/rdf/2016-06/ome_core/DetectorType#CCD">
        <rdf:type rdf:resource="http://www.openmicroscopy.org/rdf/2016-06/ome_core/DetectorType"/>
        <rdfs:label xml:lang="en">CCD</rdfs:label>
    </owl:NamedIndividual>
    


    <!-- http://www.openmicroscopy.org/rdf/2016-06/ome_core/DetectorType#CMOS -->

    <owl:NamedIndividual rdf:about="http://www.openmicroscopy.org/rdf/2016-06/ome_core/DetectorType#CMOS">
        <rdf:type rdf:resource="http://www.openmicroscopy.org/rdf/2016-06/ome_core/DetectorType"/>
        <rdfs:label xml:lang="en">CMOS</rdfs:label>
    </owl:NamedIndividual>
    


    <!-- http://www.openmicroscopy.org/rdf/2016-06/ome_core/DetectorType#EBCCD -->

    <owl:NamedIndividual rdf:about="http://www.openmicroscopy.org/rdf/2016-06/ome_core/DetectorType#EBCCD">
        <rdf:type rdf:resource="http://www.openmicroscopy.org/rdf/2016-06/ome_core/DetectorType"/>
        <rdfs:label xml:lang="en">EBCCD</rdfs:label>
    </owl:NamedIndividual>
    


    <!-- http://www.openmicroscopy.org/rdf/2016-06/ome_core/DetectorType#EMCCD -->

    <owl:NamedIndividual rdf:about="http://www.openmicroscopy.org/rdf/2016-06/ome_core/DetectorType#EMCCD">
        <rdf:type rdf:resource="http://www.openmicroscopy.org/rdf/2016-06/ome_core/DetectorType"/>
        <rdfs:label xml:lang="en">EMCCD</rdfs:label>
    </owl:NamedIndividual>
    


    <!-- http://www.openmicroscopy.org/rdf/2016-06/ome_core/DetectorType#FTIR -->

    <owl:NamedIndividual rdf:about="http://www.openmicroscopy.org/rdf/2016-06/ome_core/DetectorType#FTIR">
        <rdf:type rdf:resource="http://www.openmicroscopy.org/rdf/2016-06/ome_core/DetectorType"/>
        <rdfs:label xml:lang="en">FTIR</rdfs:label>
    </owl:NamedIndividual>
    


    <!-- http://www.openmicroscopy.org/rdf/2016-06/ome_core/DetectorType#PMT -->

    <owl:NamedIndividual rdf:about="http://www.openmicroscopy.org/rdf/2016-06/ome_core/DetectorType#PMT">
        <rdf:type rdf:resource="http://www.openmicroscopy.org/rdf/2016-06/ome_core/DetectorType"/>
        <rdfs:label xml:lang="en">PMT</rdfs:label>
    </owl:NamedIndividual>
    


    <!-- http://www.openmicroscopy.org/rdf/2016-06/ome_core/DetectorType#analogVideo -->

    <owl:NamedIndividual rdf:about="http://www.openmicroscopy.org/rdf/2016-06/ome_core/DetectorType#analogVideo">
        <rdf:type rdf:resource="http://www.openmicroscopy.org/rdf/2016-06/ome_core/DetectorType"/>
        <rdfs:label xml:lang="en">analog video</rdfs:label>
    </owl:NamedIndividual>
    


    <!-- http://www.openmicroscopy.org/rdf/2016-06/ome_core/DetectorType#correlationSpectroscopy -->

    <owl:NamedIndividual rdf:about="http://www.openmicroscopy.org/rdf/2016-06/ome_core/DetectorType#correlationSpectroscopy">
        <rdf:type rdf:resource="http://www.openmicroscopy.org/rdf/2016-06/ome_core/DetectorType"/>
        <rdfs:label xml:lang="en">correlation spectroscopy</rdfs:label>
    </owl:NamedIndividual>
    


    <!-- http://www.openmicroscopy.org/rdf/2016-06/ome_core/DetectorType#intensifiedCCD -->

    <owl:NamedIndividual rdf:about="http://www.openmicroscopy.org/rdf/2016-06/ome_core/DetectorType#intensifiedCCD">
        <rdf:type rdf:resource="http://www.openmicroscopy.org/rdf/2016-06/ome_core/DetectorType"/>
        <rdfs:label xml:lang="en">intensified CCD</rdfs:label>
    </owl:NamedIndividual>
    


    <!-- http://www.openmicroscopy.org/rdf/2016-06/ome_core/DetectorType#lifetimeImaging -->

    <owl:NamedIndividual rdf:about="http://www.openmicroscopy.org/rdf/2016-06/ome_core/DetectorType#lifetimeImaging">
        <rdf:type rdf:resource="http://www.openmicroscopy.org/rdf/2016-06/ome_core/DetectorType"/>
        <rdfs:label xml:lang="en">lifetime imaging</rdfs:label>
    </owl:NamedIndividual>
    


    <!-- http://www.openmicroscopy.org/rdf/2016-06/ome_core/DetectorType#photodiode -->

    <owl:NamedIndividual rdf:about="http://www.openmicroscopy.org/rdf/2016-06/ome_core/DetectorType#photodiode">
        <rdf:type rdf:resource="http://www.openmicroscopy.org/rdf/2016-06/ome_core/DetectorType"/>
        <rdfs:label xml:lang="en">photodiode</rdfs:label>
    </owl:NamedIndividual>
    


    <!-- http://www.openmicroscopy.org/rdf/2016-06/ome_core/DetectorType#spectroscopy -->

    <owl:NamedIndividual rdf:about="http://www.openmicroscopy.org/rdf/2016-06/ome_core/DetectorType#spectroscopy">
        <rdf:type rdf:resource="http://www.openmicroscopy.org/rdf/2016-06/ome_core/DetectorType"/>
        <rdfs:label xml:lang="en">spectroscopy</rdfs:label>
    </owl:NamedIndividual>
    


    <!-- http://www.openmicroscopy.org/rdf/2016-06/ome_core/DimensionOrder#xyctz -->

    <owl:NamedIndividual rdf:about="http://www.openmicroscopy.org/rdf/2016-06/ome_core/DimensionOrder#xyctz">
        <rdf:type rdf:resource="http://www.openmicroscopy.org/rdf/2016-06/ome_core/DimensionOrder"/>
        <rdfs:label xml:lang="en">xyctz</rdfs:label>
    </owl:NamedIndividual>
    


    <!-- http://www.openmicroscopy.org/rdf/2016-06/ome_core/DimensionOrder#xyczt -->

    <owl:NamedIndividual rdf:about="http://www.openmicroscopy.org/rdf/2016-06/ome_core/DimensionOrder#xyczt">
        <rdf:type rdf:resource="http://www.openmicroscopy.org/rdf/2016-06/ome_core/DimensionOrder"/>
        <rdfs:label xml:lang="en">xyczt</rdfs:label>
    </owl:NamedIndividual>
    


    <!-- http://www.openmicroscopy.org/rdf/2016-06/ome_core/DimensionOrder#xytcz -->

    <owl:NamedIndividual rdf:about="http://www.openmicroscopy.org/rdf/2016-06/ome_core/DimensionOrder#xytcz">
        <rdf:type rdf:resource="http://www.openmicroscopy.org/rdf/2016-06/ome_core/DimensionOrder"/>
        <rdfs:label xml:lang="en">xytcz</rdfs:label>
    </owl:NamedIndividual>
    


    <!-- http://www.openmicroscopy.org/rdf/2016-06/ome_core/DimensionOrder#xytzc -->

    <owl:NamedIndividual rdf:about="http://www.openmicroscopy.org/rdf/2016-06/ome_core/DimensionOrder#xytzc">
        <rdf:type rdf:resource="http://www.openmicroscopy.org/rdf/2016-06/ome_core/DimensionOrder"/>
        <rdfs:label xml:lang="en">xytzc</rdfs:label>
    </owl:NamedIndividual>
    


    <!-- http://www.openmicroscopy.org/rdf/2016-06/ome_core/DimensionOrder#xyzct -->

    <owl:NamedIndividual rdf:about="http://www.openmicroscopy.org/rdf/2016-06/ome_core/DimensionOrder#xyzct">
        <rdf:type rdf:resource="http://www.openmicroscopy.org/rdf/2016-06/ome_core/DimensionOrder"/>
        <rdfs:label xml:lang="en">xyzct</rdfs:label>
    </owl:NamedIndividual>
    


    <!-- http://www.openmicroscopy.org/rdf/2016-06/ome_core/DimensionOrder#xyztc -->

    <owl:NamedIndividual rdf:about="http://www.openmicroscopy.org/rdf/2016-06/ome_core/DimensionOrder#xyztc">
        <rdf:type rdf:resource="http://www.openmicroscopy.org/rdf/2016-06/ome_core/DimensionOrder"/>
        <rdfs:label xml:lang="en">xyztc</rdfs:label>
    </owl:NamedIndividual>
    


    <!-- http://www.openmicroscopy.org/rdf/2016-06/ome_core/ExperimentType#FISH -->

    <owl:NamedIndividual rdf:about="http://www.openmicroscopy.org/rdf/2016-06/ome_core/ExperimentType#FISH">
        <rdf:type rdf:resource="http://www.openmicroscopy.org/rdf/2016-06/ome_core/ExperimentType"/>
        <rdfs:label xml:lang="en">FISH</rdfs:label>
    </owl:NamedIndividual>
    


    <!-- http://www.openmicroscopy.org/rdf/2016-06/ome_core/ExperimentType#FP -->

    <owl:NamedIndividual rdf:about="http://www.openmicroscopy.org/rdf/2016-06/ome_core/ExperimentType#FP">
        <rdf:type rdf:resource="http://www.openmicroscopy.org/rdf/2016-06/ome_core/ExperimentType"/>
        <rdfs:label xml:lang="en">FP</rdfs:label>
    </owl:NamedIndividual>
    


    <!-- http://www.openmicroscopy.org/rdf/2016-06/ome_core/ExperimentType#FRET -->

    <owl:NamedIndividual rdf:about="http://www.openmicroscopy.org/rdf/2016-06/ome_core/ExperimentType#FRET">
        <rdf:type rdf:resource="http://www.openmicroscopy.org/rdf/2016-06/ome_core/ExperimentType"/>
        <rdfs:label xml:lang="en">FRET</rdfs:label>
    </owl:NamedIndividual>
    


    <!-- http://www.openmicroscopy.org/rdf/2016-06/ome_core/ExperimentType#PGIDocumentation -->

    <owl:NamedIndividual rdf:about="http://www.openmicroscopy.org/rdf/2016-06/ome_core/ExperimentType#PGIDocumentation">
        <rdf:type rdf:resource="http://www.openmicroscopy.org/rdf/2016-06/ome_core/ExperimentType"/>
        <rdfs:label xml:lang="en">PGI documentation</rdfs:label>
    </owl:NamedIndividual>
    


    <!-- http://www.openmicroscopy.org/rdf/2016-06/ome_core/ExperimentType#SPIM -->

    <owl:NamedIndividual rdf:about="http://www.openmicroscopy.org/rdf/2016-06/ome_core/ExperimentType#SPIM">
        <rdf:type rdf:resource="http://www.openmicroscopy.org/rdf/2016-06/ome_core/ExperimentType"/>
        <rdfs:label xml:lang="en">SPIM</rdfs:label>
    </owl:NamedIndividual>
    


    <!-- http://www.openmicroscopy.org/rdf/2016-06/ome_core/ExperimentType#colocalization -->

    <owl:NamedIndividual rdf:about="http://www.openmicroscopy.org/rdf/2016-06/ome_core/ExperimentType#colocalization">
        <rdf:type rdf:resource="http://www.openmicroscopy.org/rdf/2016-06/ome_core/ExperimentType"/>
        <rdfs:label xml:lang="en">colocalization</rdfs:label>
    </owl:NamedIndividual>
    


    <!-- http://www.openmicroscopy.org/rdf/2016-06/ome_core/ExperimentType#electrophysiology -->

    <owl:NamedIndividual rdf:about="http://www.openmicroscopy.org/rdf/2016-06/ome_core/ExperimentType#electrophysiology">
        <rdf:type rdf:resource="http://www.openmicroscopy.org/rdf/2016-06/ome_core/ExperimentType"/>
        <rdfs:label xml:lang="en">electrophysiology</rdfs:label>
    </owl:NamedIndividual>
    


    <!-- http://www.openmicroscopy.org/rdf/2016-06/ome_core/ExperimentType#fluorescenceLifetime -->

    <owl:NamedIndividual rdf:about="http://www.openmicroscopy.org/rdf/2016-06/ome_core/ExperimentType#fluorescenceLifetime">
        <rdf:type rdf:resource="http://www.openmicroscopy.org/rdf/2016-06/ome_core/ExperimentType"/>
        <rdfs:label xml:lang="en">fluorescence lifetime</rdfs:label>
    </owl:NamedIndividual>
    


    <!-- http://www.openmicroscopy.org/rdf/2016-06/ome_core/ExperimentType#fourDPlus -->

    <owl:NamedIndividual rdf:about="http://www.openmicroscopy.org/rdf/2016-06/ome_core/ExperimentType#fourDPlus">
        <rdf:type rdf:resource="http://www.openmicroscopy.org/rdf/2016-06/ome_core/ExperimentType"/>
        <rdfs:label xml:lang="en">4D plus</rdfs:label>
    </owl:NamedIndividual>
    


    <!-- http://www.openmicroscopy.org/rdf/2016-06/ome_core/ExperimentType#immunocytochemistry -->

    <owl:NamedIndividual rdf:about="http://www.openmicroscopy.org/rdf/2016-06/ome_core/ExperimentType#immunocytochemistry">
        <rdf:type rdf:resource="http://www.openmicroscopy.org/rdf/2016-06/ome_core/ExperimentType"/>
        <rdfs:label xml:lang="en">immunocytochemistry</rdfs:label>
    </owl:NamedIndividual>
    


    <!-- http://www.openmicroscopy.org/rdf/2016-06/ome_core/ExperimentType#immunofluorescence -->

    <owl:NamedIndividual rdf:about="http://www.openmicroscopy.org/rdf/2016-06/ome_core/ExperimentType#immunofluorescence">
        <rdf:type rdf:resource="http://www.openmicroscopy.org/rdf/2016-06/ome_core/ExperimentType"/>
        <rdfs:label xml:lang="en">immunofluorescence</rdfs:label>
    </owl:NamedIndividual>
    


    <!-- http://www.openmicroscopy.org/rdf/2016-06/ome_core/ExperimentType#ionImaging -->

    <owl:NamedIndividual rdf:about="http://www.openmicroscopy.org/rdf/2016-06/ome_core/ExperimentType#ionImaging">
        <rdf:type rdf:resource="http://www.openmicroscopy.org/rdf/2016-06/ome_core/ExperimentType"/>
        <rdfs:label xml:lang="en">ion imaging</rdfs:label>
    </owl:NamedIndividual>
    


    <!-- http://www.openmicroscopy.org/rdf/2016-06/ome_core/ExperimentType#photoablation -->

    <owl:NamedIndividual rdf:about="http://www.openmicroscopy.org/rdf/2016-06/ome_core/ExperimentType#photoablation">
        <rdf:type rdf:resource="http://www.openmicroscopy.org/rdf/2016-06/ome_core/ExperimentType"/>
        <rdfs:label xml:lang="en">photoablation</rdfs:label>
    </owl:NamedIndividual>
    


    <!-- http://www.openmicroscopy.org/rdf/2016-06/ome_core/ExperimentType#photoactivation -->

    <owl:NamedIndividual rdf:about="http://www.openmicroscopy.org/rdf/2016-06/ome_core/ExperimentType#photoactivation">
        <rdf:type rdf:resource="http://www.openmicroscopy.org/rdf/2016-06/ome_core/ExperimentType"/>
        <rdfs:label xml:lang="en">photoactivation</rdfs:label>
    </owl:NamedIndividual>
    


    <!-- http://www.openmicroscopy.org/rdf/2016-06/ome_core/ExperimentType#photobleaching -->

    <owl:NamedIndividual rdf:about="http://www.openmicroscopy.org/rdf/2016-06/ome_core/ExperimentType#photobleaching">
        <rdf:type rdf:resource="http://www.openmicroscopy.org/rdf/2016-06/ome_core/ExperimentType"/>
        <rdfs:label xml:lang="en">photobleaching</rdfs:label>
    </owl:NamedIndividual>
    


    <!-- http://www.openmicroscopy.org/rdf/2016-06/ome_core/ExperimentType#screen -->

    <owl:NamedIndividual rdf:about="http://www.openmicroscopy.org/rdf/2016-06/ome_core/ExperimentType#screen">
        <rdf:type rdf:resource="http://www.openmicroscopy.org/rdf/2016-06/ome_core/ExperimentType"/>
        <rdfs:label xml:lang="en">screen</rdfs:label>
    </owl:NamedIndividual>
    


    <!-- http://www.openmicroscopy.org/rdf/2016-06/ome_core/ExperimentType#spectralImaging -->

    <owl:NamedIndividual rdf:about="http://www.openmicroscopy.org/rdf/2016-06/ome_core/ExperimentType#spectralImaging">
        <rdf:type rdf:resource="http://www.openmicroscopy.org/rdf/2016-06/ome_core/ExperimentType"/>
        <rdfs:label xml:lang="en">spectral imaging</rdfs:label>
    </owl:NamedIndividual>
    


    <!-- http://www.openmicroscopy.org/rdf/2016-06/ome_core/ExperimentType#timeLapse -->

    <owl:NamedIndividual rdf:about="http://www.openmicroscopy.org/rdf/2016-06/ome_core/ExperimentType#timeLapse">
        <rdf:type rdf:resource="http://www.openmicroscopy.org/rdf/2016-06/ome_core/ExperimentType"/>
        <rdfs:label xml:lang="en">time lapse</rdfs:label>
    </owl:NamedIndividual>
    


    <!-- http://www.openmicroscopy.org/rdf/2016-06/ome_core/FilamentType#Halogen -->

    <owl:NamedIndividual rdf:about="http://www.openmicroscopy.org/rdf/2016-06/ome_core/FilamentType#Halogen">
        <rdf:type rdf:resource="http://www.openmicroscopy.org/rdf/2016-06/ome_core/FilamentType"/>
        <rdfs:label xml:lang="en">Halogen</rdfs:label>
    </owl:NamedIndividual>
    


    <!-- http://www.openmicroscopy.org/rdf/2016-06/ome_core/FilamentType#Incandescent -->

    <owl:NamedIndividual rdf:about="http://www.openmicroscopy.org/rdf/2016-06/ome_core/FilamentType#Incandescent">
        <rdf:type rdf:resource="http://www.openmicroscopy.org/rdf/2016-06/ome_core/FilamentType"/>
        <rdfs:label xml:lang="en">Incandescent</rdfs:label>
    </owl:NamedIndividual>
    


    <!-- http://www.openmicroscopy.org/rdf/2016-06/ome_core/FillRule#evenOdd -->

    <owl:NamedIndividual rdf:about="http://www.openmicroscopy.org/rdf/2016-06/ome_core/FillRule#evenOdd">
        <rdf:type rdf:resource="http://www.openmicroscopy.org/rdf/2016-06/ome_core/FillRule"/>
        <rdfs:label xml:lang="en">even odd</rdfs:label>
    </owl:NamedIndividual>
    


    <!-- http://www.openmicroscopy.org/rdf/2016-06/ome_core/FillRule#nonZero -->

    <owl:NamedIndividual rdf:about="http://www.openmicroscopy.org/rdf/2016-06/ome_core/FillRule#nonZero">
        <rdf:type rdf:resource="http://www.openmicroscopy.org/rdf/2016-06/ome_core/FillRule"/>
        <rdfs:label xml:lang="en">non zero</rdfs:label>
    </owl:NamedIndividual>
    


    <!-- http://www.openmicroscopy.org/rdf/2016-06/ome_core/FilterType#bandPass -->

    <owl:NamedIndividual rdf:about="http://www.openmicroscopy.org/rdf/2016-06/ome_core/FilterType#bandPass">
        <rdf:type rdf:resource="http://www.openmicroscopy.org/rdf/2016-06/ome_core/FilterType"/>
        <rdfs:label xml:lang="en">band pass</rdfs:label>
    </owl:NamedIndividual>
    


    <!-- http://www.openmicroscopy.org/rdf/2016-06/ome_core/FilterType#dichroic -->

    <owl:NamedIndividual rdf:about="http://www.openmicroscopy.org/rdf/2016-06/ome_core/FilterType#dichroic">
        <rdf:type rdf:resource="http://www.openmicroscopy.org/rdf/2016-06/ome_core/FilterType"/>
        <rdfs:label xml:lang="en">dichroic</rdfs:label>
    </owl:NamedIndividual>
    


    <!-- http://www.openmicroscopy.org/rdf/2016-06/ome_core/FilterType#longPass -->

    <owl:NamedIndividual rdf:about="http://www.openmicroscopy.org/rdf/2016-06/ome_core/FilterType#longPass">
        <rdf:type rdf:resource="http://www.openmicroscopy.org/rdf/2016-06/ome_core/FilterType"/>
        <rdfs:label xml:lang="en">long pass</rdfs:label>
    </owl:NamedIndividual>
    


    <!-- http://www.openmicroscopy.org/rdf/2016-06/ome_core/FilterType#multiPass -->

    <owl:NamedIndividual rdf:about="http://www.openmicroscopy.org/rdf/2016-06/ome_core/FilterType#multiPass">
        <rdf:type rdf:resource="http://www.openmicroscopy.org/rdf/2016-06/ome_core/FilterType"/>
        <rdfs:label xml:lang="en">multi pass</rdfs:label>
    </owl:NamedIndividual>
    


    <!-- http://www.openmicroscopy.org/rdf/2016-06/ome_core/FilterType#neutralDensity -->

    <owl:NamedIndividual rdf:about="http://www.openmicroscopy.org/rdf/2016-06/ome_core/FilterType#neutralDensity">
        <rdf:type rdf:resource="http://www.openmicroscopy.org/rdf/2016-06/ome_core/FilterType"/>
        <rdfs:label xml:lang="en">neutral density</rdfs:label>
    </owl:NamedIndividual>
    


    <!-- http://www.openmicroscopy.org/rdf/2016-06/ome_core/FilterType#shortPass -->

    <owl:NamedIndividual rdf:about="http://www.openmicroscopy.org/rdf/2016-06/ome_core/FilterType#shortPass">
        <rdf:type rdf:resource="http://www.openmicroscopy.org/rdf/2016-06/ome_core/FilterType"/>
        <rdfs:label xml:lang="en">short pass</rdfs:label>
    </owl:NamedIndividual>
    


    <!-- http://www.openmicroscopy.org/rdf/2016-06/ome_core/FilterType#tuneable -->

    <owl:NamedIndividual rdf:about="http://www.openmicroscopy.org/rdf/2016-06/ome_core/FilterType#tuneable">
        <rdf:type rdf:resource="http://www.openmicroscopy.org/rdf/2016-06/ome_core/FilterType"/>
        <rdfs:label xml:lang="en">tuneable</rdfs:label>
    </owl:NamedIndividual>
    


    <!-- http://www.openmicroscopy.org/rdf/2016-06/ome_core/FontFamily#cursive -->

    <owl:NamedIndividual rdf:about="http://www.openmicroscopy.org/rdf/2016-06/ome_core/FontFamily#cursive">
        <rdf:type rdf:resource="http://www.openmicroscopy.org/rdf/2016-06/ome_core/FontFamily"/>
        <rdfs:label xml:lang="en">cursive</rdfs:label>
    </owl:NamedIndividual>
    


    <!-- http://www.openmicroscopy.org/rdf/2016-06/ome_core/FontFamily#fantasy -->

    <owl:NamedIndividual rdf:about="http://www.openmicroscopy.org/rdf/2016-06/ome_core/FontFamily#fantasy">
        <rdf:type rdf:resource="http://www.openmicroscopy.org/rdf/2016-06/ome_core/FontFamily"/>
        <rdfs:label xml:lang="en">fantasy</rdfs:label>
    </owl:NamedIndividual>
    


    <!-- http://www.openmicroscopy.org/rdf/2016-06/ome_core/FontFamily#monospace -->

    <owl:NamedIndividual rdf:about="http://www.openmicroscopy.org/rdf/2016-06/ome_core/FontFamily#monospace">
        <rdf:type rdf:resource="http://www.openmicroscopy.org/rdf/2016-06/ome_core/FontFamily"/>
        <rdfs:label xml:lang="en">monospace</rdfs:label>
    </owl:NamedIndividual>
    


    <!-- http://www.openmicroscopy.org/rdf/2016-06/ome_core/FontFamily#sansSerif -->

    <owl:NamedIndividual rdf:about="http://www.openmicroscopy.org/rdf/2016-06/ome_core/FontFamily#sansSerif">
        <rdf:type rdf:resource="http://www.openmicroscopy.org/rdf/2016-06/ome_core/FontFamily"/>
        <rdfs:label xml:lang="en">sans-serif</rdfs:label>
    </owl:NamedIndividual>
    


    <!-- http://www.openmicroscopy.org/rdf/2016-06/ome_core/FontFamily#serif -->

    <owl:NamedIndividual rdf:about="http://www.openmicroscopy.org/rdf/2016-06/ome_core/FontFamily#serif">
        <rdf:type rdf:resource="http://www.openmicroscopy.org/rdf/2016-06/ome_core/FontFamily"/>
        <rdfs:label xml:lang="en">serif</rdfs:label>
    </owl:NamedIndividual>
    


    <!-- http://www.openmicroscopy.org/rdf/2016-06/ome_core/FontStyle#bold -->

    <owl:NamedIndividual rdf:about="http://www.openmicroscopy.org/rdf/2016-06/ome_core/FontStyle#bold">
        <rdf:type rdf:resource="http://www.openmicroscopy.org/rdf/2016-06/ome_core/FontStyle"/>
        <rdfs:label xml:lang="en">bold</rdfs:label>
    </owl:NamedIndividual>
    


    <!-- http://www.openmicroscopy.org/rdf/2016-06/ome_core/FontStyle#boldItalic -->

    <owl:NamedIndividual rdf:about="http://www.openmicroscopy.org/rdf/2016-06/ome_core/FontStyle#boldItalic">
        <rdf:type rdf:resource="http://www.openmicroscopy.org/rdf/2016-06/ome_core/FontStyle"/>
        <rdfs:label xml:lang="en">bold italic</rdfs:label>
    </owl:NamedIndividual>
    


    <!-- http://www.openmicroscopy.org/rdf/2016-06/ome_core/FontStyle#italic -->

    <owl:NamedIndividual rdf:about="http://www.openmicroscopy.org/rdf/2016-06/ome_core/FontStyle#italic">
        <rdf:type rdf:resource="http://www.openmicroscopy.org/rdf/2016-06/ome_core/FontStyle"/>
        <rdfs:label xml:lang="en">italic</rdfs:label>
    </owl:NamedIndividual>
    


    <!-- http://www.openmicroscopy.org/rdf/2016-06/ome_core/FontStyle#normal -->

    <owl:NamedIndividual rdf:about="http://www.openmicroscopy.org/rdf/2016-06/ome_core/FontStyle#normal">
        <rdf:type rdf:resource="http://www.openmicroscopy.org/rdf/2016-06/ome_core/FontStyle"/>
        <rdfs:label xml:lang="en">normal</rdfs:label>
    </owl:NamedIndividual>
    


    <!-- http://www.openmicroscopy.org/rdf/2016-06/ome_core/IlluminationType#epifluorescence -->

    <owl:NamedIndividual rdf:about="http://www.openmicroscopy.org/rdf/2016-06/ome_core/IlluminationType#epifluorescence">
        <rdf:type rdf:resource="http://www.openmicroscopy.org/rdf/2016-06/ome_core/IlluminationType"/>
        <rdfs:label xml:lang="en">epifluorescence</rdfs:label>
    </owl:NamedIndividual>
    


    <!-- http://www.openmicroscopy.org/rdf/2016-06/ome_core/IlluminationType#nonLinear -->

    <owl:NamedIndividual rdf:about="http://www.openmicroscopy.org/rdf/2016-06/ome_core/IlluminationType#nonLinear">
        <rdf:type rdf:resource="http://www.openmicroscopy.org/rdf/2016-06/ome_core/IlluminationType"/>
        <rdfs:label xml:lang="en">non linear</rdfs:label>
    </owl:NamedIndividual>
    


    <!-- http://www.openmicroscopy.org/rdf/2016-06/ome_core/IlluminationType#oblique -->

    <owl:NamedIndividual rdf:about="http://www.openmicroscopy.org/rdf/2016-06/ome_core/IlluminationType#oblique">
        <rdf:type rdf:resource="http://www.openmicroscopy.org/rdf/2016-06/ome_core/IlluminationType"/>
        <rdfs:label xml:lang="en">oblique</rdfs:label>
    </owl:NamedIndividual>
    


    <!-- http://www.openmicroscopy.org/rdf/2016-06/ome_core/IlluminationType#transmitted -->

    <owl:NamedIndividual rdf:about="http://www.openmicroscopy.org/rdf/2016-06/ome_core/IlluminationType#transmitted">
        <rdf:type rdf:resource="http://www.openmicroscopy.org/rdf/2016-06/ome_core/IlluminationType"/>
        <rdfs:label xml:lang="en">transmitted</rdfs:label>
    </owl:NamedIndividual>
    


    <!-- http://www.openmicroscopy.org/rdf/2016-06/ome_core/Immersion#air -->

    <owl:NamedIndividual rdf:about="http://www.openmicroscopy.org/rdf/2016-06/ome_core/Immersion#air">
        <rdf:type rdf:resource="http://www.openmicroscopy.org/rdf/2016-06/ome_core/Immersion"/>
        <rdfs:label xml:lang="en">air</rdfs:label>
    </owl:NamedIndividual>
    


    <!-- http://www.openmicroscopy.org/rdf/2016-06/ome_core/Immersion#glycerol -->

    <owl:NamedIndividual rdf:about="http://www.openmicroscopy.org/rdf/2016-06/ome_core/Immersion#glycerol">
        <rdf:type rdf:resource="http://www.openmicroscopy.org/rdf/2016-06/ome_core/Immersion"/>
        <rdfs:label xml:lang="en">glycerol</rdfs:label>
    </owl:NamedIndividual>
    


    <!-- http://www.openmicroscopy.org/rdf/2016-06/ome_core/Immersion#multi -->

    <owl:NamedIndividual rdf:about="http://www.openmicroscopy.org/rdf/2016-06/ome_core/Immersion#multi">
        <rdf:type rdf:resource="http://www.openmicroscopy.org/rdf/2016-06/ome_core/Immersion"/>
        <rdfs:label xml:lang="en">multi</rdfs:label>
    </owl:NamedIndividual>
    


    <!-- http://www.openmicroscopy.org/rdf/2016-06/ome_core/Immersion#oil -->

    <owl:NamedIndividual rdf:about="http://www.openmicroscopy.org/rdf/2016-06/ome_core/Immersion#oil">
        <rdf:type rdf:resource="http://www.openmicroscopy.org/rdf/2016-06/ome_core/Immersion"/>
        <rdfs:label xml:lang="en">oil</rdfs:label>
    </owl:NamedIndividual>
    


    <!-- http://www.openmicroscopy.org/rdf/2016-06/ome_core/Immersion#water -->

    <owl:NamedIndividual rdf:about="http://www.openmicroscopy.org/rdf/2016-06/ome_core/Immersion#water">
        <rdf:type rdf:resource="http://www.openmicroscopy.org/rdf/2016-06/ome_core/Immersion"/>
        <rdfs:label xml:lang="en">water</rdfs:label>
    </owl:NamedIndividual>
    


    <!-- http://www.openmicroscopy.org/rdf/2016-06/ome_core/Immersion#waterDipping -->

    <owl:NamedIndividual rdf:about="http://www.openmicroscopy.org/rdf/2016-06/ome_core/Immersion#waterDipping">
        <rdf:type rdf:resource="http://www.openmicroscopy.org/rdf/2016-06/ome_core/Immersion"/>
        <rdfs:label xml:lang="en">water dipping</rdfs:label>
    </owl:NamedIndividual>
    


    <!-- http://www.openmicroscopy.org/rdf/2016-06/ome_core/Laser/dye -->

    <owl:NamedIndividual rdf:about="http://www.openmicroscopy.org/rdf/2016-06/ome_core/Laser/dye">
        <rdf:type rdf:resource="http://www.openmicroscopy.org/rdf/2016-06/ome_core/Laser"/>
        <rdfs:label xml:lang="en">dye</rdfs:label>
    </owl:NamedIndividual>
    


    <!-- http://www.openmicroscopy.org/rdf/2016-06/ome_core/Laser/excimer -->

    <owl:NamedIndividual rdf:about="http://www.openmicroscopy.org/rdf/2016-06/ome_core/Laser/excimer">
        <rdf:type rdf:resource="http://www.openmicroscopy.org/rdf/2016-06/ome_core/Laser"/>
        <rdfs:label xml:lang="en">excimer</rdfs:label>
    </owl:NamedIndividual>
    


    <!-- http://www.openmicroscopy.org/rdf/2016-06/ome_core/Laser/freeElectron -->

    <owl:NamedIndividual rdf:about="http://www.openmicroscopy.org/rdf/2016-06/ome_core/Laser/freeElectron">
        <rdf:type rdf:resource="http://www.openmicroscopy.org/rdf/2016-06/ome_core/Laser"/>
        <rdfs:label xml:lang="en">free electron</rdfs:label>
    </owl:NamedIndividual>
    


    <!-- http://www.openmicroscopy.org/rdf/2016-06/ome_core/Laser/gas -->

    <owl:NamedIndividual rdf:about="http://www.openmicroscopy.org/rdf/2016-06/ome_core/Laser/gas">
        <rdf:type rdf:resource="http://www.openmicroscopy.org/rdf/2016-06/ome_core/Laser"/>
        <rdfs:label xml:lang="en">gas</rdfs:label>
    </owl:NamedIndividual>
    


    <!-- http://www.openmicroscopy.org/rdf/2016-06/ome_core/Laser/metalVapor -->

    <owl:NamedIndividual rdf:about="http://www.openmicroscopy.org/rdf/2016-06/ome_core/Laser/metalVapor">
        <rdf:type rdf:resource="http://www.openmicroscopy.org/rdf/2016-06/ome_core/Laser"/>
        <rdfs:label xml:lang="en">metal vapor</rdfs:label>
    </owl:NamedIndividual>
    


    <!-- http://www.openmicroscopy.org/rdf/2016-06/ome_core/Laser/semiconductor -->

    <owl:NamedIndividual rdf:about="http://www.openmicroscopy.org/rdf/2016-06/ome_core/Laser/semiconductor">
        <rdf:type rdf:resource="http://www.openmicroscopy.org/rdf/2016-06/ome_core/Laser"/>
        <rdfs:label xml:lang="en">semiconductor</rdfs:label>
    </owl:NamedIndividual>
    


    <!-- http://www.openmicroscopy.org/rdf/2016-06/ome_core/Laser/solidState -->

    <owl:NamedIndividual rdf:about="http://www.openmicroscopy.org/rdf/2016-06/ome_core/Laser/solidState">
        <rdf:type rdf:resource="http://www.openmicroscopy.org/rdf/2016-06/ome_core/Laser"/>
        <rdfs:label xml:lang="en">solid state</rdfs:label>
    </owl:NamedIndividual>
    


    <!-- http://www.openmicroscopy.org/rdf/2016-06/ome_core/LaserMedium#Ag -->

    <owl:NamedIndividual rdf:about="http://www.openmicroscopy.org/rdf/2016-06/ome_core/LaserMedium#Ag">
        <rdf:type rdf:resource="http://www.openmicroscopy.org/rdf/2016-06/ome_core/LaserMedium"/>
        <rdfs:label xml:lang="en">Ag</rdfs:label>
    </owl:NamedIndividual>
    


    <!-- http://www.openmicroscopy.org/rdf/2016-06/ome_core/LaserMedium#Alexandrite -->

    <owl:NamedIndividual rdf:about="http://www.openmicroscopy.org/rdf/2016-06/ome_core/LaserMedium#Alexandrite">
        <rdf:type rdf:resource="http://www.openmicroscopy.org/rdf/2016-06/ome_core/LaserMedium"/>
        <rdfs:label xml:lang="en">Alexandrite</rdfs:label>
    </owl:NamedIndividual>
    


    <!-- http://www.openmicroscopy.org/rdf/2016-06/ome_core/LaserMedium#Ar -->

    <owl:NamedIndividual rdf:about="http://www.openmicroscopy.org/rdf/2016-06/ome_core/LaserMedium#Ar">
        <rdf:type rdf:resource="http://www.openmicroscopy.org/rdf/2016-06/ome_core/LaserMedium"/>
        <rdfs:label xml:lang="en">Ar</rdfs:label>
    </owl:NamedIndividual>
    


    <!-- http://www.openmicroscopy.org/rdf/2016-06/ome_core/LaserMedium#ArCl -->

    <owl:NamedIndividual rdf:about="http://www.openmicroscopy.org/rdf/2016-06/ome_core/LaserMedium#ArCl">
        <rdf:type rdf:resource="http://www.openmicroscopy.org/rdf/2016-06/ome_core/LaserMedium"/>
        <rdfs:label xml:lang="en">ArCl</rdfs:label>
    </owl:NamedIndividual>
    


    <!-- http://www.openmicroscopy.org/rdf/2016-06/ome_core/LaserMedium#ArFl -->

    <owl:NamedIndividual rdf:about="http://www.openmicroscopy.org/rdf/2016-06/ome_core/LaserMedium#ArFl">
        <rdf:type rdf:resource="http://www.openmicroscopy.org/rdf/2016-06/ome_core/LaserMedium"/>
        <rdfs:label xml:lang="en">ArFl</rdfs:label>
    </owl:NamedIndividual>
    


    <!-- http://www.openmicroscopy.org/rdf/2016-06/ome_core/LaserMedium#CO -->

    <owl:NamedIndividual rdf:about="http://www.openmicroscopy.org/rdf/2016-06/ome_core/LaserMedium#CO">
        <rdf:type rdf:resource="http://www.openmicroscopy.org/rdf/2016-06/ome_core/LaserMedium"/>
        <rdfs:label xml:lang="en">CO</rdfs:label>
    </owl:NamedIndividual>
    


    <!-- http://www.openmicroscopy.org/rdf/2016-06/ome_core/LaserMedium#CO2 -->

    <owl:NamedIndividual rdf:about="http://www.openmicroscopy.org/rdf/2016-06/ome_core/LaserMedium#CO2">
        <rdf:type rdf:resource="http://www.openmicroscopy.org/rdf/2016-06/ome_core/LaserMedium"/>
        <rdfs:label xml:lang="en">CO2</rdfs:label>
    </owl:NamedIndividual>
    


    <!-- http://www.openmicroscopy.org/rdf/2016-06/ome_core/LaserMedium#CoumarinC30 -->

    <owl:NamedIndividual rdf:about="http://www.openmicroscopy.org/rdf/2016-06/ome_core/LaserMedium#CoumarinC30">
        <rdf:type rdf:resource="http://www.openmicroscopy.org/rdf/2016-06/ome_core/LaserMedium"/>
        <rdfs:label xml:lang="en">CoumarinC30</rdfs:label>
    </owl:NamedIndividual>
    


    <!-- http://www.openmicroscopy.org/rdf/2016-06/ome_core/LaserMedium#Cu -->

    <owl:NamedIndividual rdf:about="http://www.openmicroscopy.org/rdf/2016-06/ome_core/LaserMedium#Cu">
        <rdf:type rdf:resource="http://www.openmicroscopy.org/rdf/2016-06/ome_core/LaserMedium"/>
        <rdfs:label xml:lang="en">Cu</rdfs:label>
    </owl:NamedIndividual>
    


    <!-- http://www.openmicroscopy.org/rdf/2016-06/ome_core/LaserMedium#EMinus -->

    <owl:NamedIndividual rdf:about="http://www.openmicroscopy.org/rdf/2016-06/ome_core/LaserMedium#EMinus">
        <rdf:type rdf:resource="http://www.openmicroscopy.org/rdf/2016-06/ome_core/LaserMedium"/>
        <rdfs:label xml:lang="en">EMinus</rdfs:label>
    </owl:NamedIndividual>
    


    <!-- http://www.openmicroscopy.org/rdf/2016-06/ome_core/LaserMedium#ErGlass -->

    <owl:NamedIndividual rdf:about="http://www.openmicroscopy.org/rdf/2016-06/ome_core/LaserMedium#ErGlass">
        <rdf:type rdf:resource="http://www.openmicroscopy.org/rdf/2016-06/ome_core/LaserMedium"/>
        <rdfs:label xml:lang="en">ErGlass</rdfs:label>
    </owl:NamedIndividual>
    


    <!-- http://www.openmicroscopy.org/rdf/2016-06/ome_core/LaserMedium#ErYAG -->

    <owl:NamedIndividual rdf:about="http://www.openmicroscopy.org/rdf/2016-06/ome_core/LaserMedium#ErYAG">
        <rdf:type rdf:resource="http://www.openmicroscopy.org/rdf/2016-06/ome_core/LaserMedium"/>
        <rdfs:label xml:lang="en">ErYAG</rdfs:label>
    </owl:NamedIndividual>
    


    <!-- http://www.openmicroscopy.org/rdf/2016-06/ome_core/LaserMedium#GaAlAs -->

    <owl:NamedIndividual rdf:about="http://www.openmicroscopy.org/rdf/2016-06/ome_core/LaserMedium#GaAlAs">
        <rdf:type rdf:resource="http://www.openmicroscopy.org/rdf/2016-06/ome_core/LaserMedium"/>
        <rdfs:label xml:lang="en">GaAlAs</rdfs:label>
    </owl:NamedIndividual>
    


    <!-- http://www.openmicroscopy.org/rdf/2016-06/ome_core/LaserMedium#GaAs -->

    <owl:NamedIndividual rdf:about="http://www.openmicroscopy.org/rdf/2016-06/ome_core/LaserMedium#GaAs">
        <rdf:type rdf:resource="http://www.openmicroscopy.org/rdf/2016-06/ome_core/LaserMedium"/>
        <rdfs:label xml:lang="en">GaAs</rdfs:label>
    </owl:NamedIndividual>
    


    <!-- http://www.openmicroscopy.org/rdf/2016-06/ome_core/LaserMedium#H2O -->

    <owl:NamedIndividual rdf:about="http://www.openmicroscopy.org/rdf/2016-06/ome_core/LaserMedium#H2O">
        <rdf:type rdf:resource="http://www.openmicroscopy.org/rdf/2016-06/ome_core/LaserMedium"/>
        <rdfs:label xml:lang="en">H2O</rdfs:label>
    </owl:NamedIndividual>
    


    <!-- http://www.openmicroscopy.org/rdf/2016-06/ome_core/LaserMedium#HFl -->

    <owl:NamedIndividual rdf:about="http://www.openmicroscopy.org/rdf/2016-06/ome_core/LaserMedium#HFl">
        <rdf:type rdf:resource="http://www.openmicroscopy.org/rdf/2016-06/ome_core/LaserMedium"/>
        <rdfs:label xml:lang="en">HFl</rdfs:label>
    </owl:NamedIndividual>
    


    <!-- http://www.openmicroscopy.org/rdf/2016-06/ome_core/LaserMedium#HeCd -->

    <owl:NamedIndividual rdf:about="http://www.openmicroscopy.org/rdf/2016-06/ome_core/LaserMedium#HeCd">
        <rdf:type rdf:resource="http://www.openmicroscopy.org/rdf/2016-06/ome_core/LaserMedium"/>
        <rdfs:label xml:lang="en">HeCd</rdfs:label>
    </owl:NamedIndividual>
    


    <!-- http://www.openmicroscopy.org/rdf/2016-06/ome_core/LaserMedium#HeNe -->

    <owl:NamedIndividual rdf:about="http://www.openmicroscopy.org/rdf/2016-06/ome_core/LaserMedium#HeNe">
        <rdf:type rdf:resource="http://www.openmicroscopy.org/rdf/2016-06/ome_core/LaserMedium"/>
        <rdfs:label xml:lang="en">HeNe</rdfs:label>
    </owl:NamedIndividual>
    


    <!-- http://www.openmicroscopy.org/rdf/2016-06/ome_core/LaserMedium#HoYAG -->

    <owl:NamedIndividual rdf:about="http://www.openmicroscopy.org/rdf/2016-06/ome_core/LaserMedium#HoYAG">
        <rdf:type rdf:resource="http://www.openmicroscopy.org/rdf/2016-06/ome_core/LaserMedium"/>
        <rdfs:label xml:lang="en">HoYAG</rdfs:label>
    </owl:NamedIndividual>
    


    <!-- http://www.openmicroscopy.org/rdf/2016-06/ome_core/LaserMedium#HoYLF -->

    <owl:NamedIndividual rdf:about="http://www.openmicroscopy.org/rdf/2016-06/ome_core/LaserMedium#HoYLF">
        <rdf:type rdf:resource="http://www.openmicroscopy.org/rdf/2016-06/ome_core/LaserMedium"/>
        <rdfs:label xml:lang="en">HoYLF</rdfs:label>
    </owl:NamedIndividual>
    


    <!-- http://www.openmicroscopy.org/rdf/2016-06/ome_core/LaserMedium#Kr -->

    <owl:NamedIndividual rdf:about="http://www.openmicroscopy.org/rdf/2016-06/ome_core/LaserMedium#Kr">
        <rdf:type rdf:resource="http://www.openmicroscopy.org/rdf/2016-06/ome_core/LaserMedium"/>
        <rdfs:label xml:lang="en">Kr</rdfs:label>
    </owl:NamedIndividual>
    


    <!-- http://www.openmicroscopy.org/rdf/2016-06/ome_core/LaserMedium#KrCl -->

    <owl:NamedIndividual rdf:about="http://www.openmicroscopy.org/rdf/2016-06/ome_core/LaserMedium#KrCl">
        <rdf:type rdf:resource="http://www.openmicroscopy.org/rdf/2016-06/ome_core/LaserMedium"/>
        <rdfs:label xml:lang="en">KrCl</rdfs:label>
    </owl:NamedIndividual>
    


    <!-- http://www.openmicroscopy.org/rdf/2016-06/ome_core/LaserMedium#KrFl -->

    <owl:NamedIndividual rdf:about="http://www.openmicroscopy.org/rdf/2016-06/ome_core/LaserMedium#KrFl">
        <rdf:type rdf:resource="http://www.openmicroscopy.org/rdf/2016-06/ome_core/LaserMedium"/>
        <rdfs:label xml:lang="en">KrFl</rdfs:label>
    </owl:NamedIndividual>
    


    <!-- http://www.openmicroscopy.org/rdf/2016-06/ome_core/LaserMedium#N -->

    <owl:NamedIndividual rdf:about="http://www.openmicroscopy.org/rdf/2016-06/ome_core/LaserMedium#N">
        <rdf:type rdf:resource="http://www.openmicroscopy.org/rdf/2016-06/ome_core/LaserMedium"/>
        <rdfs:label xml:lang="en">N</rdfs:label>
    </owl:NamedIndividual>
    


    <!-- http://www.openmicroscopy.org/rdf/2016-06/ome_core/LaserMedium#NdGlass -->

    <owl:NamedIndividual rdf:about="http://www.openmicroscopy.org/rdf/2016-06/ome_core/LaserMedium#NdGlass">
        <rdf:type rdf:resource="http://www.openmicroscopy.org/rdf/2016-06/ome_core/LaserMedium"/>
        <rdfs:label xml:lang="en">NdGlass</rdfs:label>
    </owl:NamedIndividual>
    


    <!-- http://www.openmicroscopy.org/rdf/2016-06/ome_core/LaserMedium#NdYAG -->

    <owl:NamedIndividual rdf:about="http://www.openmicroscopy.org/rdf/2016-06/ome_core/LaserMedium#NdYAG">
        <rdf:type rdf:resource="http://www.openmicroscopy.org/rdf/2016-06/ome_core/LaserMedium"/>
        <rdfs:label xml:lang="en">NdYAG</rdfs:label>
    </owl:NamedIndividual>
    


    <!-- http://www.openmicroscopy.org/rdf/2016-06/ome_core/LaserMedium#Rhodamine6G -->

    <owl:NamedIndividual rdf:about="http://www.openmicroscopy.org/rdf/2016-06/ome_core/LaserMedium#Rhodamine6G">
        <rdf:type rdf:resource="http://www.openmicroscopy.org/rdf/2016-06/ome_core/LaserMedium"/>
        <rdfs:label xml:lang="en">Rhodamine6G</rdfs:label>
    </owl:NamedIndividual>
    


    <!-- http://www.openmicroscopy.org/rdf/2016-06/ome_core/LaserMedium#Ruby -->

    <owl:NamedIndividual rdf:about="http://www.openmicroscopy.org/rdf/2016-06/ome_core/LaserMedium#Ruby">
        <rdf:type rdf:resource="http://www.openmicroscopy.org/rdf/2016-06/ome_core/LaserMedium"/>
        <rdfs:label xml:lang="en">Ruby</rdfs:label>
    </owl:NamedIndividual>
    


    <!-- http://www.openmicroscopy.org/rdf/2016-06/ome_core/LaserMedium#TiSapphire -->

    <owl:NamedIndividual rdf:about="http://www.openmicroscopy.org/rdf/2016-06/ome_core/LaserMedium#TiSapphire">
        <rdf:type rdf:resource="http://www.openmicroscopy.org/rdf/2016-06/ome_core/LaserMedium"/>
        <rdfs:label xml:lang="en">TiSapphire</rdfs:label>
    </owl:NamedIndividual>
    


    <!-- http://www.openmicroscopy.org/rdf/2016-06/ome_core/LaserMedium#Xe -->

    <owl:NamedIndividual rdf:about="http://www.openmicroscopy.org/rdf/2016-06/ome_core/LaserMedium#Xe">
        <rdf:type rdf:resource="http://www.openmicroscopy.org/rdf/2016-06/ome_core/LaserMedium"/>
        <rdfs:label xml:lang="en">Xe</rdfs:label>
    </owl:NamedIndividual>
    


    <!-- http://www.openmicroscopy.org/rdf/2016-06/ome_core/LaserMedium#XeBr -->

    <owl:NamedIndividual rdf:about="http://www.openmicroscopy.org/rdf/2016-06/ome_core/LaserMedium#XeBr">
        <rdf:type rdf:resource="http://www.openmicroscopy.org/rdf/2016-06/ome_core/LaserMedium"/>
        <rdfs:label xml:lang="en">XeBr</rdfs:label>
    </owl:NamedIndividual>
    


    <!-- http://www.openmicroscopy.org/rdf/2016-06/ome_core/LaserMedium#XeCl -->

    <owl:NamedIndividual rdf:about="http://www.openmicroscopy.org/rdf/2016-06/ome_core/LaserMedium#XeCl">
        <rdf:type rdf:resource="http://www.openmicroscopy.org/rdf/2016-06/ome_core/LaserMedium"/>
        <rdfs:label xml:lang="en">XeCl</rdfs:label>
    </owl:NamedIndividual>
    


    <!-- http://www.openmicroscopy.org/rdf/2016-06/ome_core/LaserMedium#XeFl -->

    <owl:NamedIndividual rdf:about="http://www.openmicroscopy.org/rdf/2016-06/ome_core/LaserMedium#XeFl">
        <rdf:type rdf:resource="http://www.openmicroscopy.org/rdf/2016-06/ome_core/LaserMedium"/>
        <rdfs:label xml:lang="en">XeFl</rdfs:label>
    </owl:NamedIndividual>
    


    <!-- http://www.openmicroscopy.org/rdf/2016-06/ome_core/Marker#arrow -->

    <owl:NamedIndividual rdf:about="http://www.openmicroscopy.org/rdf/2016-06/ome_core/Marker#arrow">
        <rdf:type rdf:resource="http://www.openmicroscopy.org/rdf/2016-06/ome_core/Marker"/>
        <rdfs:label xml:lang="en">arrow</rdfs:label>
    </owl:NamedIndividual>
    


    <!-- http://www.openmicroscopy.org/rdf/2016-06/ome_core/MicrobeamManipuration#FLIP -->

    <owl:NamedIndividual rdf:about="http://www.openmicroscopy.org/rdf/2016-06/ome_core/MicrobeamManipuration#FLIP">
        <rdf:type rdf:resource="http://www.openmicroscopy.org/rdf/2016-06/ome_core/MicrobeamManipuration"/>
        <rdfs:label xml:lang="en">FLIP</rdfs:label>
    </owl:NamedIndividual>
    


    <!-- http://www.openmicroscopy.org/rdf/2016-06/ome_core/MicrobeamManipuration#FRAP -->

    <owl:NamedIndividual rdf:about="http://www.openmicroscopy.org/rdf/2016-06/ome_core/MicrobeamManipuration#FRAP">
        <rdf:type rdf:resource="http://www.openmicroscopy.org/rdf/2016-06/ome_core/MicrobeamManipuration"/>
        <rdfs:label xml:lang="en">FRAP</rdfs:label>
    </owl:NamedIndividual>
    


    <!-- http://www.openmicroscopy.org/rdf/2016-06/ome_core/MicrobeamManipuration#inverseFRAP -->

    <owl:NamedIndividual rdf:about="http://www.openmicroscopy.org/rdf/2016-06/ome_core/MicrobeamManipuration#inverseFRAP">
        <rdf:type rdf:resource="http://www.openmicroscopy.org/rdf/2016-06/ome_core/MicrobeamManipuration"/>
        <rdfs:label xml:lang="en">inverse FRAP</rdfs:label>
    </owl:NamedIndividual>
    


    <!-- http://www.openmicroscopy.org/rdf/2016-06/ome_core/MicrobeamManipuration#opticalTrapping -->

    <owl:NamedIndividual rdf:about="http://www.openmicroscopy.org/rdf/2016-06/ome_core/MicrobeamManipuration#opticalTrapping">
        <rdf:type rdf:resource="http://www.openmicroscopy.org/rdf/2016-06/ome_core/MicrobeamManipuration"/>
        <rdfs:label xml:lang="en">optical trapping</rdfs:label>
    </owl:NamedIndividual>
    


    <!-- http://www.openmicroscopy.org/rdf/2016-06/ome_core/MicrobeamManipuration#photoablation -->

    <owl:NamedIndividual rdf:about="http://www.openmicroscopy.org/rdf/2016-06/ome_core/MicrobeamManipuration#photoablation">
        <rdf:type rdf:resource="http://www.openmicroscopy.org/rdf/2016-06/ome_core/MicrobeamManipuration"/>
        <rdfs:label xml:lang="en">photoablation</rdfs:label>
    </owl:NamedIndividual>
    


    <!-- http://www.openmicroscopy.org/rdf/2016-06/ome_core/MicrobeamManipuration#photoactivation -->

    <owl:NamedIndividual rdf:about="http://www.openmicroscopy.org/rdf/2016-06/ome_core/MicrobeamManipuration#photoactivation">
        <rdf:type rdf:resource="http://www.openmicroscopy.org/rdf/2016-06/ome_core/MicrobeamManipuration"/>
        <rdfs:label xml:lang="en">photoactivation</rdfs:label>
    </owl:NamedIndividual>
    


    <!-- http://www.openmicroscopy.org/rdf/2016-06/ome_core/MicrobeamManipuration#uncaging -->

    <owl:NamedIndividual rdf:about="http://www.openmicroscopy.org/rdf/2016-06/ome_core/MicrobeamManipuration#uncaging">
        <rdf:type rdf:resource="http://www.openmicroscopy.org/rdf/2016-06/ome_core/MicrobeamManipuration"/>
        <rdfs:label xml:lang="en">uncaging</rdfs:label>
    </owl:NamedIndividual>
    


    <!-- http://www.openmicroscopy.org/rdf/2016-06/ome_core/Microscope#dissection -->

    <owl:NamedIndividual rdf:about="http://www.openmicroscopy.org/rdf/2016-06/ome_core/Microscope#dissection">
        <rdf:type rdf:resource="http://www.openmicroscopy.org/rdf/2016-06/ome_core/Microscope"/>
        <rdfs:label xml:lang="en">dissection</rdfs:label>
    </owl:NamedIndividual>
    


    <!-- http://www.openmicroscopy.org/rdf/2016-06/ome_core/Microscope#electrophysiology -->

    <owl:NamedIndividual rdf:about="http://www.openmicroscopy.org/rdf/2016-06/ome_core/Microscope#electrophysiology">
        <rdf:type rdf:resource="http://www.openmicroscopy.org/rdf/2016-06/ome_core/Microscope"/>
        <rdfs:label xml:lang="en">electrophysiology</rdfs:label>
    </owl:NamedIndividual>
    


    <!-- http://www.openmicroscopy.org/rdf/2016-06/ome_core/Microscope#inverted -->

    <owl:NamedIndividual rdf:about="http://www.openmicroscopy.org/rdf/2016-06/ome_core/Microscope#inverted">
        <rdf:type rdf:resource="http://www.openmicroscopy.org/rdf/2016-06/ome_core/Microscope"/>
        <rdfs:label xml:lang="en">inverted</rdfs:label>
    </owl:NamedIndividual>
    


    <!-- http://www.openmicroscopy.org/rdf/2016-06/ome_core/Microscope#upright -->

    <owl:NamedIndividual rdf:about="http://www.openmicroscopy.org/rdf/2016-06/ome_core/Microscope#upright">
        <rdf:type rdf:resource="http://www.openmicroscopy.org/rdf/2016-06/ome_core/Microscope"/>
        <rdfs:label xml:lang="en">upright</rdfs:label>
    </owl:NamedIndividual>
    


    <!-- http://www.openmicroscopy.org/rdf/2016-06/ome_core/ObjectiveMedium#air -->

    <owl:NamedIndividual rdf:about="http://www.openmicroscopy.org/rdf/2016-06/ome_core/ObjectiveMedium#air">
        <rdf:type rdf:resource="http://www.openmicroscopy.org/rdf/2016-06/ome_core/ObjectiveMedium"/>
        <rdfs:label xml:lang="en">air</rdfs:label>
    </owl:NamedIndividual>
    


    <!-- http://www.openmicroscopy.org/rdf/2016-06/ome_core/ObjectiveMedium#glycerol -->

    <owl:NamedIndividual rdf:about="http://www.openmicroscopy.org/rdf/2016-06/ome_core/ObjectiveMedium#glycerol">
        <rdf:type rdf:resource="http://www.openmicroscopy.org/rdf/2016-06/ome_core/ObjectiveMedium"/>
        <rdfs:label xml:lang="en">glycerol</rdfs:label>
    </owl:NamedIndividual>
    


    <!-- http://www.openmicroscopy.org/rdf/2016-06/ome_core/ObjectiveMedium#oil -->

    <owl:NamedIndividual rdf:about="http://www.openmicroscopy.org/rdf/2016-06/ome_core/ObjectiveMedium#oil">
        <rdf:type rdf:resource="http://www.openmicroscopy.org/rdf/2016-06/ome_core/ObjectiveMedium"/>
        <rdfs:label xml:lang="en">oil</rdfs:label>
    </owl:NamedIndividual>
    


    <!-- http://www.openmicroscopy.org/rdf/2016-06/ome_core/ObjectiveMedium#water -->

    <owl:NamedIndividual rdf:about="http://www.openmicroscopy.org/rdf/2016-06/ome_core/ObjectiveMedium#water">
        <rdf:type rdf:resource="http://www.openmicroscopy.org/rdf/2016-06/ome_core/ObjectiveMedium"/>
        <rdfs:label xml:lang="en">water</rdfs:label>
    </owl:NamedIndividual>
    


    <!-- http://www.openmicroscopy.org/rdf/2016-06/ome_core/PixelType#bit -->

    <owl:NamedIndividual rdf:about="http://www.openmicroscopy.org/rdf/2016-06/ome_core/PixelType#bit">
        <rdf:type rdf:resource="http://www.openmicroscopy.org/rdf/2016-06/ome_core/PixelType"/>
        <rdfs:label xml:lang="en">bit</rdfs:label>
    </owl:NamedIndividual>
    


    <!-- http://www.openmicroscopy.org/rdf/2016-06/ome_core/PixelType#complex -->

    <owl:NamedIndividual rdf:about="http://www.openmicroscopy.org/rdf/2016-06/ome_core/PixelType#complex">
        <rdf:type rdf:resource="http://www.openmicroscopy.org/rdf/2016-06/ome_core/PixelType"/>
        <rdfs:label xml:lang="en">complex</rdfs:label>
    </owl:NamedIndividual>
    


    <!-- http://www.openmicroscopy.org/rdf/2016-06/ome_core/PixelType#double -->

    <owl:NamedIndividual rdf:about="http://www.openmicroscopy.org/rdf/2016-06/ome_core/PixelType#double">
        <rdf:type rdf:resource="http://www.openmicroscopy.org/rdf/2016-06/ome_core/PixelType"/>
        <rdfs:label xml:lang="en">double</rdfs:label>
    </owl:NamedIndividual>
    


    <!-- http://www.openmicroscopy.org/rdf/2016-06/ome_core/PixelType#doubleComplex -->

    <owl:NamedIndividual rdf:about="http://www.openmicroscopy.org/rdf/2016-06/ome_core/PixelType#doubleComplex">
        <rdf:type rdf:resource="http://www.openmicroscopy.org/rdf/2016-06/ome_core/PixelType"/>
        <rdfs:label xml:lang="en">double-complex</rdfs:label>
    </owl:NamedIndividual>
    


    <!-- http://www.openmicroscopy.org/rdf/2016-06/ome_core/PixelType#float -->

    <owl:NamedIndividual rdf:about="http://www.openmicroscopy.org/rdf/2016-06/ome_core/PixelType#float">
        <rdf:type rdf:resource="http://www.openmicroscopy.org/rdf/2016-06/ome_core/PixelType"/>
        <rdfs:label xml:lang="en">float</rdfs:label>
    </owl:NamedIndividual>
    


    <!-- http://www.openmicroscopy.org/rdf/2016-06/ome_core/PixelType#int16 -->

    <owl:NamedIndividual rdf:about="http://www.openmicroscopy.org/rdf/2016-06/ome_core/PixelType#int16">
        <rdf:type rdf:resource="http://www.openmicroscopy.org/rdf/2016-06/ome_core/PixelType"/>
        <rdfs:label xml:lang="en">int16</rdfs:label>
    </owl:NamedIndividual>
    


    <!-- http://www.openmicroscopy.org/rdf/2016-06/ome_core/PixelType#int32 -->

    <owl:NamedIndividual rdf:about="http://www.openmicroscopy.org/rdf/2016-06/ome_core/PixelType#int32">
        <rdf:type rdf:resource="http://www.openmicroscopy.org/rdf/2016-06/ome_core/PixelType"/>
        <rdfs:label xml:lang="en">int32</rdfs:label>
    </owl:NamedIndividual>
    


    <!-- http://www.openmicroscopy.org/rdf/2016-06/ome_core/PixelType#int8 -->

    <owl:NamedIndividual rdf:about="http://www.openmicroscopy.org/rdf/2016-06/ome_core/PixelType#int8">
        <rdf:type rdf:resource="http://www.openmicroscopy.org/rdf/2016-06/ome_core/PixelType"/>
        <rdfs:label xml:lang="en">int8</rdfs:label>
    </owl:NamedIndividual>
    


    <!-- http://www.openmicroscopy.org/rdf/2016-06/ome_core/PixelType#uint16 -->

    <owl:NamedIndividual rdf:about="http://www.openmicroscopy.org/rdf/2016-06/ome_core/PixelType#uint16">
        <rdf:type rdf:resource="http://www.openmicroscopy.org/rdf/2016-06/ome_core/PixelType"/>
        <rdfs:label xml:lang="en">uint16</rdfs:label>
    </owl:NamedIndividual>
    


    <!-- http://www.openmicroscopy.org/rdf/2016-06/ome_core/PixelType#uint32 -->

    <owl:NamedIndividual rdf:about="http://www.openmicroscopy.org/rdf/2016-06/ome_core/PixelType#uint32">
        <rdf:type rdf:resource="http://www.openmicroscopy.org/rdf/2016-06/ome_core/PixelType"/>
        <rdfs:label xml:lang="en">uint32</rdfs:label>
    </owl:NamedIndividual>
    


    <!-- http://www.openmicroscopy.org/rdf/2016-06/ome_core/PixelType#uint8 -->

    <owl:NamedIndividual rdf:about="http://www.openmicroscopy.org/rdf/2016-06/ome_core/PixelType#uint8">
        <rdf:type rdf:resource="http://www.openmicroscopy.org/rdf/2016-06/ome_core/PixelType"/>
        <rdfs:label xml:lang="en">uint8</rdfs:label>
    </owl:NamedIndividual>
    


    <!-- http://www.openmicroscopy.org/rdf/2016-06/ome_core/Pulse#CW -->

    <owl:NamedIndividual rdf:about="http://www.openmicroscopy.org/rdf/2016-06/ome_core/Pulse#CW">
        <rdf:type rdf:resource="http://www.openmicroscopy.org/rdf/2016-06/ome_core/Pulse"/>
        <rdfs:label xml:lang="en">CW</rdfs:label>
    </owl:NamedIndividual>
    


    <!-- http://www.openmicroscopy.org/rdf/2016-06/ome_core/Pulse#modeLocked -->

    <owl:NamedIndividual rdf:about="http://www.openmicroscopy.org/rdf/2016-06/ome_core/Pulse#modeLocked">
        <rdf:type rdf:resource="http://www.openmicroscopy.org/rdf/2016-06/ome_core/Pulse"/>
        <rdfs:label xml:lang="en">modeLocked</rdfs:label>
    </owl:NamedIndividual>
    


    <!-- http://www.openmicroscopy.org/rdf/2016-06/ome_core/Pulse#qSwitched -->

    <owl:NamedIndividual rdf:about="http://www.openmicroscopy.org/rdf/2016-06/ome_core/Pulse#qSwitched">
        <rdf:type rdf:resource="http://www.openmicroscopy.org/rdf/2016-06/ome_core/Pulse"/>
        <rdfs:label xml:lang="en">q switched</rdfs:label>
    </owl:NamedIndividual>
    


    <!-- http://www.openmicroscopy.org/rdf/2016-06/ome_core/Pulse#repetitive -->

    <owl:NamedIndividual rdf:about="http://www.openmicroscopy.org/rdf/2016-06/ome_core/Pulse#repetitive">
        <rdf:type rdf:resource="http://www.openmicroscopy.org/rdf/2016-06/ome_core/Pulse"/>
        <rdfs:label xml:lang="en">repetitive</rdfs:label>
    </owl:NamedIndividual>
    


    <!-- http://www.openmicroscopy.org/rdf/2016-06/ome_core/Pulse#single -->

    <owl:NamedIndividual rdf:about="http://www.openmicroscopy.org/rdf/2016-06/ome_core/Pulse#single">
        <rdf:type rdf:resource="http://www.openmicroscopy.org/rdf/2016-06/ome_core/Pulse"/>
        <rdfs:label xml:lang="en">single</rdfs:label>
    </owl:NamedIndividual>
    


    <!-- 
    ///////////////////////////////////////////////////////////////////////////////////////
    //
    // Annotations
    //
    ///////////////////////////////////////////////////////////////////////////////////////
     -->

    <rdf:Description rdf:about="http://www.openmicroscopy.org/rdf/2016-06/ome_core/readOutRate">
        <rdfs:comment xml:lang="en">Property &quot;readOutRate&quot; specifies the speed at which the detector can count pixels. {used:CCD,EMCCD}  This is the bytes per second that can be read from the detector (like a baud rate).</rdfs:comment>
        <rdfs:comment xml:lang="en">Property &quot;readOutRate&quot; specifies the speed at which the detector can count pixels.</rdfs:comment>
        <rdfs:label xml:lang="en">read out rate</rdfs:label>
    </rdf:Description>
    <rdf:Description rdf:about="http://www.openmicroscopy.org/rdf/2016-06/ome_core/tagAnnotation">
        <rdfs:label xml:lang="en">tag annotation</rdfs:label>
        <rdfs:comment xml:lang="en">Property &quot;tagAnnotation&quot; specifies the annotation that represents as a tag.</rdfs:comment>
    </rdf:Description>
    <rdf:Description rdf:about="http://www.openmicroscopy.org/rdf/2016-06/ome_core/termAnnotationValue">
        <rdfs:label xml:lang="en">term annotation</rdfs:label>
        <rdfs:comment xml:lang="en">Property &quot;termAnnotation&quot; specifies the ontology term annotation.</rdfs:comment>
    </rdf:Description>
</rdf:RDF>



<!-- Generated by the OWL API (version 4.5.9.2019-02-01T07:24:44Z) https://github.com/owlcs/owlapi -->

